<?xml version="1.0"?>
<rdf:RDF xmlns="http://purl.obolibrary.org/obo/foodon.owl#"
     xml:base="http://purl.obolibrary.org/obo/foodon.owl"
     xmlns:dc="http://purl.org/dc/elements/1.1/"
     xmlns:obo="http://purl.obolibrary.org/obo/"
     xmlns:owl="http://www.w3.org/2002/07/owl#"
     xmlns:rdf="http://www.w3.org/1999/02/22-rdf-syntax-ns#"
     xmlns:xml="http://www.w3.org/XML/1998/namespace"
     xmlns:xsd="http://www.w3.org/2001/XMLSchema#"
     xmlns:rdfs="http://www.w3.org/2000/01/rdf-schema#"
     xmlns:terms="http://purl.org/dc/terms/"
     xmlns:foodon="http://purl.obolibrary.org/obo/foodon.owl#"
     xmlns:oboInOwl="http://www.geneontology.org/formats/oboInOwl#">
    <owl:Ontology rdf:about="http://purl.obolibrary.org/obo/foodon.owl">
        <owl:versionIRI rdf:resource="http://purl.obolibrary.org/obo/foodon/releases/2022-02-01/foodon.owl"/>
        <dc:contributor>Anoosha Sehar</dc:contributor>
        <dc:contributor>Damion Dooley</dc:contributor>
        <dc:contributor>Diane Alexander</dc:contributor>
        <dc:contributor>Emma Griffiths</dc:contributor>
        <dc:contributor>Gurinder Gosal</dc:contributor>
        <dc:contributor>Hande Küçük McGinty</dc:contributor>
        <dc:contributor>Lauren Chen</dc:contributor>
        <dc:contributor>Magalie Weber</dc:contributor>
        <dc:contributor>Rihannon Cameron</dc:contributor>
        <terms:date>2022-02-01</terms:date>
        <terms:description xml:lang="en">FOODON</terms:description>
        <terms:description xml:lang="en">Food Ontology (food datum subset)</terms:description>
        <terms:description xml:lang="en">FoodOn (http://foodon.org) is a consortium-driven project to build a comprehensive and easily accessible global farm-to-fork ontology about food, that accurately and consistently describes foods commonly known in cultures from around the world.</terms:description>
        <terms:license>https://creativecommons.org/licenses/by/3.0</terms:license>
    </owl:Ontology>
    


    <!-- 
    ///////////////////////////////////////////////////////////////////////////////////////
    //
    // Annotation properties
    //
    ///////////////////////////////////////////////////////////////////////////////////////
     -->


    


    <!-- http://purl.obolibrary.org/obo/IAO_0000114 -->


    <owl:AnnotationProperty rdf:about="http://purl.obolibrary.org/obo/IAO_0000114"/>
    


    <!-- http://purl.obolibrary.org/obo/IAO_0000115 -->


    <owl:AnnotationProperty rdf:about="http://purl.obolibrary.org/obo/IAO_0000115"/>
    


    <!-- http://purl.obolibrary.org/obo/IAO_0000117 -->


    <owl:AnnotationProperty rdf:about="http://purl.obolibrary.org/obo/IAO_0000117"/>
    


    <!-- http://purl.obolibrary.org/obo/IAO_0000118 -->


    <owl:AnnotationProperty rdf:about="http://purl.obolibrary.org/obo/IAO_0000118"/>
    


    <!-- http://purl.obolibrary.org/obo/IAO_0000119 -->


    <owl:AnnotationProperty rdf:about="http://purl.obolibrary.org/obo/IAO_0000119"/>
    


    <!-- http://purl.obolibrary.org/obo/IAO_0000412 -->


    <owl:AnnotationProperty rdf:about="http://purl.obolibrary.org/obo/IAO_0000412"/>
    


    <!-- http://purl.obolibrary.org/obo/foodon.owl#default-namespace -->


    <owl:AnnotationProperty rdf:about="http://purl.obolibrary.org/obo/foodon.owl#default-namespace"/>
    


    <!-- http://purl.org/dc/elements/1.1/contributor -->


    <owl:AnnotationProperty rdf:about="http://purl.org/dc/elements/1.1/contributor"/>
    


    <!-- http://purl.org/dc/elements/1.1/date -->


    <owl:AnnotationProperty rdf:about="http://purl.org/dc/elements/1.1/date"/>
    


    <!-- http://purl.org/dc/terms/date -->


    <owl:AnnotationProperty rdf:about="http://purl.org/dc/terms/date"/>
    


    <!-- http://purl.org/dc/terms/description -->


    <owl:AnnotationProperty rdf:about="http://purl.org/dc/terms/description"/>
    


    <!-- http://purl.org/dc/terms/license -->


    <owl:AnnotationProperty rdf:about="http://purl.org/dc/terms/license"/>
    


    <!-- http://purl.org/dc/terms/title -->


    <owl:AnnotationProperty rdf:about="http://purl.org/dc/terms/title"/>
    


    <!-- http://www.geneontology.org/formats/oboInOwl#hasDbXref -->


    <owl:AnnotationProperty rdf:about="http://www.geneontology.org/formats/oboInOwl#hasDbXref"/>
    


    <!-- http://www.geneontology.org/formats/oboInOwl#hasExactSynonym -->


    <owl:AnnotationProperty rdf:about="http://www.geneontology.org/formats/oboInOwl#hasExactSynonym"/>
    


    <!-- http://www.geneontology.org/formats/oboInOwl#hasSynonym -->


    <owl:AnnotationProperty rdf:about="http://www.geneontology.org/formats/oboInOwl#hasSynonym"/>
    


    <!-- http://www.w3.org/2000/01/rdf-schema#comment -->


    <owl:AnnotationProperty rdf:about="http://www.w3.org/2000/01/rdf-schema#comment"/>
    


    <!-- http://www.w3.org/2000/01/rdf-schema#label -->


    <owl:AnnotationProperty rdf:about="http://www.w3.org/2000/01/rdf-schema#label"/>
    


    <!-- http://www.w3.org/2000/01/rdf-schema#seeAlso -->


    <owl:AnnotationProperty rdf:about="http://www.w3.org/2000/01/rdf-schema#seeAlso"/>
    


    <!-- 
    ///////////////////////////////////////////////////////////////////////////////////////
    //
    // Classes
    //
    ///////////////////////////////////////////////////////////////////////////////////////
     -->


    


    <!-- http://purl.obolibrary.org/obo/FOODON_00002886 -->


    <owl:Class rdf:about="http://purl.obolibrary.org/obo/FOODON_00002886">
        <rdfs:subClassOf rdf:resource="http://purl.obolibrary.org/obo/FOODON_03510115"/>
        <obo:IAO_0000114 rdf:resource="http://purl.obolibrary.org/obo/IAO_0000428"/>
        <obo:IAO_0000115 xml:lang="en">Synbiotic claim or use refers to food ingredients or dietary supplements combining probiotics and prebiotics in a form of synergism that beneficially affect the host.</obo:IAO_0000115>
        <obo:IAO_0000117 rdf:resource="http://orcid.org/0000-0002-8844-9165"/>
        <obo:IAO_0000119 rdf:resource="https://en.wikipedia.org/wiki/Synbiotics"/>
        <dc:date rdf:datatype="http://www.w3.org/2001/XMLSchema#dateTime">2019-08-08T03:32:51Z</dc:date>
        <rdfs:label xml:lang="en">synbiotic claim or use</rdfs:label>
    </owl:Class>
    


    <!-- http://purl.obolibrary.org/obo/FOODON_00003446 -->


    <owl:Class rdf:about="http://purl.obolibrary.org/obo/FOODON_00003446">
        <rdfs:subClassOf rdf:resource="http://purl.obolibrary.org/obo/FOODON_03530005"/>
        <obo:IAO_0000114 rdf:resource="http://purl.obolibrary.org/obo/IAO_0000122"/>
        <obo:IAO_0000115 xml:lang="en">A date recommended for the use of a product while at peak quality, this date is not a reflection of safety unless used on infant formula.</obo:IAO_0000115>
        <obo:IAO_0000117 rdf:resource="http://orcid.org/0000-0002-8844-9165"/>
        <obo:IAO_0000119 rdf:resource="https://www.fsis.usda.gov/wps/portal/fsis/topics/food-safety-education/get-answers/food-safety-fact-sheets/food-labeling/food-product-dating/food-product-dating"/>
        <dc:date rdf:datatype="http://www.w3.org/2001/XMLSchema#dateTime">2020-09-22T15:01:59Z</dc:date>
        <rdfs:label xml:lang="en">food quality date</rdfs:label>
    </owl:Class>
    


    <!-- http://purl.obolibrary.org/obo/FOODON_00003451 -->


    <owl:Class rdf:about="http://purl.obolibrary.org/obo/FOODON_00003451">
        <rdfs:subClassOf rdf:resource="http://purl.obolibrary.org/obo/FOODON_00003446"/>
        <obo:IAO_0000114 rdf:resource="http://purl.obolibrary.org/obo/IAO_0000122"/>
        <obo:IAO_0000115 xml:lang="en">A date which indicates when a product should be frozen to maintain peak quality. It is not a purchase or safety date.</obo:IAO_0000115>
        <obo:IAO_0000117 rdf:resource="http://orcid.org/0000-0002-8844-9165"/>
        <obo:IAO_0000119 rdf:resource="https://www.fsis.usda.gov/wps/portal/fsis/topics/food-safety-education/get-answers/food-safety-fact-sheets/food-labeling/food-product-dating/food-product-dating"/>
        <dc:date rdf:datatype="http://www.w3.org/2001/XMLSchema#dateTime">2020-09-22T15:05:58Z</dc:date>
        <rdfs:label xml:lang="en">food freeze-by date</rdfs:label>
    </owl:Class>
    


    <!-- http://purl.obolibrary.org/obo/FOODON_00003452 -->


    <owl:Class rdf:about="http://purl.obolibrary.org/obo/FOODON_00003452">
        <rdfs:subClassOf rdf:resource="http://purl.obolibrary.org/obo/FOODON_00003446"/>
        <obo:IAO_0000114 rdf:resource="http://purl.obolibrary.org/obo/IAO_0000122"/>
        <obo:IAO_0000115 xml:lang="en">A date intended for inventory management indicating how long to display a product for retail sale.  It is not a safety date.</obo:IAO_0000115>
        <obo:IAO_0000117 rdf:resource="http://orcid.org/0000-0002-8844-9165"/>
        <obo:IAO_0000119 rdf:resource="https://www.fsis.usda.gov/wps/portal/fsis/topics/food-safety-education/get-answers/food-safety-fact-sheets/food-labeling/food-product-dating/food-product-dating"/>
        <dc:date rdf:datatype="http://www.w3.org/2001/XMLSchema#dateTime">2020-09-22T15:07:12Z</dc:date>
        <oboInOwl:hasDbXref rdf:resource="https://www.gs1.org/voc/sellByDate"/>
        <rdfs:label xml:lang="en">food sell-by date</rdfs:label>
    </owl:Class>
    


    <!-- http://purl.obolibrary.org/obo/FOODON_00003453 -->


    <owl:Class rdf:about="http://purl.obolibrary.org/obo/FOODON_00003453">
        <rdfs:subClassOf rdf:resource="http://purl.obolibrary.org/obo/FOODON_00003446"/>
        <obo:IAO_0000114 rdf:resource="http://purl.obolibrary.org/obo/IAO_0000122"/>
        <obo:IAO_0000115 xml:lang="en">A last date recommended to a consumer for the use of the product while at peak quality.</obo:IAO_0000115>
        <obo:IAO_0000117 rdf:resource="http://orcid.org/0000-0002-8844-9165"/>
        <obo:IAO_0000119 rdf:resource="https://www.fsis.usda.gov/wps/portal/fsis/topics/food-safety-education/get-answers/food-safety-fact-sheets/food-labeling/food-product-dating/food-product-dating"/>
        <dc:date rdf:datatype="http://www.w3.org/2001/XMLSchema#dateTime">2020-09-22T15:09:40Z</dc:date>
        <oboInOwl:hasDbXref rdf:resource="https://www.gs1.org/voc/bestBeforeDate"/>
        <oboInOwl:hasExactSynonym xml:lang="en">best if used by</oboInOwl:hasExactSynonym>
        <oboInOwl:hasExactSynonym xml:lang="en">use-by date</oboInOwl:hasExactSynonym>
        <rdfs:comment xml:lang="en">This is also a safety date when used on infant formula regulated by the U.S. Food and Drug Administration (FDA).</rdfs:comment>
        <rdfs:label xml:lang="en">best if used by date</rdfs:label>
    </owl:Class>
    


    <!-- http://purl.obolibrary.org/obo/FOODON_00003454 -->


    <owl:Class rdf:about="http://purl.obolibrary.org/obo/FOODON_00003454">
        <rdfs:subClassOf rdf:resource="http://purl.obolibrary.org/obo/FOODON_03530005"/>
        <obo:IAO_0000115 xml:lang="en">A food product&apos;s packaging date as marked by a food manufacturer or retailer.</obo:IAO_0000115>
        <obo:IAO_0000117 rdf:resource="http://orcid.org/0000-0002-8844-9165"/>
        <obo:IAO_0000119 rdf:resource="https://www.gs1.org/voc/packagingDate"/>
        <dc:date rdf:datatype="http://www.w3.org/2001/XMLSchema#dateTime">2020-09-22T16:46:49Z</dc:date>
        <oboInOwl:hasDbXref rdf:resource="https://www.gs1.org/voc/packagingDate"/>
        <rdfs:label xml:lang="en">food packaging date</rdfs:label>
    </owl:Class>
    


    <!-- http://purl.obolibrary.org/obo/FOODON_00003455 -->


    <owl:Class rdf:about="http://purl.obolibrary.org/obo/FOODON_00003455">
        <rdfs:subClassOf rdf:resource="http://purl.obolibrary.org/obo/FOODON_03530005"/>
        <obo:IAO_0000115 xml:lang="en">A food product&apos;s production or assembly date as marked by a food manufacturer.</obo:IAO_0000115>
        <obo:IAO_0000117 rdf:resource="http://orcid.org/0000-0002-8844-9165"/>
        <obo:IAO_0000119 rdf:resource="https://www.gs1.org/voc/productionDate"/>
        <dc:date rdf:datatype="http://www.w3.org/2001/XMLSchema#dateTime">2020-09-22T16:47:43Z</dc:date>
        <oboInOwl:hasDbXref rdf:resource="https://www.gs1.org/voc/productionDate"/>
        <rdfs:label xml:lang="en">food production date</rdfs:label>
    </owl:Class>
    


    <!-- http://purl.obolibrary.org/obo/FOODON_00003843 -->


    <owl:Class rdf:about="http://purl.obolibrary.org/obo/FOODON_00003843">
        <rdfs:subClassOf rdf:resource="http://purl.obolibrary.org/obo/FOODON_03530005"/>
        <obo:IAO_0000114 rdf:resource="http://purl.obolibrary.org/obo/IAO_0000122"/>
        <obo:IAO_0000115 xml:lang="en">A food datum which is the proportion of a nutrient remaining in a cooked food in relation to the amount of that nutrient present in a given weight of the food before cooking.</obo:IAO_0000115>
        <obo:IAO_0000117 rdf:resource="http://orcid.org/0000-0002-8844-9165"/>
        <obo:IAO_0000119 rdf:resource="https://pubmed.ncbi.nlm.nih.gov/1238446/"/>
        <dc:date rdf:datatype="http://www.w3.org/2001/XMLSchema#dateTime">2021-05-20T23:00:12Z</dc:date>
        <rdfs:comment xml:lang="en">&quot;Thus, the direct measure of true retentions requires data on the weights of the food both before and after cooking, as well as the contents of the nutrient per gram (or other unit of weight) of raw and cooked food.&quot; - Comparisons of Methods for Calculationg Retentions of Nutrients in Cooked Foods.(https://pubmed.ncbi.nlm.nih.gov/1238446/)</rdfs:comment>
        <rdfs:label xml:lang="en">true nutrient retention factor</rdfs:label>
        <rdfs:seeAlso rdf:resource="https://data.nal.usda.gov/system/files/retn06.pdf"/>
    </owl:Class>
    


    <!-- http://purl.obolibrary.org/obo/FOODON_00003844 -->


    <owl:Class rdf:about="http://purl.obolibrary.org/obo/FOODON_00003844">
        <rdfs:subClassOf rdf:resource="http://purl.obolibrary.org/obo/FOODON_03530005"/>
        <obo:IAO_0000115 xml:lang="en">A food datum which is the ratio of nutrient content in a cooked food - without inclusion of components that may have been separated during the cooking process - to nutrient content in the raw food, with both values expressed on a moisture-free basis.</obo:IAO_0000115>
        <obo:IAO_0000117 rdf:resource="http://orcid.org/0000-0002-8844-9165"/>
        <obo:IAO_0000119 rdf:resource="https://pubmed.ncbi.nlm.nih.gov/1238446/"/>
        <dc:date rdf:datatype="http://www.w3.org/2001/XMLSchema#dateTime">2021-05-20T23:00:12Z</dc:date>
        <rdfs:comment xml:lang="en">&quot;The use of apparent rather than true retentions involves the assumption that solids are not lost to any practical extent with cooking. This assumption is clearly not valid for meats, which give up both fat and protein to the drippings when cooked; it is probably not valid for vegetables, legumes, and many cereal products, either. &quot;(https://pubmed.ncbi.nlm.nih.gov/1238446/)</rdfs:comment>
        <rdfs:label xml:lang="en">apparent nutrient retention factor</rdfs:label>
    </owl:Class>
    


    <!-- http://purl.obolibrary.org/obo/FOODON_00004049 -->


    <owl:Class rdf:about="http://purl.obolibrary.org/obo/FOODON_00004049">
        <rdfs:subClassOf rdf:resource="http://purl.obolibrary.org/obo/FOODON_03530254"/>
        <obo:IAO_0000117 rdf:resource="http://orcid.org/0000-0002-8844-9165"/>
        <dc:date rdf:datatype="http://www.w3.org/2001/XMLSchema#dateTime">2021-11-11T09:56:27Z</dc:date>
        <rdfs:label xml:lang="en">Quality Wines Produced in Specified Regions</rdfs:label>
    </owl:Class>
    


    <!-- http://purl.obolibrary.org/obo/FOODON_00004053 -->


    <owl:Class rdf:about="http://purl.obolibrary.org/obo/FOODON_00004053">
        <rdfs:subClassOf rdf:resource="http://purl.obolibrary.org/obo/FOODON_03530087"/>
        <rdfs:label xml:lang="en">Vintners Quality Alliance</rdfs:label>
    </owl:Class>
    


    <!-- http://purl.obolibrary.org/obo/FOODON_00004054 -->


    <owl:Class rdf:about="http://purl.obolibrary.org/obo/FOODON_00004054">
        <rdfs:subClassOf rdf:resource="http://purl.obolibrary.org/obo/FOODON_03530087"/>
        <rdfs:label xml:lang="en">American Viticultural Area</rdfs:label>
    </owl:Class>
    


    <!-- http://purl.obolibrary.org/obo/FOODON_00004055 -->


    <owl:Class rdf:about="http://purl.obolibrary.org/obo/FOODON_00004055">
        <rdfs:subClassOf rdf:resource="http://purl.obolibrary.org/obo/FOODON_03530087"/>
        <obo:IAO_0000114 rdf:resource="http://purl.obolibrary.org/obo/IAO_0000122"/>
        <obo:IAO_0000119 rdf:resource="https://en.wikipedia.org/wiki/Denominaci%C3%B3n_de_origen"/>
        <rdfs:comment xml:lang="en">&quot;In wines, it parallels the hierarchical systems of France (1935) and Italy (1963), although Rioja (1925) and Jerez (1933) preceded the full system.&quot;[https://en.wikipedia.org/wiki/Denominaci%C3%B3n_de_origen]</rdfs:comment>
        <rdfs:label xml:lang="en">Denominación de origen</rdfs:label>
    </owl:Class>
    


    <!-- http://purl.obolibrary.org/obo/FOODON_00004056 -->


    <owl:Class rdf:about="http://purl.obolibrary.org/obo/FOODON_00004056">
        <rdfs:subClassOf rdf:resource="http://purl.obolibrary.org/obo/FOODON_03530087"/>
        <rdfs:label xml:lang="en">Spanish wine production framework</rdfs:label>
    </owl:Class>
    


    <!-- http://purl.obolibrary.org/obo/FOODON_00004057 -->


    <owl:Class rdf:about="http://purl.obolibrary.org/obo/FOODON_00004057">
        <rdfs:subClassOf rdf:resource="http://purl.obolibrary.org/obo/FOODON_00004056"/>
        <rdfs:label xml:lang="en">Denominación de Origen Protegida</rdfs:label>
    </owl:Class>
    


    <!-- http://purl.obolibrary.org/obo/FOODON_00004058 -->


    <owl:Class rdf:about="http://purl.obolibrary.org/obo/FOODON_00004058">
        <rdfs:subClassOf rdf:resource="http://purl.obolibrary.org/obo/FOODON_00004056"/>
        <rdfs:label xml:lang="en">Denominación de Origen Calificada</rdfs:label>
    </owl:Class>
    


    <!-- http://purl.obolibrary.org/obo/FOODON_00004059 -->


    <owl:Class rdf:about="http://purl.obolibrary.org/obo/FOODON_00004059">
        <rdfs:subClassOf rdf:resource="http://purl.obolibrary.org/obo/FOODON_00004056"/>
        <rdfs:label xml:lang="en">Vino de Pago</rdfs:label>
    </owl:Class>
    


    <!-- http://purl.obolibrary.org/obo/FOODON_00004060 -->


    <owl:Class rdf:about="http://purl.obolibrary.org/obo/FOODON_00004060">
        <rdfs:subClassOf rdf:resource="http://purl.obolibrary.org/obo/FOODON_00004056"/>
        <rdfs:label xml:lang="en">Vino de Calidad con indicación geográfica</rdfs:label>
    </owl:Class>
    


    <!-- http://purl.obolibrary.org/obo/FOODON_00004061 -->


    <owl:Class rdf:about="http://purl.obolibrary.org/obo/FOODON_00004061">
        <rdfs:subClassOf rdf:resource="http://purl.obolibrary.org/obo/FOODON_00004056"/>
        <rdfs:label xml:lang="en">Indicación geográfica protegida</rdfs:label>
    </owl:Class>
    


    <!-- http://purl.obolibrary.org/obo/FOODON_00004062 -->


    <owl:Class rdf:about="http://purl.obolibrary.org/obo/FOODON_00004062">
        <rdfs:subClassOf rdf:resource="http://purl.obolibrary.org/obo/FOODON_00004056"/>
        <rdfs:label xml:lang="en">Vino de Mesa</rdfs:label>
    </owl:Class>
    


    <!-- http://purl.obolibrary.org/obo/FOODON_03510017 -->


    <owl:Class rdf:about="http://purl.obolibrary.org/obo/FOODON_03510017">
        <rdfs:subClassOf rdf:resource="http://purl.obolibrary.org/obo/FOODON_03510065"/>
        <obo:IAO_0000114 rdf:resource="http://purl.obolibrary.org/obo/IAO_0000428"/>
        <obo:IAO_0000115 xml:lang="en">All narrower term definitions extracted from 58 Federal Register 2302, January 6, 1993, part 101.62(b).</obo:IAO_0000115>
        <obo:IAO_0000412>http://langual.org</obo:IAO_0000412>
        <oboInOwl:hasDbXref>http://www.langual.org/langual_thesaurus.asp?termid=P0017</oboInOwl:hasDbXref>
        <rdfs:label xml:lang="en">fat special claim or use</rdfs:label>
    </owl:Class>
    


    <!-- http://purl.obolibrary.org/obo/FOODON_03510023 -->


    <owl:Class rdf:about="http://purl.obolibrary.org/obo/FOODON_03510023">
        <rdfs:subClassOf rdf:resource="http://purl.obolibrary.org/obo/FOODON_03510032"/>
        <obo:IAO_0000114 rdf:resource="http://purl.obolibrary.org/obo/IAO_0000428"/>
        <obo:IAO_0000115 xml:lang="en">Renamed from *FOOD FOR SPECIAL DIETARY USE* [LanguaL 2008].

These descriptors are used either for foods intended for special dietary use as defined in 21 CFR 105 or for foods that have special characteristics indicated in the name or labeling. Such claims would include &apos;low calorie&apos;, &apos;low cholesterol&apos;, &apos;diet&apos; or &apos;dietetic&apos;, etc. Prior to february 1992, this category of descriptors was limited solely to food for adult humans. The category is now used in conjunction with any appropriate *CONSUMER GROUP* descriptor(s), for example, &apos;low sugar baby food&apos; would be indexed by *INFANT OR TODDLER FOOD* as well as by *LOW SUGARS FOOD*.</obo:IAO_0000115>
        <obo:IAO_0000412>http://langual.org</obo:IAO_0000412>
        <oboInOwl:hasDbXref>http://www.langual.org/langual_thesaurus.asp?termid=P0023</oboInOwl:hasDbXref>
        <oboInOwl:hasSynonym xml:lang="en">dietary food</oboInOwl:hasSynonym>
        <oboInOwl:hasSynonym xml:lang="en">dietary use</oboInOwl:hasSynonym>
        <oboInOwl:hasSynonym xml:lang="en">food for dietary use</oboInOwl:hasSynonym>
        <oboInOwl:hasSynonym xml:lang="en">food for special dietary use</oboInOwl:hasSynonym>
        <oboInOwl:hasSynonym xml:lang="en">special dietary food</oboInOwl:hasSynonym>
        <rdfs:label xml:lang="en">dietary claim or use</rdfs:label>
    </owl:Class>
    


    <!-- http://purl.obolibrary.org/obo/FOODON_03510032 -->


    <owl:Class rdf:about="http://purl.obolibrary.org/obo/FOODON_03510032">
        <rdfs:subClassOf rdf:resource="http://purl.obolibrary.org/obo/FOODON_03530005"/>
        <obo:IAO_0000114 rdf:resource="http://purl.obolibrary.org/obo/IAO_0000428"/>
        <obo:IAO_0000115 xml:lang="en">Dietary use, where the food has special characteristics, claims or uses or is intended for individuals with particular dietary needs; and label or labeling claims, used when special dietary use factor terms were derived from actual food labels. Multiple descriptors may be used from all three categories. [FDA CFSAN 1995]</obo:IAO_0000115>
        <obo:IAO_0000412>http://langual.org</obo:IAO_0000412>
        <oboInOwl:hasDbXref>http://www.langual.org/langual_thesaurus.asp?termid=P0032</oboInOwl:hasDbXref>
        <rdfs:label xml:lang="en">dietary use/label claim</rdfs:label>
    </owl:Class>
    


    <!-- http://purl.obolibrary.org/obo/FOODON_03510033 -->


    <owl:Class rdf:about="http://purl.obolibrary.org/obo/FOODON_03510033">
        <rdfs:subClassOf rdf:resource="http://purl.obolibrary.org/obo/FOODON_03510066"/>
        <obo:IAO_0000114 rdf:resource="http://purl.obolibrary.org/obo/IAO_0000428"/>
        <obo:IAO_0000115 xml:lang="en">A claim that a food is low in energy, and any claim likely to have the same meaning for the consumer, may only be made where the product does not contain more than 40 kcal (170 kJ)/100 g for solids or more than 20 kcal (80 kJ)/100 ml for liquids. For table-top sweeteners the limit of 4 kcal (17 kJ)/portion, with equivalent sweetening properties to 6 g of sucrose (approximately 1 teaspoon of sucrose), applies [REGULATION (EC) No 1924/2006 Corrigendum 2007-01-18].

Food having 40 calories or less per amount customarily consumed (and per 50 grams of food if the amount customarily consumed is small). Meals and main dishes contain 120 calories or less per 100 grams of food [US FDA]</obo:IAO_0000115>
        <obo:IAO_0000412>http://langual.org</obo:IAO_0000412>
        <oboInOwl:hasDbXref>http://www.langual.org/langual_thesaurus.asp?termid=P0033</oboInOwl:hasDbXref>
        <oboInOwl:hasSynonym xml:lang="en">low calorie food</oboInOwl:hasSynonym>
        <rdfs:comment xml:lang="en">LanguaL curation note: Renamed from *LOW CALORIE FOOD* [LanguaL 2008].</rdfs:comment>
        <rdfs:label xml:lang="en">low energy food claim or use</rdfs:label>
    </owl:Class>
    


    <!-- http://purl.obolibrary.org/obo/FOODON_03510034 -->


    <owl:Class rdf:about="http://purl.obolibrary.org/obo/FOODON_03510034">
        <rdfs:subClassOf rdf:resource="http://purl.obolibrary.org/obo/FOODON_03510066"/>
        <obo:IAO_0000114 rdf:resource="http://purl.obolibrary.org/obo/IAO_0000428"/>
        <obo:IAO_0000115 xml:lang="en">A claim that a food is energy-reduced, and any claim likely to have the same meaning for the consumer, may only be made where the energy value is reduced by at least 30 %, with an indication of the characteristic(s) which make(s) the
food reduced in its total energy value [REGULATION (EC) No 1924/2006 Corrigendum 2007-01-18].

Food having at least 25% fewer calories per amount customarily consumed from the calories of a comparable food product. The complarable food may not be &apos;low calorie&apos; [US FDA].</obo:IAO_0000115>
        <obo:IAO_0000412>http://langual.org</obo:IAO_0000412>
        <oboInOwl:hasDbXref>http://www.langual.org/langual_thesaurus.asp?termid=P0034</oboInOwl:hasDbXref>
        <oboInOwl:hasSynonym xml:lang="en">reduced calorie food</oboInOwl:hasSynonym>
        <rdfs:comment xml:lang="en">LanguaL curation note: Renamed from *REDUCED CALORIE FOOD* [LanguaL 2008].</rdfs:comment>
        <rdfs:label xml:lang="en">reduced energy food claim or use</rdfs:label>
    </owl:Class>
    


    <!-- http://purl.obolibrary.org/obo/FOODON_03510035 -->


    <owl:Class rdf:about="http://purl.obolibrary.org/obo/FOODON_03510035">
        <rdfs:subClassOf rdf:resource="http://purl.obolibrary.org/obo/FOODON_03510077"/>
        <obo:IAO_0000114 rdf:resource="http://purl.obolibrary.org/obo/IAO_0000428"/>
        <obo:IAO_0000115 xml:lang="en">A claim that a food is sodium-free or salt-free, and any claim likely to have the same meaning for the consumer, may only be made where the product contains no more than 0,005 g of sodium, or the equivalent value for salt, per 100 g. [REGULATION (EC) No 1924/2006 Corrigendum 2007-01-18].

Food having less than 5 milligrams of salt or sodium per amount customarily consumed (or for meals and main dishes, less than 5 miligrams of salt or sodium per labeled serving). Such foods must not contain an ingredient that is salt or sodium or generally understood to comtain salt or sodium except where the ingredient listed is footnoted &apos;*adds a trivial amount of {salt or sodium}&apos; [US FDA]</obo:IAO_0000115>
        <obo:IAO_0000412>http://langual.org</obo:IAO_0000412>
        <oboInOwl:hasDbXref>http://www.langual.org/langual_thesaurus.asp?termid=P0035</oboInOwl:hasDbXref>
        <oboInOwl:hasSynonym xml:lang="en">sodium or salt free food</oboInOwl:hasSynonym>
        <rdfs:label xml:lang="en">salt or sodium free claim or use</rdfs:label>
    </owl:Class>
    


    <!-- http://purl.obolibrary.org/obo/FOODON_03510036 -->


    <owl:Class rdf:about="http://purl.obolibrary.org/obo/FOODON_03510036">
        <rdfs:subClassOf rdf:resource="http://purl.obolibrary.org/obo/FOODON_03510077"/>
        <obo:IAO_0000114 rdf:resource="http://purl.obolibrary.org/obo/IAO_0000428"/>
        <obo:IAO_0000115 xml:lang="en">A claim that a food is very low in sodium/salt, and any claim likely to have the same meaning for the consumer, may only be made where the product contains no more than 0,04 g of sodium, or the equivalent value for salt, per 100 g or per 100 ml. This claim shall not be used for natural mineral waters and other waters [REGULATION (EC) No 1924/2006 Corrigendum 2007-01-18].

Food having 35 milligrams or less salt or sodium per amount customarily consumed (and per 50 grams if the amount customarily consumed is small). Meals and main dishes contain 35 milligrams or less salt or sodium per 100 grams of food [US FDA]</obo:IAO_0000115>
        <obo:IAO_0000412>http://langual.org</obo:IAO_0000412>
        <oboInOwl:hasDbXref>http://www.langual.org/langual_thesaurus.asp?termid=P0036</oboInOwl:hasDbXref>
        <oboInOwl:hasSynonym xml:lang="en">very low sodium or salt food</oboInOwl:hasSynonym>
        <rdfs:label xml:lang="en">very low salt or sodium claim or use</rdfs:label>
    </owl:Class>
    


    <!-- http://purl.obolibrary.org/obo/FOODON_03510037 -->


    <owl:Class rdf:about="http://purl.obolibrary.org/obo/FOODON_03510037">
        <rdfs:subClassOf rdf:resource="http://purl.obolibrary.org/obo/FOODON_03510077"/>
        <obo:IAO_0000114 rdf:resource="http://purl.obolibrary.org/obo/IAO_0000428"/>
        <obo:IAO_0000412>http://langual.org</obo:IAO_0000412>
        <oboInOwl:hasDbXref>http://www.langual.org/langual_thesaurus.asp?termid=P0037</oboInOwl:hasDbXref>
        <oboInOwl:hasSynonym xml:lang="en">reduced sodium or salt food</oboInOwl:hasSynonym>
        <rdfs:label xml:lang="en">reduced salt or sodium claim or use</rdfs:label>
    </owl:Class>
    


    <!-- http://purl.obolibrary.org/obo/FOODON_03510038 -->


    <owl:Class rdf:about="http://purl.obolibrary.org/obo/FOODON_03510038">
        <rdfs:subClassOf rdf:resource="http://purl.obolibrary.org/obo/FOODON_03510077"/>
        <obo:IAO_0000114 rdf:resource="http://purl.obolibrary.org/obo/IAO_0000428"/>
        <obo:IAO_0000115 xml:lang="en">A claim that a food is low in sodium/salt, and any claim likely to have the same meaning for the consumer, may only be made where the product contains no more than 0,12 g of sodium, or the equivalent value for salt, per 100 g or per 100 ml. For waters, other than natural mineral waters falling within the scope of Directive 80/777/EEC, this value should not exceed 2 mg of sodium per 100 ml [REGULATION (EC) No 1924/2006 Corrigendum 2007-01-18].

Food having 140 milligrams or less salt or sodium per amount customarily consumed. Meals and main dishes have 140 milligrams or less salt or sodium per 100 grams food [US FDA]</obo:IAO_0000115>
        <obo:IAO_0000412>http://langual.org</obo:IAO_0000412>
        <oboInOwl:hasDbXref>http://www.langual.org/langual_thesaurus.asp?termid=P0038</oboInOwl:hasDbXref>
        <oboInOwl:hasSynonym xml:lang="en">low sodium or salt food</oboInOwl:hasSynonym>
        <rdfs:label xml:lang="en">low salt or sodium claim or use</rdfs:label>
    </owl:Class>
    


    <!-- http://purl.obolibrary.org/obo/FOODON_03510039 -->


    <owl:Class rdf:about="http://purl.obolibrary.org/obo/FOODON_03510039">
        <rdfs:subClassOf rdf:resource="http://purl.obolibrary.org/obo/FOODON_03510069"/>
        <obo:IAO_0000114 rdf:resource="http://purl.obolibrary.org/obo/IAO_0000428"/>
        <obo:IAO_0000115 xml:lang="en">A claim that a food is low in fat, and any claim likely to have the same meaning for the consumer, may only be made where the product contains no more than 3 g of fat per 100 g for solids or 1,5 g of fat per 100 ml for liquids (1,8 g of fat per 100 ml for semi-skimmed milk). [REGULATION (EC) No 1924/2006 Corrigendum 2007-01-18].

Food having 3 grams of fat or less per amount customarily consumed (and per 50 grams of food if the amount customarily consumed is small). Meals and main dishes contain 3 grams or less fat per 100 grams of food and not more than 30% of calories from fat [US FDA].</obo:IAO_0000115>
        <obo:IAO_0000412>http://langual.org</obo:IAO_0000412>
        <oboInOwl:hasDbXref>http://www.langual.org/langual_thesaurus.asp?termid=P0039</oboInOwl:hasDbXref>
        <rdfs:label xml:lang="en">low fat food</rdfs:label>
    </owl:Class>
    


    <!-- http://purl.obolibrary.org/obo/FOODON_03510040 -->


    <owl:Class rdf:about="http://purl.obolibrary.org/obo/FOODON_03510040">
        <rdfs:subClassOf rdf:resource="http://purl.obolibrary.org/obo/FOODON_03510069"/>
        <obo:IAO_0000114 rdf:resource="http://purl.obolibrary.org/obo/IAO_0000428"/>
        <obo:IAO_0000115 xml:lang="en">Food containing at least 25% less fat per amount customarily consumed from the fat content of a comparable food product. The comparable food may not be &apos;low fat&apos;.</obo:IAO_0000115>
        <obo:IAO_0000412>http://langual.org</obo:IAO_0000412>
        <oboInOwl:hasDbXref>http://www.langual.org/langual_thesaurus.asp?termid=P0040</oboInOwl:hasDbXref>
        <rdfs:label xml:lang="en">reduced fat food</rdfs:label>
    </owl:Class>
    


    <!-- http://purl.obolibrary.org/obo/FOODON_03510041 -->


    <owl:Class rdf:about="http://purl.obolibrary.org/obo/FOODON_03510041">
        <rdfs:subClassOf rdf:resource="http://purl.obolibrary.org/obo/FOODON_03510065"/>
        <obo:IAO_0000114 rdf:resource="http://purl.obolibrary.org/obo/IAO_0000428"/>
        <obo:IAO_0000115 xml:lang="en">All narrower term definitions extracted from 58 Federal Register 2302, January 6, 1993, part 101.62(d).</obo:IAO_0000115>
        <obo:IAO_0000412>http://langual.org</obo:IAO_0000412>
        <oboInOwl:hasDbXref>http://www.langual.org/langual_thesaurus.asp?termid=P0041</oboInOwl:hasDbXref>
        <rdfs:label xml:lang="en">cholesterol special claim or use</rdfs:label>
    </owl:Class>
    


    <!-- http://purl.obolibrary.org/obo/FOODON_03510042 -->


    <owl:Class rdf:about="http://purl.obolibrary.org/obo/FOODON_03510042">
        <rdfs:subClassOf rdf:resource="http://purl.obolibrary.org/obo/FOODON_03510149"/>
        <obo:IAO_0000114 rdf:resource="http://purl.obolibrary.org/obo/IAO_0000428"/>
        <obo:IAO_0000115 xml:lang="en">Food having less than 2 milligrams cholesterol per amount customarily consumed (or for meals and main dishes, less than 2 milligrams cholesterol per labeled serving). Such food must contain no ingredient that contains cholesterol except where the ingredient listed has been footnoted &apos;*adds a trivial amount of cholesterol&apos;. If the food contains less than 2 milligrams cholesterol per amount customarily consumed by special processing and the total fat exceeds 13 grams cholesterol per amount or labeled serving, the amount of cholesterol must be &apos;Substantially less&apos; (25%) than in a comparable food with significant market share (5% of market).</obo:IAO_0000115>
        <obo:IAO_0000412>http://langual.org</obo:IAO_0000412>
        <oboInOwl:hasDbXref>http://www.langual.org/langual_thesaurus.asp?termid=P0042</oboInOwl:hasDbXref>
        <oboInOwl:hasSynonym xml:lang="en">no cholesterol food</oboInOwl:hasSynonym>
        <rdfs:label xml:lang="en">cholesterol free claim or use</rdfs:label>
    </owl:Class>
    


    <!-- http://purl.obolibrary.org/obo/FOODON_03510043 -->


    <owl:Class rdf:about="http://purl.obolibrary.org/obo/FOODON_03510043">
        <rdfs:subClassOf rdf:resource="http://purl.obolibrary.org/obo/FOODON_03510149"/>
        <obo:IAO_0000114 rdf:resource="http://purl.obolibrary.org/obo/IAO_0000428"/>
        <obo:IAO_0000115 xml:lang="en">Food having 20 miligrams or less cholesterol per amount customarily consumed (and per 50 grams of food if the amount customarily consumed is small). Meals and main dishes contain 20 milligrams or less cholesterol per 100 grams of food. If the food qualifies by special processing and total fat exceeds 13 grams per amount and labeled serving, the amount of cholesterol must be &apos;substantially less&apos; (25%) than in a comparable food with significant market share (5% of market).</obo:IAO_0000115>
        <obo:IAO_0000412>http://langual.org</obo:IAO_0000412>
        <oboInOwl:hasDbXref>http://www.langual.org/langual_thesaurus.asp?termid=P0043</oboInOwl:hasDbXref>
        <rdfs:label xml:lang="en">low in cholesterol claim or use</rdfs:label>
    </owl:Class>
    


    <!-- http://purl.obolibrary.org/obo/FOODON_03510044 -->


    <owl:Class rdf:about="http://purl.obolibrary.org/obo/FOODON_03510044">
        <rdfs:subClassOf rdf:resource="http://purl.obolibrary.org/obo/FOODON_03510149"/>
        <obo:IAO_0000114 rdf:resource="http://purl.obolibrary.org/obo/IAO_0000428"/>
        <obo:IAO_0000115 xml:lang="en">Food having at least 25% less cholesterol per amount customarily consumed from the cholesterol content of a comparable food product. The comparable food may not be &apos;low cholesterol&apos;.</obo:IAO_0000115>
        <obo:IAO_0000412>http://langual.org</obo:IAO_0000412>
        <oboInOwl:hasDbXref>http://www.langual.org/langual_thesaurus.asp?termid=P0044</oboInOwl:hasDbXref>
        <rdfs:label xml:lang="en">reduced cholesterol claim or use</rdfs:label>
    </owl:Class>
    


    <!-- http://purl.obolibrary.org/obo/FOODON_03510045 -->


    <owl:Class rdf:about="http://purl.obolibrary.org/obo/FOODON_03510045">
        <rdfs:subClassOf rdf:resource="http://purl.obolibrary.org/obo/FOODON_03510065"/>
        <obo:IAO_0000114 rdf:resource="http://purl.obolibrary.org/obo/IAO_0000428"/>
        <obo:IAO_0000115 xml:lang="en">All narrower term definitions are extracted from 58 Federal Register 2302, January 6, 1993, part 101.60(b) and from Corrigendum to Regulation (EC) No 1924/2006 of the European Parliament and of the Council of 20 December 2006 on nutrition and health claims made on foods.</obo:IAO_0000115>
        <obo:IAO_0000412>http://langual.org</obo:IAO_0000412>
        <oboInOwl:hasDbXref>http://www.langual.org/langual_thesaurus.asp?termid=P0045</oboInOwl:hasDbXref>
        <oboInOwl:hasSynonym xml:lang="en">calorie special claim or use</oboInOwl:hasSynonym>
        <rdfs:comment xml:lang="en">LanguaL curation note: Renamed from *CALORIE SPECIAL CLAIM OR USE*.</rdfs:comment>
        <rdfs:label xml:lang="en">energy special claim or use</rdfs:label>
    </owl:Class>
    


    <!-- http://purl.obolibrary.org/obo/FOODON_03510047 -->


    <owl:Class rdf:about="http://purl.obolibrary.org/obo/FOODON_03510047">
        <rdfs:subClassOf rdf:resource="http://purl.obolibrary.org/obo/FOODON_03510065"/>
        <obo:IAO_0000114 rdf:resource="http://purl.obolibrary.org/obo/IAO_0000428"/>
        <obo:IAO_0000115 xml:lang="en">All narrower term definitions extracted from 58 Federal Register 2032, January 6, 1993, part 101.61.</obo:IAO_0000115>
        <obo:IAO_0000412>http://langual.org</obo:IAO_0000412>
        <oboInOwl:hasDbXref>http://www.langual.org/langual_thesaurus.asp?termid=P0047</oboInOwl:hasDbXref>
        <oboInOwl:hasSynonym xml:lang="en">sodium or salt special diet</oboInOwl:hasSynonym>
        <rdfs:label xml:lang="en">salt or sodium special claim or use</rdfs:label>
    </owl:Class>
    


    <!-- http://purl.obolibrary.org/obo/FOODON_03510048 -->


    <owl:Class rdf:about="http://purl.obolibrary.org/obo/FOODON_03510048">
        <rdfs:subClassOf rdf:resource="http://purl.obolibrary.org/obo/FOODON_03510049"/>
        <obo:IAO_0000114 rdf:resource="http://purl.obolibrary.org/obo/IAO_0000428"/>
        <obo:IAO_0000115 xml:lang="en">A claim that a food is high in fibre, and any claim likely to have the same meaning for the consumer, may only be made where the product contains at least 6 g of fibre per 100 g or at least 3 g of fibre per 100 kcal [REGULATION (EC) No 1924/2006 Corrigendum 2007-01-18].

Food that is promoted as a source of or as high in dietary fiber (often called simply &apos;fiber&apos;).</obo:IAO_0000115>
        <obo:IAO_0000412>http://langual.org</obo:IAO_0000412>
        <oboInOwl:hasDbXref>http://www.langual.org/langual_thesaurus.asp?termid=P0048</oboInOwl:hasDbXref>
        <oboInOwl:hasSynonym xml:lang="en">high dietary fiber food</oboInOwl:hasSynonym>
        <rdfs:label xml:lang="en">high fiber food</rdfs:label>
    </owl:Class>
    


    <!-- http://purl.obolibrary.org/obo/FOODON_03510049 -->


    <owl:Class rdf:about="http://purl.obolibrary.org/obo/FOODON_03510049">
        <rdfs:subClassOf rdf:resource="http://purl.obolibrary.org/obo/FOODON_03510065"/>
        <obo:IAO_0000114 rdf:resource="http://purl.obolibrary.org/obo/IAO_0000428"/>
        <obo:IAO_0000115 xml:lang="en">Food that is promoted as being either high or low in dietary fiber (often called simply &apos;fiber&apos;). If the food is not low in total fat, total fat must be stated in conjunction with claim such as &apos;more fiber&apos;.</obo:IAO_0000115>
        <obo:IAO_0000412>http://langual.org</obo:IAO_0000412>
        <oboInOwl:hasDbXref>http://www.langual.org/langual_thesaurus.asp?termid=P0049</oboInOwl:hasDbXref>
        <oboInOwl:hasSynonym xml:lang="en">dietary fiber special claim or use</oboInOwl:hasSynonym>
        <rdfs:label xml:lang="en">fiber special claim or use</rdfs:label>
    </owl:Class>
    


    <!-- http://purl.obolibrary.org/obo/FOODON_03510054 -->


    <owl:Class rdf:about="http://purl.obolibrary.org/obo/FOODON_03510054">
        <rdfs:subClassOf rdf:resource="http://purl.obolibrary.org/obo/FOODON_03510069"/>
        <obo:IAO_0000114 rdf:resource="http://purl.obolibrary.org/obo/IAO_0000428"/>
        <obo:IAO_0000115 xml:lang="en">A claim that a food is fat-free, and any claim likely to have the same meaning for the consumer, may only be made where the product contains no more than 0,5 g of fat per 100 g or 100 ml. However, claims expressed as &quot;X % fat-free&quot; shall be prohibited [REGULATION (EC) No 1924/2006 Corrigendum].

Food having less than 0.5 grams fat per amount customarily consumed. Meals and main dishes have less than 0.5 grams fat per labeled serving. Such foods must contain no ingredient that is fat or understood to contain fat except when the ingredient listed has been footnoted &apos;*adds a trivial amount of fat&apos;.</obo:IAO_0000115>
        <obo:IAO_0000412>http://langual.org</obo:IAO_0000412>
        <oboInOwl:hasDbXref>http://www.langual.org/langual_thesaurus.asp?termid=P0054</oboInOwl:hasDbXref>
        <oboInOwl:hasSynonym xml:lang="en">no fat food</oboInOwl:hasSynonym>
        <oboInOwl:hasSynonym xml:lang="en">nonfat food</oboInOwl:hasSynonym>
        <rdfs:label xml:lang="en">fat free food</rdfs:label>
    </owl:Class>
    


    <!-- http://purl.obolibrary.org/obo/FOODON_03510055 -->


    <owl:Class rdf:about="http://purl.obolibrary.org/obo/FOODON_03510055">
        <rdfs:subClassOf rdf:resource="http://purl.obolibrary.org/obo/FOODON_03510066"/>
        <obo:IAO_0000114 rdf:resource="http://purl.obolibrary.org/obo/IAO_0000428"/>
        <obo:IAO_0000115 xml:lang="en">A claim that a food is energy-free, and any claim likely to have the same meaning for the consumer, may only be made where the product does not contain more than 4 kcal (17 kJ)/100 ml. For table-top sweeteners the limit of 0.4 kcal (1.7 kJ)/portion, with equivalent sweetening properties to 6 g of sucrose (approximately 1 teaspoon of sucrose), applies [REGULATION (EC) No 1924/2006 Corrigendum 2007-01-18].

Food having less than 5 calories per amount customarily consumed. Calorie amount is not defined for meals or main dishes [US FDA]</obo:IAO_0000115>
        <obo:IAO_0000412>http://langual.org</obo:IAO_0000412>
        <oboInOwl:hasDbXref>http://www.langual.org/langual_thesaurus.asp?termid=P0055</oboInOwl:hasDbXref>
        <oboInOwl:hasSynonym xml:lang="en">calorie free food</oboInOwl:hasSynonym>
        <rdfs:comment xml:lang="en">LanguaL curation note: Renamed from *CALORIE FREE FOOD* [LanguaL 2008].</rdfs:comment>
        <rdfs:label xml:lang="en">energy free food claim or use</rdfs:label>
    </owl:Class>
    


    <!-- http://purl.obolibrary.org/obo/FOODON_03510056 -->


    <owl:Class rdf:about="http://purl.obolibrary.org/obo/FOODON_03510056">
        <rdfs:subClassOf rdf:resource="http://purl.obolibrary.org/obo/FOODON_03510091"/>
        <obo:IAO_0000114 rdf:resource="http://purl.obolibrary.org/obo/IAO_0000428"/>
        <obo:IAO_0000115 xml:lang="en">A claim that a food is sugars-free, and any claim likely to have the same meaning for the consumer, may only be made where the product contains no more than 0,5 g of sugars per 100 g or 100 ml [REGULATION (EC) No 1924/2006 Corrigendum 2007-01-18].

Food having less than 0.5 grams sugars per amount customarily consumed (or for meals and main dishes, less than 0.5 grams sugars per labeled serving). Such foods nust contain no ingredient that is a sugar or generally understood to contain sugars except where the ingredient listed is footnoted &apos;*adds a trivial amount of sugars&apos; [US FDA]</obo:IAO_0000115>
        <obo:IAO_0000412>http://langual.org</obo:IAO_0000412>
        <oboInOwl:hasDbXref>http://www.langual.org/langual_thesaurus.asp?termid=P0056</oboInOwl:hasDbXref>
        <oboInOwl:hasSynonym xml:lang="en">sugar free food</oboInOwl:hasSynonym>
        <rdfs:label xml:lang="en">sugars free food</rdfs:label>
    </owl:Class>
    


    <!-- http://purl.obolibrary.org/obo/FOODON_03510057 -->


    <owl:Class rdf:about="http://purl.obolibrary.org/obo/FOODON_03510057">
        <rdfs:subClassOf rdf:resource="http://purl.obolibrary.org/obo/FOODON_03510071"/>
        <obo:IAO_0000114 rdf:resource="http://purl.obolibrary.org/obo/IAO_0000428"/>
        <obo:IAO_0000115 xml:lang="en">A claim that a food is low in saturated fat, and any claim likely to have the same meaning for the consumer, may only be made if the sum of saturated fatty acids and trans-fatty acids in the product does not exceed 1.5 g per 100 g for solids or 0.75 g/100 ml for liquids and in either case the sum of saturated fatty acids and trans-fatty acids must not provide more than 10 % of energy. [REGULATION (EC) No 1924/2006 Corrigendum 2007-01-18].

Food having one gram or less saturated fat per amount customarily consumed and 15% or less of calories from saturated fat. Meals and main dishes contain one gram or less saturated fat per 100 grams food and less than 10% of calories from saturated fat.</obo:IAO_0000115>
        <obo:IAO_0000412>http://langual.org</obo:IAO_0000412>
        <oboInOwl:hasDbXref>http://www.langual.org/langual_thesaurus.asp?termid=P0057</oboInOwl:hasDbXref>
        <rdfs:label xml:lang="en">low in saturated fat food</rdfs:label>
    </owl:Class>
    


    <!-- http://purl.obolibrary.org/obo/FOODON_03510059 -->


    <owl:Class rdf:about="http://purl.obolibrary.org/obo/FOODON_03510059">
        <rdfs:subClassOf rdf:resource="http://purl.obolibrary.org/obo/FOODON_03510023"/>
        <obo:IAO_0000114 rdf:resource="http://purl.obolibrary.org/obo/IAO_0000428"/>
        <obo:IAO_0000412>http://langual.org</obo:IAO_0000412>
        <oboInOwl:hasDbXref>http://www.langual.org/langual_thesaurus.asp?termid=P0059</oboInOwl:hasDbXref>
        <oboInOwl:hasSynonym xml:lang="en">label claim</oboInOwl:hasSynonym>
        <rdfs:comment xml:lang="en">LanguaL curation note: Renamed from *LABEL CLAIM* [LanguaL 2008].

Use when any &apos;claim or use&apos; index term is derived from either the food name appearing on the label or from information appearing on the label that is separate from the food name.</rdfs:comment>
        <rdfs:label xml:lang="en">general label claim</rdfs:label>
    </owl:Class>
    


    <!-- http://purl.obolibrary.org/obo/FOODON_03510060 -->


    <owl:Class rdf:about="http://purl.obolibrary.org/obo/FOODON_03510060">
        <rdfs:subClassOf rdf:resource="http://purl.obolibrary.org/obo/FOODON_03510045"/>
        <obo:IAO_0000114 rdf:resource="http://purl.obolibrary.org/obo/IAO_0000428"/>
        <obo:IAO_0000115 xml:lang="en">[REGULATION (EC) No 1924/2006 Corrigendum 2007-01-18]</obo:IAO_0000115>
        <obo:IAO_0000412>http://langual.org</obo:IAO_0000412>
        <oboInOwl:hasDbXref>http://www.langual.org/langual_thesaurus.asp?termid=P0060</oboInOwl:hasDbXref>
        <oboInOwl:hasSynonym xml:lang="en">high calorie food</oboInOwl:hasSynonym>
        <rdfs:comment xml:lang="en">LanguaL curation note: Renamed from *HIGH CALORIE FOOD* [LanguaL 2008].</rdfs:comment>
        <rdfs:label xml:lang="en">high energy food claim or use</rdfs:label>
    </owl:Class>
    


    <!-- http://purl.obolibrary.org/obo/FOODON_03510061 -->


    <owl:Class rdf:about="http://purl.obolibrary.org/obo/FOODON_03510061">
        <rdfs:subClassOf rdf:resource="http://purl.obolibrary.org/obo/FOODON_03510065"/>
        <rdfs:subClassOf rdf:resource="http://purl.obolibrary.org/obo/FOODON_03510103"/>
        <obo:IAO_0000114 rdf:resource="http://purl.obolibrary.org/obo/IAO_0000428"/>
        <obo:IAO_0000115 xml:lang="en">All narrower term definitions extracted from 58 Federal Register 2302, January 6, 1993, part 101.60(c).</obo:IAO_0000115>
        <obo:IAO_0000412>http://langual.org</obo:IAO_0000412>
        <oboInOwl:hasDbXref>http://www.langual.org/langual_thesaurus.asp?termid=P0061</oboInOwl:hasDbXref>
        <rdfs:label xml:lang="en">sugars special claim or use</rdfs:label>
    </owl:Class>
    


    <!-- http://purl.obolibrary.org/obo/FOODON_03510062 -->


    <owl:Class rdf:about="http://purl.obolibrary.org/obo/FOODON_03510062">
        <rdfs:subClassOf rdf:resource="http://purl.obolibrary.org/obo/FOODON_03510090"/>
        <obo:IAO_0000114 rdf:resource="http://purl.obolibrary.org/obo/IAO_0000428"/>
        <obo:IAO_0000115 xml:lang="en">A claim that a food is low in sugars, and any claim likely to have the same meaning for the consumer, may only be made where the product contains no more than 5 g of sugars per 100 g for solids or 2,5 g of sugars per 100 ml for liquids [REGULATION (EC) No 1924/2006 Corrigendum 2007-01-18].

Not defined in U.S. Federal Register; no basis for a recommended intake.</obo:IAO_0000115>
        <obo:IAO_0000412>http://langual.org</obo:IAO_0000412>
        <oboInOwl:hasDbXref>http://www.langual.org/langual_thesaurus.asp?termid=P0062</oboInOwl:hasDbXref>
        <rdfs:label xml:lang="en">low sugars food</rdfs:label>
    </owl:Class>
    


    <!-- http://purl.obolibrary.org/obo/FOODON_03510063 -->


    <owl:Class rdf:about="http://purl.obolibrary.org/obo/FOODON_03510063">
        <rdfs:subClassOf rdf:resource="http://purl.obolibrary.org/obo/FOODON_03510049"/>
        <obo:IAO_0000114 rdf:resource="http://purl.obolibrary.org/obo/IAO_0000428"/>
        <obo:IAO_0000412>http://langual.org</obo:IAO_0000412>
        <oboInOwl:hasDbXref>http://www.langual.org/langual_thesaurus.asp?termid=P0063</oboInOwl:hasDbXref>
        <rdfs:label xml:lang="en">low fiber food</rdfs:label>
    </owl:Class>
    


    <!-- http://purl.obolibrary.org/obo/FOODON_03510065 -->


    <owl:Class rdf:about="http://purl.obolibrary.org/obo/FOODON_03510065">
        <rdfs:subClassOf rdf:resource="http://purl.obolibrary.org/obo/FOODON_03510023"/>
        <obo:IAO_0000114 rdf:resource="http://purl.obolibrary.org/obo/IAO_0000428"/>
        <obo:IAO_0000115 xml:lang="en">As defined in Corrigendum to Regulation (EC) No 1924/2006 of the European Parliament and of the Council of 20 December 2006 on nutrition and health claims made on foods, &quot;claim&quot; means any message or representation, which is not
mandatory under Community or national legislation, including pictorial, graphic or symbolic representation, in any form, which states, suggests or implies that a food has particular characteristics; specificly, &quot;nutrition claim&quot; means any claim which states, suggests or implies that a food has particular beneficial nutritional properties
due to:

(a) the energy (calorific value) it (i) provides; (ii) provides at a reduced or increased rate; or (iii) does not provide;

and/or

(b) the nutrients or other substances it (i) contains; (ii) contains in reduced or  increased proportions; or (iii) does not contain.</obo:IAO_0000115>
        <obo:IAO_0000412>http://langual.org</obo:IAO_0000412>
        <oboInOwl:hasDbXref>http://www.langual.org/langual_thesaurus.asp?termid=P0065</oboInOwl:hasDbXref>
        <rdfs:comment xml:lang="en">LanguaL curation note: Used for  any claim which states, suggests or implies that a food has particular beneficial nutritional properties.

For European regulations, see http://ec.europa.eu/food/food/labellingnutrition/claims/community_register/nutrition_claims_en.htm</rdfs:comment>
        <rdfs:label xml:lang="en">nutrition-related claim or use</rdfs:label>
    </owl:Class>
    


    <!-- http://purl.obolibrary.org/obo/FOODON_03510066 -->


    <owl:Class rdf:about="http://purl.obolibrary.org/obo/FOODON_03510066">
        <rdfs:subClassOf rdf:resource="http://purl.obolibrary.org/obo/FOODON_03510045"/>
        <obo:IAO_0000114 rdf:resource="http://purl.obolibrary.org/obo/IAO_0000428"/>
        <obo:IAO_0000412>http://langual.org</obo:IAO_0000412>
        <oboInOwl:hasDbXref>http://www.langual.org/langual_thesaurus.asp?termid=P0066</oboInOwl:hasDbXref>
        <oboInOwl:hasSynonym xml:lang="en">no or reduced calories claim or use</oboInOwl:hasSynonym>
        <oboInOwl:hasSynonym xml:lang="en">reduced or no calories claim or use</oboInOwl:hasSynonym>
        <oboInOwl:hasSynonym xml:lang="en">reduced or no energy claim or use</oboInOwl:hasSynonym>
        <rdfs:comment xml:lang="en">LanguaL curation note: Renamed from *NO OR REDUCED CALORIES CLAIM OR USE* [LanguaL 2008].</rdfs:comment>
        <rdfs:label xml:lang="en">no or reduced energy claim or use</rdfs:label>
    </owl:Class>
    


    <!-- http://purl.obolibrary.org/obo/FOODON_03510069 -->


    <owl:Class rdf:about="http://purl.obolibrary.org/obo/FOODON_03510069">
        <rdfs:subClassOf rdf:resource="http://purl.obolibrary.org/obo/FOODON_03510017"/>
        <obo:IAO_0000114 rdf:resource="http://purl.obolibrary.org/obo/IAO_0000428"/>
        <obo:IAO_0000412>http://langual.org</obo:IAO_0000412>
        <oboInOwl:hasDbXref>http://www.langual.org/langual_thesaurus.asp?termid=P0069</oboInOwl:hasDbXref>
        <oboInOwl:hasSynonym xml:lang="en">reduced or no fat claim or use</oboInOwl:hasSynonym>
        <rdfs:label xml:lang="en">no or reduced fat claim or use</rdfs:label>
    </owl:Class>
    


    <!-- http://purl.obolibrary.org/obo/FOODON_03510070 -->


    <owl:Class rdf:about="http://purl.obolibrary.org/obo/FOODON_03510070">
        <rdfs:subClassOf rdf:resource="http://purl.obolibrary.org/obo/FOODON_03510069"/>
        <obo:IAO_0000114 rdf:resource="http://purl.obolibrary.org/obo/IAO_0000428"/>
        <obo:IAO_0000412>http://langual.org</obo:IAO_0000412>
        <oboInOwl:hasDbXref>http://www.langual.org/langual_thesaurus.asp?termid=P0070</oboInOwl:hasDbXref>
        <rdfs:label xml:lang="en">no fat added claim or use</rdfs:label>
    </owl:Class>
    


    <!-- http://purl.obolibrary.org/obo/FOODON_03510071 -->


    <owl:Class rdf:about="http://purl.obolibrary.org/obo/FOODON_03510071">
        <rdfs:subClassOf rdf:resource="http://purl.obolibrary.org/obo/FOODON_03510017"/>
        <obo:IAO_0000114 rdf:resource="http://purl.obolibrary.org/obo/IAO_0000428"/>
        <obo:IAO_0000115 xml:lang="en">All narrower term definitions extracted from 58 Federal Register 2302, January 6, 1993, part 101.62(c).</obo:IAO_0000115>
        <obo:IAO_0000412>http://langual.org</obo:IAO_0000412>
        <oboInOwl:hasDbXref>http://www.langual.org/langual_thesaurus.asp?termid=P0071</oboInOwl:hasDbXref>
        <rdfs:label xml:lang="en">saturated fat-related claim or use</rdfs:label>
    </owl:Class>
    


    <!-- http://purl.obolibrary.org/obo/FOODON_03510072 -->


    <owl:Class rdf:about="http://purl.obolibrary.org/obo/FOODON_03510072">
        <rdfs:subClassOf rdf:resource="http://purl.obolibrary.org/obo/FOODON_03510071"/>
        <obo:IAO_0000114 rdf:resource="http://purl.obolibrary.org/obo/IAO_0000428"/>
        <obo:IAO_0000412>http://langual.org</obo:IAO_0000412>
        <oboInOwl:hasDbXref>http://www.langual.org/langual_thesaurus.asp?termid=P0072</oboInOwl:hasDbXref>
        <rdfs:label xml:lang="en">no animal fat added claim or use</rdfs:label>
    </owl:Class>
    


    <!-- http://purl.obolibrary.org/obo/FOODON_03510073 -->


    <owl:Class rdf:about="http://purl.obolibrary.org/obo/FOODON_03510073">
        <rdfs:subClassOf rdf:resource="http://purl.obolibrary.org/obo/FOODON_03510071"/>
        <obo:IAO_0000114 rdf:resource="http://purl.obolibrary.org/obo/IAO_0000428"/>
        <obo:IAO_0000412>http://langual.org</obo:IAO_0000412>
        <oboInOwl:hasDbXref>http://www.langual.org/langual_thesaurus.asp?termid=P0073</oboInOwl:hasDbXref>
        <oboInOwl:hasSynonym xml:lang="en">no coconut oil added claim or use</oboInOwl:hasSynonym>
        <rdfs:label xml:lang="en">no tropical oils added claim or use</rdfs:label>
    </owl:Class>
    


    <!-- http://purl.obolibrary.org/obo/FOODON_03510074 -->


    <owl:Class rdf:about="http://purl.obolibrary.org/obo/FOODON_03510074">
        <rdfs:subClassOf rdf:resource="http://purl.obolibrary.org/obo/FOODON_03510071"/>
        <obo:IAO_0000114 rdf:resource="http://purl.obolibrary.org/obo/IAO_0000428"/>
        <obo:IAO_0000412>http://langual.org</obo:IAO_0000412>
        <oboInOwl:hasDbXref>http://www.langual.org/langual_thesaurus.asp?termid=P0074</oboInOwl:hasDbXref>
        <rdfs:label xml:lang="en">no palm oil added claim or use</rdfs:label>
    </owl:Class>
    


    <!-- http://purl.obolibrary.org/obo/FOODON_03510075 -->


    <owl:Class rdf:about="http://purl.obolibrary.org/obo/FOODON_03510075">
        <rdfs:subClassOf rdf:resource="http://purl.obolibrary.org/obo/FOODON_03510049"/>
        <obo:IAO_0000114 rdf:resource="http://purl.obolibrary.org/obo/IAO_0000428"/>
        <obo:IAO_0000412>http://langual.org</obo:IAO_0000412>
        <oboInOwl:hasDbXref>http://www.langual.org/langual_thesaurus.asp?termid=P0075</oboInOwl:hasDbXref>
        <oboInOwl:hasSynonym xml:lang="en">fiber rich claim or use</oboInOwl:hasSynonym>
        <rdfs:label xml:lang="en">rich in fiber claim or use</rdfs:label>
    </owl:Class>
    


    <!-- http://purl.obolibrary.org/obo/FOODON_03510076 -->


    <owl:Class rdf:about="http://purl.obolibrary.org/obo/FOODON_03510076">
        <rdfs:subClassOf rdf:resource="http://purl.obolibrary.org/obo/FOODON_03510075"/>
        <obo:IAO_0000114 rdf:resource="http://purl.obolibrary.org/obo/IAO_0000428"/>
        <obo:IAO_0000412>http://langual.org</obo:IAO_0000412>
        <oboInOwl:hasDbXref>http://www.langual.org/langual_thesaurus.asp?termid=P0076</oboInOwl:hasDbXref>
        <oboInOwl:hasSynonym xml:lang="en">natural fiber source</oboInOwl:hasSynonym>
        <rdfs:label xml:lang="en">naturally rich in fiber claim or use</rdfs:label>
    </owl:Class>
    


    <!-- http://purl.obolibrary.org/obo/FOODON_03510077 -->


    <owl:Class rdf:about="http://purl.obolibrary.org/obo/FOODON_03510077">
        <rdfs:subClassOf rdf:resource="http://purl.obolibrary.org/obo/FOODON_03510047"/>
        <obo:IAO_0000114 rdf:resource="http://purl.obolibrary.org/obo/IAO_0000428"/>
        <obo:IAO_0000412>http://langual.org</obo:IAO_0000412>
        <oboInOwl:hasDbXref>http://www.langual.org/langual_thesaurus.asp?termid=P0077</oboInOwl:hasDbXref>
        <oboInOwl:hasSynonym xml:lang="en">less salt added claim or use</oboInOwl:hasSynonym>
        <oboInOwl:hasSynonym xml:lang="en">reduced or no salt or sodium claim or use</oboInOwl:hasSynonym>
        <rdfs:label xml:lang="en">no or reduced salt or sodium claim or use</rdfs:label>
    </owl:Class>
    


    <!-- http://purl.obolibrary.org/obo/FOODON_03510078 -->


    <owl:Class rdf:about="http://purl.obolibrary.org/obo/FOODON_03510078">
        <rdfs:subClassOf rdf:resource="http://purl.obolibrary.org/obo/FOODON_03510077"/>
        <obo:IAO_0000114 rdf:resource="http://purl.obolibrary.org/obo/IAO_0000428"/>
        <obo:IAO_0000412>http://langual.org</obo:IAO_0000412>
        <oboInOwl:hasDbXref>http://www.langual.org/langual_thesaurus.asp?termid=P0078</oboInOwl:hasDbXref>
        <oboInOwl:hasSynonym xml:lang="en">unsalted claim or use</oboInOwl:hasSynonym>
        <rdfs:comment xml:lang="en">LanguaL curation note: No salt added and &apos;unsalted&apos; must meet conditions of use and must declare &apos;this is not a sodium free food&apos; on the information panel if the food is not &apos;sodium free&apos;. (28 Federal Register 2302, January 6, 1993).</rdfs:comment>
        <rdfs:label xml:lang="en">no salt added claim or use</rdfs:label>
    </owl:Class>
    


    <!-- http://purl.obolibrary.org/obo/FOODON_03510080 -->


    <owl:Class rdf:about="http://purl.obolibrary.org/obo/FOODON_03510080">
        <rdfs:subClassOf rdf:resource="http://purl.obolibrary.org/obo/FOODON_03510035"/>
        <obo:IAO_0000114 rdf:resource="http://purl.obolibrary.org/obo/IAO_0000428"/>
        <obo:IAO_0000115 xml:lang="en">Food having less than 5 milligrams salt per amount customarily consumed (or for meals and main dishes less than 5 milligrams salt per labeled serving). Such food must contain no ingredient that is salt or generally understood to contain salt except where the ingredient listed is footnoted &apos;*adds a trivial amount of salt&apos;.</obo:IAO_0000115>
        <obo:IAO_0000412>http://langual.org</obo:IAO_0000412>
        <oboInOwl:hasDbXref>http://www.langual.org/langual_thesaurus.asp?termid=P0080</oboInOwl:hasDbXref>
        <rdfs:label xml:lang="en">salt free claim or use</rdfs:label>
    </owl:Class>
    


    <!-- http://purl.obolibrary.org/obo/FOODON_03510083 -->


    <owl:Class rdf:about="http://purl.obolibrary.org/obo/FOODON_03510083">
        <rdfs:subClassOf rdf:resource="http://purl.obolibrary.org/obo/FOODON_03510038"/>
        <obo:IAO_0000114 rdf:resource="http://purl.obolibrary.org/obo/IAO_0000428"/>
        <obo:IAO_0000412>http://langual.org</obo:IAO_0000412>
        <oboInOwl:hasDbXref>http://www.langual.org/langual_thesaurus.asp?termid=P0083</oboInOwl:hasDbXref>
        <rdfs:label xml:lang="en">low salt claim or use</rdfs:label>
    </owl:Class>
    


    <!-- http://purl.obolibrary.org/obo/FOODON_03510085 -->


    <owl:Class rdf:about="http://purl.obolibrary.org/obo/FOODON_03510085">
        <rdfs:subClassOf rdf:resource="http://purl.obolibrary.org/obo/FOODON_03510036"/>
        <obo:IAO_0000114 rdf:resource="http://purl.obolibrary.org/obo/IAO_0000428"/>
        <obo:IAO_0000115 xml:lang="en">Food having less than 35 milligrams of salt per serving and per 100 grams of food. (U.S. proposed)</obo:IAO_0000115>
        <obo:IAO_0000412>http://langual.org</obo:IAO_0000412>
        <oboInOwl:hasDbXref>http://www.langual.org/langual_thesaurus.asp?termid=P0085</oboInOwl:hasDbXref>
        <rdfs:label xml:lang="en">very low salt claim or use</rdfs:label>
    </owl:Class>
    


    <!-- http://purl.obolibrary.org/obo/FOODON_03510087 -->


    <owl:Class rdf:about="http://purl.obolibrary.org/obo/FOODON_03510087">
        <rdfs:subClassOf rdf:resource="http://purl.obolibrary.org/obo/FOODON_03510037"/>
        <obo:IAO_0000114 rdf:resource="http://purl.obolibrary.org/obo/IAO_0000428"/>
        <obo:IAO_0000412>http://langual.org</obo:IAO_0000412>
        <oboInOwl:hasDbXref>http://www.langual.org/langual_thesaurus.asp?termid=P0087</oboInOwl:hasDbXref>
        <rdfs:label xml:lang="en">reduced salt claim or use</rdfs:label>
    </owl:Class>
    


    <!-- http://purl.obolibrary.org/obo/FOODON_03510088 -->


    <owl:Class rdf:about="http://purl.obolibrary.org/obo/FOODON_03510088">
        <rdfs:subClassOf rdf:resource="http://purl.obolibrary.org/obo/FOODON_03510152"/>
        <obo:IAO_0000114 rdf:resource="http://purl.obolibrary.org/obo/IAO_0000428"/>
        <obo:IAO_0000412>http://langual.org</obo:IAO_0000412>
        <oboInOwl:hasDbXref>http://www.langual.org/langual_thesaurus.asp?termid=P0088</oboInOwl:hasDbXref>
        <rdfs:label xml:lang="en">naturally sodium-free food</rdfs:label>
    </owl:Class>
    


    <!-- http://purl.obolibrary.org/obo/FOODON_03510090 -->


    <owl:Class rdf:about="http://purl.obolibrary.org/obo/FOODON_03510090">
        <rdfs:subClassOf rdf:resource="http://purl.obolibrary.org/obo/FOODON_03510061"/>
        <obo:IAO_0000114 rdf:resource="http://purl.obolibrary.org/obo/IAO_0000428"/>
        <obo:IAO_0000412>http://langual.org</obo:IAO_0000412>
        <oboInOwl:hasDbXref>http://www.langual.org/langual_thesaurus.asp?termid=P0090</oboInOwl:hasDbXref>
        <oboInOwl:hasSynonym xml:lang="en">reduced or no sugar label claim</oboInOwl:hasSynonym>
        <rdfs:label xml:lang="en">no or reduced sugar claim or use</rdfs:label>
    </owl:Class>
    


    <!-- http://purl.obolibrary.org/obo/FOODON_03510091 -->


    <owl:Class rdf:about="http://purl.obolibrary.org/obo/FOODON_03510091">
        <rdfs:subClassOf rdf:resource="http://purl.obolibrary.org/obo/FOODON_03510090"/>
        <obo:IAO_0000114 rdf:resource="http://purl.obolibrary.org/obo/IAO_0000428"/>
        <obo:IAO_0000115 xml:lang="en">A claim stating that sugars have not been added to a food, and any claim likely to have the same meaning for the consumer, may only be made where the product does not contain any added mono- or disaccharides or any other food used for its sweetening properties. If sugars are naturally present in the food, the following indication should also appear on the label: &quot;CONTAINS NATURALLY OCCURRING SUGARS&quot; [REGULATION (EC) No 1924/2006 Corrigendum].

No added sugars and &apos;without added sugars&apos; are allowed if no sugar or sugar containing ingredient is added during processing. (28 Federal Register 2302, January 6, 1993)</obo:IAO_0000115>
        <obo:IAO_0000412>http://langual.org</obo:IAO_0000412>
        <oboInOwl:hasDbXref>http://www.langual.org/langual_thesaurus.asp?termid=P0091</oboInOwl:hasDbXref>
        <rdfs:label xml:lang="en">no sugars added claim or use</rdfs:label>
    </owl:Class>
    


    <!-- http://purl.obolibrary.org/obo/FOODON_03510092 -->


    <owl:Class rdf:about="http://purl.obolibrary.org/obo/FOODON_03510092">
        <rdfs:subClassOf rdf:resource="http://purl.obolibrary.org/obo/FOODON_03510065"/>
        <obo:IAO_0000114 rdf:resource="http://purl.obolibrary.org/obo/IAO_0000428"/>
        <obo:IAO_0000412>http://langual.org</obo:IAO_0000412>
        <oboInOwl:hasDbXref>http://www.langual.org/langual_thesaurus.asp?termid=P0092</oboInOwl:hasDbXref>
        <rdfs:label xml:lang="en">starch-related claim or use</rdfs:label>
    </owl:Class>
    


    <!-- http://purl.obolibrary.org/obo/FOODON_03510093 -->


    <owl:Class rdf:about="http://purl.obolibrary.org/obo/FOODON_03510093">
        <rdfs:subClassOf rdf:resource="http://purl.obolibrary.org/obo/FOODON_03510092"/>
        <obo:IAO_0000114 rdf:resource="http://purl.obolibrary.org/obo/IAO_0000428"/>
        <obo:IAO_0000412>http://langual.org</obo:IAO_0000412>
        <oboInOwl:hasDbXref>http://www.langual.org/langual_thesaurus.asp?termid=P0093</oboInOwl:hasDbXref>
        <rdfs:label xml:lang="en">no modified food starch added claim or use</rdfs:label>
    </owl:Class>
    


    <!-- http://purl.obolibrary.org/obo/FOODON_03510094 -->


    <owl:Class rdf:about="http://purl.obolibrary.org/obo/FOODON_03510094">
        <rdfs:subClassOf rdf:resource="http://purl.obolibrary.org/obo/FOODON_03510092"/>
        <obo:IAO_0000114 rdf:resource="http://purl.obolibrary.org/obo/IAO_0000428"/>
        <obo:IAO_0000412>http://langual.org</obo:IAO_0000412>
        <oboInOwl:hasDbXref>http://www.langual.org/langual_thesaurus.asp?termid=P0094</oboInOwl:hasDbXref>
        <rdfs:label xml:lang="en">no starch added claim or use</rdfs:label>
    </owl:Class>
    


    <!-- http://purl.obolibrary.org/obo/FOODON_03510095 -->


    <owl:Class rdf:about="http://purl.obolibrary.org/obo/FOODON_03510095">
        <rdfs:subClassOf rdf:resource="http://purl.obolibrary.org/obo/FOODON_03510065"/>
        <obo:IAO_0000114 rdf:resource="http://purl.obolibrary.org/obo/IAO_0000428"/>
        <obo:IAO_0000412>http://langual.org</obo:IAO_0000412>
        <oboInOwl:hasDbXref>http://www.langual.org/langual_thesaurus.asp?termid=P0095</oboInOwl:hasDbXref>
        <oboInOwl:hasSynonym xml:lang="en">mineral- or vitamin-related claim or use</oboInOwl:hasSynonym>
        <rdfs:label xml:lang="en">vitamin- or mineral-related claim or use</rdfs:label>
    </owl:Class>
    


    <!-- http://purl.obolibrary.org/obo/FOODON_03510096 -->


    <owl:Class rdf:about="http://purl.obolibrary.org/obo/FOODON_03510096">
        <rdfs:subClassOf rdf:resource="http://purl.obolibrary.org/obo/FOODON_03510023"/>
        <obo:IAO_0000114 rdf:resource="http://purl.obolibrary.org/obo/IAO_0000428"/>
        <obo:IAO_0000412>http://langual.org</obo:IAO_0000412>
        <oboInOwl:hasDbXref>http://www.langual.org/langual_thesaurus.asp?termid=P0096</oboInOwl:hasDbXref>
        <rdfs:label xml:lang="en">color-related claim or use</rdfs:label>
    </owl:Class>
    


    <!-- http://purl.obolibrary.org/obo/FOODON_03510097 -->


    <owl:Class rdf:about="http://purl.obolibrary.org/obo/FOODON_03510097">
        <rdfs:subClassOf rdf:resource="http://purl.obolibrary.org/obo/FOODON_03510096"/>
        <rdfs:subClassOf rdf:resource="http://purl.obolibrary.org/obo/FOODON_03510106"/>
        <obo:IAO_0000114 rdf:resource="http://purl.obolibrary.org/obo/IAO_0000428"/>
        <obo:IAO_0000412>http://langual.org</obo:IAO_0000412>
        <oboInOwl:hasDbXref>http://www.langual.org/langual_thesaurus.asp?termid=P0097</oboInOwl:hasDbXref>
        <rdfs:label xml:lang="en">no artificial colors claim or use</rdfs:label>
    </owl:Class>
    


    <!-- http://purl.obolibrary.org/obo/FOODON_03510098 -->


    <owl:Class rdf:about="http://purl.obolibrary.org/obo/FOODON_03510098">
        <rdfs:subClassOf rdf:resource="http://purl.obolibrary.org/obo/FOODON_03510096"/>
        <obo:IAO_0000114 rdf:resource="http://purl.obolibrary.org/obo/IAO_0000428"/>
        <obo:IAO_0000412>http://langual.org</obo:IAO_0000412>
        <oboInOwl:hasDbXref>http://www.langual.org/langual_thesaurus.asp?termid=P0098</oboInOwl:hasDbXref>
        <rdfs:label xml:lang="en">no color added claim or use</rdfs:label>
    </owl:Class>
    


    <!-- http://purl.obolibrary.org/obo/FOODON_03510099 -->


    <owl:Class rdf:about="http://purl.obolibrary.org/obo/FOODON_03510099">
        <rdfs:subClassOf rdf:resource="http://purl.obolibrary.org/obo/FOODON_03510023"/>
        <obo:IAO_0000114 rdf:resource="http://purl.obolibrary.org/obo/IAO_0000428"/>
        <obo:IAO_0000412>http://langual.org</obo:IAO_0000412>
        <oboInOwl:hasDbXref>http://www.langual.org/langual_thesaurus.asp?termid=P0099</oboInOwl:hasDbXref>
        <oboInOwl:hasSynonym xml:lang="en">taste- or flavor-related claim or use</oboInOwl:hasSynonym>
        <rdfs:label xml:lang="en">flavor- or taste-related claim or use</rdfs:label>
    </owl:Class>
    


    <!-- http://purl.obolibrary.org/obo/FOODON_03510100 -->


    <owl:Class rdf:about="http://purl.obolibrary.org/obo/FOODON_03510100">
        <rdfs:subClassOf rdf:resource="http://purl.obolibrary.org/obo/FOODON_03510099"/>
        <rdfs:subClassOf rdf:resource="http://purl.obolibrary.org/obo/FOODON_03510106"/>
        <obo:IAO_0000114 rdf:resource="http://purl.obolibrary.org/obo/IAO_0000428"/>
        <obo:IAO_0000412>http://langual.org</obo:IAO_0000412>
        <oboInOwl:hasDbXref>http://www.langual.org/langual_thesaurus.asp?termid=P0100</oboInOwl:hasDbXref>
        <oboInOwl:hasSynonym xml:lang="en">all natural flavors claim or use</oboInOwl:hasSynonym>
        <rdfs:label xml:lang="en">no artificial flavors claim or use</rdfs:label>
    </owl:Class>
    


    <!-- http://purl.obolibrary.org/obo/FOODON_03510102 -->


    <owl:Class rdf:about="http://purl.obolibrary.org/obo/FOODON_03510102">
        <rdfs:subClassOf rdf:resource="http://purl.obolibrary.org/obo/FOODON_03510099"/>
        <obo:IAO_0000114 rdf:resource="http://purl.obolibrary.org/obo/IAO_0000428"/>
        <obo:IAO_0000412>http://langual.org</obo:IAO_0000412>
        <oboInOwl:hasDbXref>http://www.langual.org/langual_thesaurus.asp?termid=P0102</oboInOwl:hasDbXref>
        <rdfs:label xml:lang="en">no flavor added claim or use</rdfs:label>
    </owl:Class>
    


    <!-- http://purl.obolibrary.org/obo/FOODON_03510103 -->


    <owl:Class rdf:about="http://purl.obolibrary.org/obo/FOODON_03510103">
        <rdfs:subClassOf rdf:resource="http://purl.obolibrary.org/obo/FOODON_03510023"/>
        <obo:IAO_0000114 rdf:resource="http://purl.obolibrary.org/obo/IAO_0000428"/>
        <obo:IAO_0000412>http://langual.org</obo:IAO_0000412>
        <oboInOwl:hasDbXref>http://www.langual.org/langual_thesaurus.asp?termid=P0103</oboInOwl:hasDbXref>
        <rdfs:label xml:lang="en">sweetener-related claim or use</rdfs:label>
    </owl:Class>
    


    <!-- http://purl.obolibrary.org/obo/FOODON_03510104 -->


    <owl:Class rdf:about="http://purl.obolibrary.org/obo/FOODON_03510104">
        <rdfs:subClassOf rdf:resource="http://purl.obolibrary.org/obo/FOODON_03510103"/>
        <rdfs:subClassOf rdf:resource="http://purl.obolibrary.org/obo/FOODON_03510106"/>
        <obo:IAO_0000114 rdf:resource="http://purl.obolibrary.org/obo/IAO_0000428"/>
        <obo:IAO_0000412>http://langual.org</obo:IAO_0000412>
        <oboInOwl:hasDbXref>http://www.langual.org/langual_thesaurus.asp?termid=P0104</oboInOwl:hasDbXref>
        <rdfs:label xml:lang="en">no artificial sweeteners claim or use</rdfs:label>
    </owl:Class>
    


    <!-- http://purl.obolibrary.org/obo/FOODON_03510105 -->


    <owl:Class rdf:about="http://purl.obolibrary.org/obo/FOODON_03510105">
        <rdfs:subClassOf rdf:resource="http://purl.obolibrary.org/obo/FOODON_03510103"/>
        <obo:IAO_0000114 rdf:resource="http://purl.obolibrary.org/obo/IAO_0000428"/>
        <obo:IAO_0000412>http://langual.org</obo:IAO_0000412>
        <oboInOwl:hasDbXref>http://www.langual.org/langual_thesaurus.asp?termid=P0105</oboInOwl:hasDbXref>
        <rdfs:label xml:lang="en">unsweetened claim or use</rdfs:label>
    </owl:Class>
    


    <!-- http://purl.obolibrary.org/obo/FOODON_03510106 -->


    <owl:Class rdf:about="http://purl.obolibrary.org/obo/FOODON_03510106">
        <rdfs:subClassOf rdf:resource="http://purl.obolibrary.org/obo/FOODON_03510023"/>
        <obo:IAO_0000114 rdf:resource="http://purl.obolibrary.org/obo/IAO_0000428"/>
        <obo:IAO_0000412>http://langual.org</obo:IAO_0000412>
        <oboInOwl:hasDbXref>http://www.langual.org/langual_thesaurus.asp?termid=P0106</oboInOwl:hasDbXref>
        <rdfs:label xml:lang="en">artificial ingredient-related claim or use</rdfs:label>
    </owl:Class>
    


    <!-- http://purl.obolibrary.org/obo/FOODON_03510107 -->


    <owl:Class rdf:about="http://purl.obolibrary.org/obo/FOODON_03510107">
        <rdfs:subClassOf rdf:resource="http://purl.obolibrary.org/obo/FOODON_03510106"/>
        <obo:IAO_0000114 rdf:resource="http://purl.obolibrary.org/obo/IAO_0000428"/>
        <obo:IAO_0000412>http://langual.org</obo:IAO_0000412>
        <oboInOwl:hasDbXref>http://www.langual.org/langual_thesaurus.asp?termid=P0107</oboInOwl:hasDbXref>
        <oboInOwl:hasSynonym xml:lang="en">all natural claim or use</oboInOwl:hasSynonym>
        <rdfs:label xml:lang="en">no artificial ingredients claim or use</rdfs:label>
    </owl:Class>
    


    <!-- http://purl.obolibrary.org/obo/FOODON_03510108 -->


    <owl:Class rdf:about="http://purl.obolibrary.org/obo/FOODON_03510108">
        <rdfs:subClassOf rdf:resource="http://purl.obolibrary.org/obo/FOODON_03510106"/>
        <obo:IAO_0000114 rdf:resource="http://purl.obolibrary.org/obo/IAO_0000428"/>
        <obo:IAO_0000412>http://langual.org</obo:IAO_0000412>
        <oboInOwl:hasDbXref>http://www.langual.org/langual_thesaurus.asp?termid=P0108</oboInOwl:hasDbXref>
        <rdfs:label xml:lang="en">no artificial additives claim or use</rdfs:label>
    </owl:Class>
    


    <!-- http://purl.obolibrary.org/obo/FOODON_03510110 -->


    <owl:Class rdf:about="http://purl.obolibrary.org/obo/FOODON_03510110">
        <rdfs:subClassOf rdf:resource="http://purl.obolibrary.org/obo/FOODON_03510023"/>
        <obo:IAO_0000114 rdf:resource="http://purl.obolibrary.org/obo/IAO_0000428"/>
        <obo:IAO_0000412>http://langual.org</obo:IAO_0000412>
        <oboInOwl:hasDbXref>http://www.langual.org/langual_thesaurus.asp?termid=P0110</oboInOwl:hasDbXref>
        <rdfs:label xml:lang="en">preservative-related claim or use</rdfs:label>
    </owl:Class>
    


    <!-- http://purl.obolibrary.org/obo/FOODON_03510111 -->


    <owl:Class rdf:about="http://purl.obolibrary.org/obo/FOODON_03510111">
        <rdfs:subClassOf rdf:resource="http://purl.obolibrary.org/obo/FOODON_03510106"/>
        <rdfs:subClassOf rdf:resource="http://purl.obolibrary.org/obo/FOODON_03510110"/>
        <obo:IAO_0000114 rdf:resource="http://purl.obolibrary.org/obo/IAO_0000428"/>
        <obo:IAO_0000412>http://langual.org</obo:IAO_0000412>
        <oboInOwl:hasDbXref>http://www.langual.org/langual_thesaurus.asp?termid=P0111</oboInOwl:hasDbXref>
        <rdfs:label xml:lang="en">no nitrite/nitrate added claim or use</rdfs:label>
    </owl:Class>
    


    <!-- http://purl.obolibrary.org/obo/FOODON_03510112 -->


    <owl:Class rdf:about="http://purl.obolibrary.org/obo/FOODON_03510112">
        <rdfs:subClassOf rdf:resource="http://purl.obolibrary.org/obo/FOODON_03510106"/>
        <rdfs:subClassOf rdf:resource="http://purl.obolibrary.org/obo/FOODON_03510110"/>
        <obo:IAO_0000114 rdf:resource="http://purl.obolibrary.org/obo/IAO_0000428"/>
        <obo:IAO_0000412>http://langual.org</obo:IAO_0000412>
        <oboInOwl:hasDbXref>http://www.langual.org/langual_thesaurus.asp?termid=P0112</oboInOwl:hasDbXref>
        <rdfs:label xml:lang="en">no sulfite added claim or use</rdfs:label>
    </owl:Class>
    


    <!-- http://purl.obolibrary.org/obo/FOODON_03510113 -->


    <owl:Class rdf:about="http://purl.obolibrary.org/obo/FOODON_03510113">
        <rdfs:subClassOf rdf:resource="http://purl.obolibrary.org/obo/FOODON_03510106"/>
        <rdfs:subClassOf rdf:resource="http://purl.obolibrary.org/obo/FOODON_03510114"/>
        <obo:IAO_0000114 rdf:resource="http://purl.obolibrary.org/obo/IAO_0000428"/>
        <obo:IAO_0000412>http://langual.org</obo:IAO_0000412>
        <oboInOwl:hasDbXref>http://www.langual.org/langual_thesaurus.asp?termid=P0113</oboInOwl:hasDbXref>
        <rdfs:label xml:lang="en">no artificial preservatives claim or use</rdfs:label>
    </owl:Class>
    


    <!-- http://purl.obolibrary.org/obo/FOODON_03510114 -->


    <owl:Class rdf:about="http://purl.obolibrary.org/obo/FOODON_03510114">
        <rdfs:subClassOf rdf:resource="http://purl.obolibrary.org/obo/FOODON_03510110"/>
        <obo:IAO_0000114 rdf:resource="http://purl.obolibrary.org/obo/IAO_0000428"/>
        <obo:IAO_0000412>http://langual.org</obo:IAO_0000412>
        <oboInOwl:hasDbXref>http://www.langual.org/langual_thesaurus.asp?termid=P0114</oboInOwl:hasDbXref>
        <rdfs:label xml:lang="en">no preservatives claim or use</rdfs:label>
    </owl:Class>
    


    <!-- http://purl.obolibrary.org/obo/FOODON_03510115 -->


    <owl:Class rdf:about="http://purl.obolibrary.org/obo/FOODON_03510115">
        <rdfs:subClassOf rdf:resource="http://purl.obolibrary.org/obo/FOODON_03510023"/>
        <obo:IAO_0000114 rdf:resource="http://purl.obolibrary.org/obo/IAO_0000428"/>
        <obo:IAO_0000412>http://langual.org</obo:IAO_0000412>
        <oboInOwl:hasDbXref>http://www.langual.org/langual_thesaurus.asp?termid=P0115</oboInOwl:hasDbXref>
        <oboInOwl:hasSynonym xml:lang="en">other constituent- or ingredient-related claim or use</oboInOwl:hasSynonym>
        <rdfs:label xml:lang="en">other ingredient- or constituent-related claim or use</rdfs:label>
    </owl:Class>
    


    <!-- http://purl.obolibrary.org/obo/FOODON_03510116 -->


    <owl:Class rdf:about="http://purl.obolibrary.org/obo/FOODON_03510116">
        <rdfs:subClassOf rdf:resource="http://purl.obolibrary.org/obo/FOODON_03510115"/>
        <obo:IAO_0000114 rdf:resource="http://purl.obolibrary.org/obo/IAO_0000428"/>
        <obo:IAO_0000412>http://langual.org</obo:IAO_0000412>
        <oboInOwl:hasDbXref>http://www.langual.org/langual_thesaurus.asp?termid=P0116</oboInOwl:hasDbXref>
        <rdfs:label xml:lang="en">no msg added claim or use</rdfs:label>
    </owl:Class>
    


    <!-- http://purl.obolibrary.org/obo/FOODON_03510117 -->


    <owl:Class rdf:about="http://purl.obolibrary.org/obo/FOODON_03510117">
        <rdfs:subClassOf rdf:resource="http://purl.obolibrary.org/obo/FOODON_03510115"/>
        <obo:IAO_0000114 rdf:resource="http://purl.obolibrary.org/obo/IAO_0000428"/>
        <obo:IAO_0000412>http://langual.org</obo:IAO_0000412>
        <oboInOwl:hasDbXref>http://www.langual.org/langual_thesaurus.asp?termid=P0117</oboInOwl:hasDbXref>
        <oboInOwl:hasSynonym xml:lang="en">no caffeine claim or use</oboInOwl:hasSynonym>
        <rdfs:label xml:lang="en">caffeine free claim or use</rdfs:label>
    </owl:Class>
    


    <!-- http://purl.obolibrary.org/obo/FOODON_03510118 -->


    <owl:Class rdf:about="http://purl.obolibrary.org/obo/FOODON_03510118">
        <rdfs:subClassOf rdf:resource="http://purl.obolibrary.org/obo/FOODON_03510117"/>
        <obo:IAO_0000114 rdf:resource="http://purl.obolibrary.org/obo/IAO_0000428"/>
        <obo:IAO_0000412>http://langual.org</obo:IAO_0000412>
        <oboInOwl:hasDbXref>http://www.langual.org/langual_thesaurus.asp?termid=P0118</oboInOwl:hasDbXref>
        <oboInOwl:hasSynonym xml:lang="en">no caffeine added claim or use</oboInOwl:hasSynonym>
        <rdfs:label xml:lang="en">naturally caffeine free claim or use</rdfs:label>
    </owl:Class>
    


    <!-- http://purl.obolibrary.org/obo/FOODON_03510119 -->


    <owl:Class rdf:about="http://purl.obolibrary.org/obo/FOODON_03510119">
        <rdfs:subClassOf rdf:resource="http://purl.obolibrary.org/obo/FOODON_03510023"/>
        <obo:IAO_0000114 rdf:resource="http://purl.obolibrary.org/obo/IAO_0000428"/>
        <obo:IAO_0000412>http://langual.org</obo:IAO_0000412>
        <oboInOwl:hasDbXref>http://www.langual.org/langual_thesaurus.asp?termid=P0119</oboInOwl:hasDbXref>
        <rdfs:label xml:lang="en">processing-related claim or use</rdfs:label>
    </owl:Class>
    


    <!-- http://purl.obolibrary.org/obo/FOODON_03510120 -->


    <owl:Class rdf:about="http://purl.obolibrary.org/obo/FOODON_03510120">
        <rdfs:subClassOf rdf:resource="http://purl.obolibrary.org/obo/FOODON_03510059"/>
        <obo:IAO_0000114 rdf:resource="http://purl.obolibrary.org/obo/IAO_0000428"/>
        <obo:IAO_0000115 xml:lang="en">A raw food that has not been frozen, heat processed or otherwise preserved.</obo:IAO_0000115>
        <obo:IAO_0000412>http://langual.org</obo:IAO_0000412>
        <oboInOwl:hasDbXref>http://www.langual.org/langual_thesaurus.asp?termid=P0120</oboInOwl:hasDbXref>
        <oboInOwl:hasSynonym xml:lang="en">fresh, label claim</oboInOwl:hasSynonym>
        <rdfs:label xml:lang="en">&quot;fresh&quot; label claim</rdfs:label>
    </owl:Class>
    


    <!-- http://purl.obolibrary.org/obo/FOODON_03510121 -->


    <owl:Class rdf:about="http://purl.obolibrary.org/obo/FOODON_03510121">
        <rdfs:subClassOf rdf:resource="http://purl.obolibrary.org/obo/FOODON_03510119"/>
        <obo:IAO_0000114 rdf:resource="http://purl.obolibrary.org/obo/IAO_0000428"/>
        <obo:IAO_0000412>http://langual.org</obo:IAO_0000412>
        <oboInOwl:hasDbXref>http://www.langual.org/langual_thesaurus.asp?termid=P0121</oboInOwl:hasDbXref>
        <rdfs:label xml:lang="en">not pasteurized claim or use</rdfs:label>
    </owl:Class>
    


    <!-- http://purl.obolibrary.org/obo/FOODON_03510122 -->


    <owl:Class rdf:about="http://purl.obolibrary.org/obo/FOODON_03510122">
        <rdfs:subClassOf rdf:resource="http://purl.obolibrary.org/obo/FOODON_03510119"/>
        <obo:IAO_0000114 rdf:resource="http://purl.obolibrary.org/obo/IAO_0000428"/>
        <obo:IAO_0000412>http://langual.org</obo:IAO_0000412>
        <oboInOwl:hasDbXref>http://www.langual.org/langual_thesaurus.asp?termid=P0122</oboInOwl:hasDbXref>
        <oboInOwl:hasSynonym xml:lang="en">unrefined or unpurified claim or use</oboInOwl:hasSynonym>
        <rdfs:label xml:lang="en">unpurified or unrefined claim or use</rdfs:label>
    </owl:Class>
    


    <!-- http://purl.obolibrary.org/obo/FOODON_03510123 -->


    <owl:Class rdf:about="http://purl.obolibrary.org/obo/FOODON_03510123">
        <rdfs:subClassOf rdf:resource="http://purl.obolibrary.org/obo/FOODON_03510119"/>
        <obo:IAO_0000114 rdf:resource="http://purl.obolibrary.org/obo/IAO_0000428"/>
        <obo:IAO_0000412>http://langual.org</obo:IAO_0000412>
        <oboInOwl:hasDbXref>http://www.langual.org/langual_thesaurus.asp?termid=P0123</oboInOwl:hasDbXref>
        <rdfs:label xml:lang="en">unbleached claim or use</rdfs:label>
    </owl:Class>
    


    <!-- http://purl.obolibrary.org/obo/FOODON_03510124 -->


    <owl:Class rdf:about="http://purl.obolibrary.org/obo/FOODON_03510124">
        <rdfs:subClassOf rdf:resource="http://purl.obolibrary.org/obo/FOODON_03510023"/>
        <obo:IAO_0000114 rdf:resource="http://purl.obolibrary.org/obo/IAO_0000428"/>
        <obo:IAO_0000115 xml:lang="en">Health claim means any claim made on the label or in labeling of a food, including a dietary supplement, that expressly or by implication, including &quot;third party&quot; references, written statements (e.g., a brand name including a term such as &quot;heart&quot;), symbols (e.g., a heart symbol), or vignettes, characterizes the relationship of any substance to a disease or health-related condition. See also 21 CFR 101.14  [http://www.accessdata.fda.gov/scripts/cdrh/cfdocs/cfcfr/CFRSearch.cfm?fr=101.14].

A claim is a health claim if in the naming of the substance or category of substances, there is a description or indication of a functionality or an implied effect on health; examples: &quot;contains antioxidants&quot; (the function is an antioxidant effect); &quot;containsprobiotics/prebiotics&quot; (the reference to probiotic/prebiotic implies a health benefit). Equally, claims which refer to an indication of a functionality in the description of a nutrient or a substance (for instance as an adjective to the substance) should also beclassified as a health claim; examples: &quot;with prebiotic fibres&quot; or &quot;contains prebiotic fibres&quot;.

In Europe, a health claim is any statement about a relationship between food and health [http://ec.europa.eu/food/food/labellingnutrition/claims/health_claims_en.htm], and only authorized health claims are legal [see http://ec.europa.eu/food/food/labellingnutrition/claims/community_register/health_claims_en.htm].
COMMISSION REGULATION (EU) No 432/2012 of 16 May 2012 establishes a list of permitted health claims made on foods, other than those referring to the reduction of disease risk and to children&quot;s development and health [http://eur-lex.europa.eu/LexUriServ/LexUriServ.do?uri=OJ:L:2012:136:0001:0040:en:PDF]</obo:IAO_0000115>
        <obo:IAO_0000412>http://langual.org</obo:IAO_0000412>
        <oboInOwl:hasDbXref>http://www.langual.org/langual_thesaurus.asp?termid=P0124</oboInOwl:hasDbXref>
        <rdfs:comment xml:lang="en">LanguaL curation note: Used for any claim that states, suggests or implies that a relationship exists between a food category, a food or one of its components and health.</rdfs:comment>
        <rdfs:label xml:lang="en">health-related claim or use</rdfs:label>
    </owl:Class>
    


    <!-- http://purl.obolibrary.org/obo/FOODON_03510125 -->


    <owl:Class rdf:about="http://purl.obolibrary.org/obo/FOODON_03510125">
        <rdfs:subClassOf rdf:resource="http://purl.obolibrary.org/obo/FOODON_03510124"/>
        <obo:IAO_0000114 rdf:resource="http://purl.obolibrary.org/obo/IAO_0000428"/>
        <obo:IAO_0000412>http://langual.org</obo:IAO_0000412>
        <oboInOwl:hasDbXref>http://www.langual.org/langual_thesaurus.asp?termid=P0125</oboInOwl:hasDbXref>
        <oboInOwl:hasSynonym xml:lang="en">does not promote tooth decay claim or use</oboInOwl:hasSynonym>
        <rdfs:label xml:lang="en">tooth decay-related claim or use</rdfs:label>
    </owl:Class>
    


    <!-- http://purl.obolibrary.org/obo/FOODON_03510126 -->


    <owl:Class rdf:about="http://purl.obolibrary.org/obo/FOODON_03510126">
        <rdfs:subClassOf rdf:resource="http://purl.obolibrary.org/obo/FOODON_03510023"/>
        <obo:IAO_0000114 rdf:resource="http://purl.obolibrary.org/obo/IAO_0000428"/>
        <obo:IAO_0000412>http://langual.org</obo:IAO_0000412>
        <oboInOwl:hasDbXref>http://www.langual.org/langual_thesaurus.asp?termid=P0126</oboInOwl:hasDbXref>
        <oboInOwl:hasSynonym xml:lang="en">custom- or religion-related claim or use</oboInOwl:hasSynonym>
        <rdfs:label xml:lang="en">religion- or customs-related claim or use</rdfs:label>
    </owl:Class>
    


    <!-- http://purl.obolibrary.org/obo/FOODON_03510127 -->


    <owl:Class rdf:about="http://purl.obolibrary.org/obo/FOODON_03510127">
        <rdfs:subClassOf rdf:resource="http://purl.obolibrary.org/obo/FOODON_03510126"/>
        <obo:IAO_0000114 rdf:resource="http://purl.obolibrary.org/obo/IAO_0000428"/>
        <obo:IAO_0000412>http://langual.org</obo:IAO_0000412>
        <oboInOwl:hasDbXref>http://www.langual.org/langual_thesaurus.asp?termid=P0127</oboInOwl:hasDbXref>
        <rdfs:label xml:lang="en">kosher claim or use</rdfs:label>
    </owl:Class>
    


    <!-- http://purl.obolibrary.org/obo/FOODON_03510128 -->


    <owl:Class rdf:about="http://purl.obolibrary.org/obo/FOODON_03510128">
        <rdfs:subClassOf rdf:resource="http://purl.obolibrary.org/obo/FOODON_03510023"/>
        <obo:IAO_0000114 rdf:resource="http://purl.obolibrary.org/obo/IAO_0000428"/>
        <obo:IAO_0000115 xml:lang="en">USA:
The 1990 Farm Act specifies that a food labeled &apos;organic&apos; must meet four requirements:  1) the food must be raised by specified methods to replenish and maintain the fertility of the soil; 2) the food must be certified as having been produced with a nationally approved list of materials and practices; 3) to be eligible for certification at least three years must have elapsed between the first organic harvest and first use of nationally approved materials on land and crops;and 4) organic foods must meet all local, state and federal regulations governing the quality and safety of the food supply.

Europe:
Foods produced in accordance with Council Regulation (EC) No 834/2007
of 28 June 2007 on organic production and labelling of organic products and repealing Regulation (EEC) No 2092/91. [http://eur-lex.europa.eu/LexUriServ/LexUriServ.do?uri=OJ:L:2007:189:0001:0023:EN:PDF]</obo:IAO_0000115>
        <obo:IAO_0000412>http://langual.org</obo:IAO_0000412>
        <oboInOwl:hasDbXref>http://www.langual.org/langual_thesaurus.asp?termid=P0128</oboInOwl:hasDbXref>
        <oboInOwl:hasSynonym xml:lang="en">no pesticides claim or use</oboInOwl:hasSynonym>
        <oboInOwl:hasSynonym xml:lang="en">organically grown label claim</oboInOwl:hasSynonym>
        <rdfs:label xml:lang="en">organic food claim or use</rdfs:label>
    </owl:Class>
    


    <!-- http://purl.obolibrary.org/obo/FOODON_03510129 -->


    <owl:Class rdf:about="http://purl.obolibrary.org/obo/FOODON_03510129">
        <rdfs:subClassOf rdf:resource="http://purl.obolibrary.org/obo/FOODON_03510059"/>
        <obo:IAO_0000114 rdf:resource="http://purl.obolibrary.org/obo/IAO_0000428"/>
        <obo:IAO_0000115 xml:lang="en">Considerations include amounts that are &apos;nutritionally trivial&apos; and amounts that can be declared as zero on the nutrition label. An additional criterion based on amount per weight (e.g., per 100 grams) is not considered necessary because the amount of nutrient in a &apos;free&apos; food is so low that even frequent and repeated consumption is unlikely to have physiological consequences. (U.S. proposed)</obo:IAO_0000115>
        <obo:IAO_0000412>http://langual.org</obo:IAO_0000412>
        <oboInOwl:hasDbXref>http://www.langual.org/langual_thesaurus.asp?termid=P0129</oboInOwl:hasDbXref>
        <oboInOwl:hasSynonym xml:lang="en">free, label claim</oboInOwl:hasSynonym>
        <rdfs:label xml:lang="en">&quot;free&quot; label claim</rdfs:label>
    </owl:Class>
    


    <!-- http://purl.obolibrary.org/obo/FOODON_03510130 -->


    <owl:Class rdf:about="http://purl.obolibrary.org/obo/FOODON_03510130">
        <rdfs:subClassOf rdf:resource="http://purl.obolibrary.org/obo/FOODON_03510059"/>
        <obo:IAO_0000114 rdf:resource="http://purl.obolibrary.org/obo/IAO_0000428"/>
        <obo:IAO_0000115 xml:lang="en">An amount customarily consumed contains 20% or more of the daily nutritional value to describe protein, vitamins, minerals, dietary fiber, or potassium. May be used on meals or main dishes to indicate that product contains a food that meets the definition.</obo:IAO_0000115>
        <obo:IAO_0000412>http://langual.org</obo:IAO_0000412>
        <oboInOwl:hasDbXref>http://www.langual.org/langual_thesaurus.asp?termid=P0130</oboInOwl:hasDbXref>
        <oboInOwl:hasSynonym xml:lang="en">excellent source of label claim</oboInOwl:hasSynonym>
        <oboInOwl:hasSynonym xml:lang="en">high, label claim</oboInOwl:hasSynonym>
        <oboInOwl:hasSynonym xml:lang="en">rich in label claim</oboInOwl:hasSynonym>
        <rdfs:label xml:lang="en">&quot;high&quot; label claim</rdfs:label>
    </owl:Class>
    


    <!-- http://purl.obolibrary.org/obo/FOODON_03510131 -->


    <owl:Class rdf:about="http://purl.obolibrary.org/obo/FOODON_03510131">
        <rdfs:subClassOf rdf:resource="http://purl.obolibrary.org/obo/FOODON_03510059"/>
        <obo:IAO_0000114 rdf:resource="http://purl.obolibrary.org/obo/IAO_0000428"/>
        <obo:IAO_0000412>http://langual.org</obo:IAO_0000412>
        <oboInOwl:hasDbXref>http://www.langual.org/langual_thesaurus.asp?termid=P0131</oboInOwl:hasDbXref>
        <oboInOwl:hasSynonym xml:lang="en">less, label claim</oboInOwl:hasSynonym>
        <rdfs:comment xml:lang="en">LanguaL curation note: Used on label comparison statements to describe foods having 25% or greater reductions in a nutrient. (U.S. proposed)</rdfs:comment>
        <rdfs:label xml:lang="en">&quot;less&quot; label claim</rdfs:label>
    </owl:Class>
    


    <!-- http://purl.obolibrary.org/obo/FOODON_03510132 -->


    <owl:Class rdf:about="http://purl.obolibrary.org/obo/FOODON_03510132">
        <rdfs:subClassOf rdf:resource="http://purl.obolibrary.org/obo/FOODON_03510059"/>
        <obo:IAO_0000114 rdf:resource="http://purl.obolibrary.org/obo/IAO_0000428"/>
        <obo:IAO_0000115 xml:lang="en">A claim stating that a product is &quot;light&quot; or &quot;lite&quot;, and any claim likely to have the same meaning for the consumer, shall follow the same conditions as those set for the term &quot;reduced&quot;, see *REDUCED {NAME OF NUTRIENT} NUTRITION CLAIM [P0132]*; the claim shall also be accompanied by an indication of the characteristic(s) which make(s) the food &quot;light&quot; or &quot;lite&quot; [REGULATION (EC) No 1924/2006 Corrigendum 2007-01-18].

Used for foods that have 33.3% fewer calories than a comparable product and a minimum reduction of more than 40 calories per serving. Any other use of &apos;light&apos; must specify whether it refers to the look, taste or smell; for example, &apos;light in color&apos;. (U.S. FDA proposed)</obo:IAO_0000115>
        <obo:IAO_0000412>http://langual.org</obo:IAO_0000412>
        <oboInOwl:hasDbXref>http://www.langual.org/langual_thesaurus.asp?termid=P0132</oboInOwl:hasDbXref>
        <oboInOwl:hasSynonym xml:lang="en">light, label claim</oboInOwl:hasSynonym>
        <rdfs:label xml:lang="en">&quot;light&quot; label claim</rdfs:label>
    </owl:Class>
    


    <!-- http://purl.obolibrary.org/obo/FOODON_03510133 -->


    <owl:Class rdf:about="http://purl.obolibrary.org/obo/FOODON_03510133">
        <rdfs:subClassOf rdf:resource="http://purl.obolibrary.org/obo/FOODON_03510059"/>
        <obo:IAO_0000114 rdf:resource="http://purl.obolibrary.org/obo/IAO_0000428"/>
        <obo:IAO_0000412>http://langual.org</obo:IAO_0000412>
        <oboInOwl:hasDbXref>http://www.langual.org/langual_thesaurus.asp?termid=P0133</oboInOwl:hasDbXref>
        <oboInOwl:hasSynonym xml:lang="en">more, label claim</oboInOwl:hasSynonym>
        <rdfs:comment xml:lang="en">LanguaL curation note: Used in label comparison statement when a food contains at least 10% more of the daily nutritional value per amount customarily consumed.</rdfs:comment>
        <rdfs:label xml:lang="en">&quot;more&quot; label claim</rdfs:label>
    </owl:Class>
    


    <!-- http://purl.obolibrary.org/obo/FOODON_03510134 -->


    <owl:Class rdf:about="http://purl.obolibrary.org/obo/FOODON_03510134">
        <rdfs:subClassOf rdf:resource="http://purl.obolibrary.org/obo/FOODON_03510059"/>
        <obo:IAO_0000114 rdf:resource="http://purl.obolibrary.org/obo/IAO_0000428"/>
        <obo:IAO_0000412>http://langual.org</obo:IAO_0000412>
        <oboInOwl:hasDbXref>http://www.langual.org/langual_thesaurus.asp?termid=P0134</oboInOwl:hasDbXref>
        <oboInOwl:hasSynonym xml:lang="en">contains label claim</oboInOwl:hasSynonym>
        <oboInOwl:hasSynonym xml:lang="en">contains, label claim</oboInOwl:hasSynonym>
        <oboInOwl:hasSynonym xml:lang="en">good source of label claim</oboInOwl:hasSynonym>
        <oboInOwl:hasSynonym xml:lang="en">good source of, label claim</oboInOwl:hasSynonym>
        <oboInOwl:hasSynonym xml:lang="en">provides label claim</oboInOwl:hasSynonym>
        <oboInOwl:hasSynonym xml:lang="en">provides, label claim</oboInOwl:hasSynonym>
        <oboInOwl:hasSynonym xml:lang="en">source of, label claim</oboInOwl:hasSynonym>
        <rdfs:comment xml:lang="en">LanguaL curation note: The amount customarily consumed contains 10% to 19% of the daily nutritional value. May be used on meals or main dishes to indicate that product contains a food that meets the definition.</rdfs:comment>
        <rdfs:label xml:lang="en">&quot;source of&quot; label claim</rdfs:label>
    </owl:Class>
    


    <!-- http://purl.obolibrary.org/obo/FOODON_03510135 -->


    <owl:Class rdf:about="http://purl.obolibrary.org/obo/FOODON_03510135">
        <rdfs:subClassOf rdf:resource="http://purl.obolibrary.org/obo/FOODON_03510127"/>
        <obo:IAO_0000114 rdf:resource="http://purl.obolibrary.org/obo/IAO_0000428"/>
        <obo:IAO_0000412>http://langual.org</obo:IAO_0000412>
        <oboInOwl:hasDbXref>http://www.langual.org/langual_thesaurus.asp?termid=P0135</oboInOwl:hasDbXref>
        <rdfs:label xml:lang="en">kosher for passover claim or use</rdfs:label>
    </owl:Class>
    


    <!-- http://purl.obolibrary.org/obo/FOODON_03510149 -->


    <owl:Class rdf:about="http://purl.obolibrary.org/obo/FOODON_03510149">
        <rdfs:subClassOf rdf:resource="http://purl.obolibrary.org/obo/FOODON_03510041"/>
        <obo:IAO_0000114 rdf:resource="http://purl.obolibrary.org/obo/IAO_0000428"/>
        <obo:IAO_0000412>http://langual.org</obo:IAO_0000412>
        <oboInOwl:hasDbXref>http://www.langual.org/langual_thesaurus.asp?termid=P0149</oboInOwl:hasDbXref>
        <oboInOwl:hasSynonym xml:lang="en">reduced or no cholesterol claim or use</oboInOwl:hasSynonym>
        <rdfs:label xml:lang="en">no or reduced cholesterol claim or use</rdfs:label>
    </owl:Class>
    


    <!-- http://purl.obolibrary.org/obo/FOODON_03510150 -->


    <owl:Class rdf:about="http://purl.obolibrary.org/obo/FOODON_03510150">
        <rdfs:subClassOf rdf:resource="http://purl.obolibrary.org/obo/FOODON_03510039"/>
        <obo:IAO_0000114 rdf:resource="http://purl.obolibrary.org/obo/IAO_0000428"/>
        <obo:IAO_0000412>http://langual.org</obo:IAO_0000412>
        <oboInOwl:hasDbXref>http://www.langual.org/langual_thesaurus.asp?termid=P0150</oboInOwl:hasDbXref>
        <oboInOwl:hasSynonym xml:lang="en">percent fat free claim or use</oboInOwl:hasSynonym>
        <rdfs:comment xml:lang="en">LanguaL curation note: Used only in describing foods that qualify as low fat. (U.S. proposed).

The claim is not allowed in EU [REGULATION (EC) No 1924/2006 Corrigendum].</rdfs:comment>
        <rdfs:label xml:lang="en">(percent) fat free claim or use</rdfs:label>
    </owl:Class>
    


    <!-- http://purl.obolibrary.org/obo/FOODON_03510152 -->


    <owl:Class rdf:about="http://purl.obolibrary.org/obo/FOODON_03510152">
        <rdfs:subClassOf rdf:resource="http://purl.obolibrary.org/obo/FOODON_03510035"/>
        <obo:IAO_0000114 rdf:resource="http://purl.obolibrary.org/obo/IAO_0000428"/>
        <obo:IAO_0000115 xml:lang="en">Food having less than 5 miligrams sodium per amount customarily consumed (or for meals and main dishes, less than 5 milligrams sodium per labeled serving). Such food must contain no ingredient that is sodium chloride or generally understood to contain sodium except where the ingredient listed is footnoted &apos;*adds a trivial amount of sodium&apos;.</obo:IAO_0000115>
        <obo:IAO_0000412>http://langual.org</obo:IAO_0000412>
        <oboInOwl:hasDbXref>http://www.langual.org/langual_thesaurus.asp?termid=P0152</oboInOwl:hasDbXref>
        <rdfs:label xml:lang="en">sodium free claim or use</rdfs:label>
    </owl:Class>
    


    <!-- http://purl.obolibrary.org/obo/FOODON_03510153 -->


    <owl:Class rdf:about="http://purl.obolibrary.org/obo/FOODON_03510153">
        <rdfs:subClassOf rdf:resource="http://purl.obolibrary.org/obo/FOODON_03510036"/>
        <obo:IAO_0000114 rdf:resource="http://purl.obolibrary.org/obo/IAO_0000428"/>
        <obo:IAO_0000115 xml:lang="en">Food having 35 milligrams or less sodium per amount customarily consumed (and per 50 grams of food if the amount customarily consumed is small). Meals and main dishes contain 35 milligrams or less sodium per 100 grams food.</obo:IAO_0000115>
        <obo:IAO_0000412>http://langual.org</obo:IAO_0000412>
        <oboInOwl:hasDbXref>http://www.langual.org/langual_thesaurus.asp?termid=P0153</oboInOwl:hasDbXref>
        <rdfs:label xml:lang="en">very low sodium claim or use</rdfs:label>
    </owl:Class>
    


    <!-- http://purl.obolibrary.org/obo/FOODON_03510154 -->


    <owl:Class rdf:about="http://purl.obolibrary.org/obo/FOODON_03510154">
        <rdfs:subClassOf rdf:resource="http://purl.obolibrary.org/obo/FOODON_03510037"/>
        <obo:IAO_0000114 rdf:resource="http://purl.obolibrary.org/obo/IAO_0000428"/>
        <obo:IAO_0000115 xml:lang="en">Food containing at least 25% less sodium per amount customarily consumed than the sodium content of a comparable food product. The comparable food may not be &apos;low sodium&apos;.</obo:IAO_0000115>
        <obo:IAO_0000412>http://langual.org</obo:IAO_0000412>
        <oboInOwl:hasDbXref>http://www.langual.org/langual_thesaurus.asp?termid=P0154</oboInOwl:hasDbXref>
        <rdfs:label xml:lang="en">reduced sodium claim or use</rdfs:label>
    </owl:Class>
    


    <!-- http://purl.obolibrary.org/obo/FOODON_03510159 -->


    <owl:Class rdf:about="http://purl.obolibrary.org/obo/FOODON_03510159">
        <rdfs:subClassOf rdf:resource="http://purl.obolibrary.org/obo/FOODON_03510023"/>
        <obo:IAO_0000114 rdf:resource="http://purl.obolibrary.org/obo/IAO_0000428"/>
        <obo:IAO_0000412>http://langual.org</obo:IAO_0000412>
        <oboInOwl:hasDbXref>http://www.langual.org/langual_thesaurus.asp?termid=P0159</oboInOwl:hasDbXref>
        <rdfs:label xml:lang="en">other special claim or use</rdfs:label>
    </owl:Class>
    


    <!-- http://purl.obolibrary.org/obo/FOODON_03510161 -->


    <owl:Class rdf:about="http://purl.obolibrary.org/obo/FOODON_03510161">
        <rdfs:subClassOf rdf:resource="http://purl.obolibrary.org/obo/FOODON_03510059"/>
        <obo:IAO_0000114 rdf:resource="http://purl.obolibrary.org/obo/IAO_0000428"/>
        <obo:IAO_0000412>http://langual.org</obo:IAO_0000412>
        <oboInOwl:hasDbXref>http://www.langual.org/langual_thesaurus.asp?termid=P0161</oboInOwl:hasDbXref>
        <rdfs:comment xml:lang="en">LanguaL curation note: Use when the &apos;claim or use&apos; index term is found in the name of the food appearing on the label (e.g., &apos;unbleached flour&apos; indexed by *UNBLEACHED CLAIM OR USE*).</rdfs:comment>
        <rdfs:label xml:lang="en">label claim in food name</rdfs:label>
    </owl:Class>
    


    <!-- http://purl.obolibrary.org/obo/FOODON_03510162 -->


    <owl:Class rdf:about="http://purl.obolibrary.org/obo/FOODON_03510162">
        <rdfs:subClassOf rdf:resource="http://purl.obolibrary.org/obo/FOODON_03510059"/>
        <obo:IAO_0000114 rdf:resource="http://purl.obolibrary.org/obo/IAO_0000428"/>
        <obo:IAO_0000412>http://langual.org</obo:IAO_0000412>
        <oboInOwl:hasDbXref>http://www.langual.org/langual_thesaurus.asp?termid=P0162</oboInOwl:hasDbXref>
        <rdfs:comment xml:lang="en">LanguaL curation note: Use when the &apos;claim or use&apos; index term appears on the food label but not in the food name (e.g., a label for bran cereal saying &apos;high in fiber&apos; indexed by *HIGH FIBER FOOD*).</rdfs:comment>
        <rdfs:label xml:lang="en">label claim separate from food name</rdfs:label>
    </owl:Class>
    


    <!-- http://purl.obolibrary.org/obo/FOODON_03510167 -->


    <owl:Class rdf:about="http://purl.obolibrary.org/obo/FOODON_03510167">
        <rdfs:subClassOf rdf:resource="http://purl.obolibrary.org/obo/FOODON_03510119"/>
        <obo:IAO_0000114 rdf:resource="http://purl.obolibrary.org/obo/IAO_0000428"/>
        <obo:IAO_0000412>http://langual.org</obo:IAO_0000412>
        <oboInOwl:hasDbXref>http://www.langual.org/langual_thesaurus.asp?termid=P0167</oboInOwl:hasDbXref>
        <rdfs:label xml:lang="en">no water added claim or use</rdfs:label>
    </owl:Class>
    


    <!-- http://purl.obolibrary.org/obo/FOODON_03510168 -->


    <owl:Class rdf:about="http://purl.obolibrary.org/obo/FOODON_03510168">
        <rdfs:subClassOf rdf:resource="http://purl.obolibrary.org/obo/FOODON_03510126"/>
        <obo:IAO_0000114 rdf:resource="http://purl.obolibrary.org/obo/IAO_0000428"/>
        <obo:IAO_0000412>http://langual.org</obo:IAO_0000412>
        <oboInOwl:hasDbXref>http://www.langual.org/langual_thesaurus.asp?termid=P0168</oboInOwl:hasDbXref>
        <oboInOwl:hasSynonym xml:lang="en">parve claim or use</oboInOwl:hasSynonym>
        <rdfs:label xml:lang="en">pareve claim or use</rdfs:label>
    </owl:Class>
    


    <!-- http://purl.obolibrary.org/obo/FOODON_03510169 -->


    <owl:Class rdf:about="http://purl.obolibrary.org/obo/FOODON_03510169">
        <rdfs:subClassOf rdf:resource="http://purl.obolibrary.org/obo/FOODON_03510099"/>
        <obo:IAO_0000114 rdf:resource="http://purl.obolibrary.org/obo/IAO_0000428"/>
        <obo:IAO_0000412>http://langual.org</obo:IAO_0000412>
        <oboInOwl:hasDbXref>http://www.langual.org/langual_thesaurus.asp?termid=P0169</oboInOwl:hasDbXref>
        <rdfs:label xml:lang="en">noncarbonated claim or use</rdfs:label>
    </owl:Class>
    


    <!-- http://purl.obolibrary.org/obo/FOODON_03510170 -->


    <owl:Class rdf:about="http://purl.obolibrary.org/obo/FOODON_03510170">
        <rdfs:subClassOf rdf:resource="http://purl.obolibrary.org/obo/FOODON_03510090"/>
        <obo:IAO_0000114 rdf:resource="http://purl.obolibrary.org/obo/IAO_0000428"/>
        <obo:IAO_0000412>http://langual.org</obo:IAO_0000412>
        <oboInOwl:hasDbXref>http://www.langual.org/langual_thesaurus.asp?termid=P0170</oboInOwl:hasDbXref>
        <rdfs:label xml:lang="en">lactose reduced food</rdfs:label>
    </owl:Class>
    


    <!-- http://purl.obolibrary.org/obo/FOODON_03510171 -->


    <owl:Class rdf:about="http://purl.obolibrary.org/obo/FOODON_03510171">
        <rdfs:subClassOf rdf:resource="http://purl.obolibrary.org/obo/FOODON_03510170"/>
        <obo:IAO_0000114 rdf:resource="http://purl.obolibrary.org/obo/IAO_0000428"/>
        <obo:IAO_0000412>http://langual.org</obo:IAO_0000412>
        <oboInOwl:hasDbXref>http://www.langual.org/langual_thesaurus.asp?termid=P0171</oboInOwl:hasDbXref>
        <rdfs:label xml:lang="en">lactose free food</rdfs:label>
    </owl:Class>
    


    <!-- http://purl.obolibrary.org/obo/FOODON_03510172 -->


    <owl:Class rdf:about="http://purl.obolibrary.org/obo/FOODON_03510172">
        <rdfs:subClassOf rdf:resource="http://purl.obolibrary.org/obo/FOODON_03510095"/>
        <obo:IAO_0000114 rdf:resource="http://purl.obolibrary.org/obo/IAO_0000428"/>
        <obo:IAO_0000412>http://langual.org</obo:IAO_0000412>
        <oboInOwl:hasDbXref>http://www.langual.org/langual_thesaurus.asp?termid=P0172</oboInOwl:hasDbXref>
        <rdfs:label xml:lang="en">unenriched claim or use</rdfs:label>
    </owl:Class>
    


    <!-- http://purl.obolibrary.org/obo/FOODON_03510173 -->


    <owl:Class rdf:about="http://purl.obolibrary.org/obo/FOODON_03510173">
        <rdfs:subClassOf rdf:resource="http://purl.obolibrary.org/obo/FOODON_03510095"/>
        <obo:IAO_0000114 rdf:resource="http://purl.obolibrary.org/obo/IAO_0000428"/>
        <obo:IAO_0000412>http://langual.org</obo:IAO_0000412>
        <oboInOwl:hasDbXref>http://www.langual.org/langual_thesaurus.asp?termid=P0173</oboInOwl:hasDbXref>
        <oboInOwl:hasSynonym xml:lang="en">no mineral or vitamin added claim or use</oboInOwl:hasSynonym>
        <rdfs:label xml:lang="en">no vitamin or mineral added claim or use</rdfs:label>
    </owl:Class>
    


    <!-- http://purl.obolibrary.org/obo/FOODON_03510174 -->


    <owl:Class rdf:about="http://purl.obolibrary.org/obo/FOODON_03510174">
        <rdfs:subClassOf rdf:resource="http://purl.obolibrary.org/obo/FOODON_03510115"/>
        <obo:IAO_0000114 rdf:resource="http://purl.obolibrary.org/obo/IAO_0000428"/>
        <obo:IAO_0000412>http://langual.org</obo:IAO_0000412>
        <oboInOwl:hasDbXref>http://www.langual.org/langual_thesaurus.asp?termid=P0174</oboInOwl:hasDbXref>
        <rdfs:label xml:lang="en">gluten free claim or use</rdfs:label>
    </owl:Class>
    


    <!-- http://purl.obolibrary.org/obo/FOODON_03510175 -->


    <owl:Class rdf:about="http://purl.obolibrary.org/obo/FOODON_03510175">
        <rdfs:subClassOf rdf:resource="http://purl.obolibrary.org/obo/FOODON_03510115"/>
        <obo:IAO_0000114 rdf:resource="http://purl.obolibrary.org/obo/IAO_0000428"/>
        <obo:IAO_0000412>http://langual.org</obo:IAO_0000412>
        <oboInOwl:hasDbXref>http://www.langual.org/langual_thesaurus.asp?termid=P0175</oboInOwl:hasDbXref>
        <rdfs:label xml:lang="en">egg free claim or use</rdfs:label>
    </owl:Class>
    


    <!-- http://purl.obolibrary.org/obo/FOODON_03510176 -->


    <owl:Class rdf:about="http://purl.obolibrary.org/obo/FOODON_03510176">
        <rdfs:subClassOf rdf:resource="http://purl.obolibrary.org/obo/FOODON_03510115"/>
        <obo:IAO_0000114 rdf:resource="http://purl.obolibrary.org/obo/IAO_0000428"/>
        <obo:IAO_0000412>http://langual.org</obo:IAO_0000412>
        <oboInOwl:hasDbXref>http://www.langual.org/langual_thesaurus.asp?termid=P0176</oboInOwl:hasDbXref>
        <rdfs:label xml:lang="en">alcohol free claim or use</rdfs:label>
    </owl:Class>
    


    <!-- http://purl.obolibrary.org/obo/FOODON_03510177 -->


    <owl:Class rdf:about="http://purl.obolibrary.org/obo/FOODON_03510177">
        <rdfs:subClassOf rdf:resource="http://purl.obolibrary.org/obo/FOODON_03510127"/>
        <obo:IAO_0000114 rdf:resource="http://purl.obolibrary.org/obo/IAO_0000428"/>
        <obo:IAO_0000412>http://langual.org</obo:IAO_0000412>
        <oboInOwl:hasDbXref>http://www.langual.org/langual_thesaurus.asp?termid=P0177</oboInOwl:hasDbXref>
        <rdfs:comment xml:lang="en">LanguaL curation note: Used to indicate a food is kosher but may contain dairy ingredients [CFSAN thesaurus].</rdfs:comment>
        <rdfs:label xml:lang="en">kosher milchlig claim or use</rdfs:label>
    </owl:Class>
    


    <!-- http://purl.obolibrary.org/obo/FOODON_03510178 -->


    <owl:Class rdf:about="http://purl.obolibrary.org/obo/FOODON_03510178">
        <rdfs:subClassOf rdf:resource="http://purl.obolibrary.org/obo/FOODON_03510059"/>
        <obo:IAO_0000114 rdf:resource="http://purl.obolibrary.org/obo/IAO_0000428"/>
        <obo:IAO_0000115 xml:lang="en">The food was quickly frozen while still fresh.</obo:IAO_0000115>
        <obo:IAO_0000412>http://langual.org</obo:IAO_0000412>
        <oboInOwl:hasDbXref>http://www.langual.org/langual_thesaurus.asp?termid=P0178</oboInOwl:hasDbXref>
        <oboInOwl:hasSynonym xml:lang="en">fresh frozen, label claim</oboInOwl:hasSynonym>
        <rdfs:label xml:lang="en">&quot;fresh frozen&quot; label claim</rdfs:label>
    </owl:Class>
    


    <!-- http://purl.obolibrary.org/obo/FOODON_03510179 -->


    <owl:Class rdf:about="http://purl.obolibrary.org/obo/FOODON_03510179">
        <rdfs:subClassOf rdf:resource="http://purl.obolibrary.org/obo/FOODON_03510071"/>
        <obo:IAO_0000114 rdf:resource="http://purl.obolibrary.org/obo/IAO_0000428"/>
        <obo:IAO_0000115 xml:lang="en">A claim that a food does not contain saturated fat, and any claim likely to have the same meaning for the consumer, may only be made where the sum of saturated fat and trans-fatty acids does not exceed 0,1 g of saturated fat per 100 g or 100 ml [REGULATION (EC) No 1924/2006 Corrigendum 2007-01-18].

Food having less than 0.5 grams saturated fat per amount customarily consumed (or for meals and main dishes, less than 0.5 grams saturated fat per labeled serving). Trans fatty acids are not more than 1% of total fat. Such foods contain no ingredient that is understood to contain saturated fat except where the ingredient listed has been footnoted &apos;*adds a trivial amount of saturated fat&apos; [US FDA].</obo:IAO_0000115>
        <obo:IAO_0000412>http://langual.org</obo:IAO_0000412>
        <oboInOwl:hasDbXref>http://www.langual.org/langual_thesaurus.asp?termid=P0179</oboInOwl:hasDbXref>
        <rdfs:label xml:lang="en">saturated fat free food</rdfs:label>
    </owl:Class>
    


    <!-- http://purl.obolibrary.org/obo/FOODON_03510180 -->


    <owl:Class rdf:about="http://purl.obolibrary.org/obo/FOODON_03510180">
        <rdfs:subClassOf rdf:resource="http://purl.obolibrary.org/obo/FOODON_03510071"/>
        <obo:IAO_0000114 rdf:resource="http://purl.obolibrary.org/obo/IAO_0000428"/>
        <obo:IAO_0000115 xml:lang="en">Food containing at least 25% less saturated fat per amount customarily consumed than the saturated fat content of a comparable food product. The comparable food product may not be &apos;low saturated fat&apos;.</obo:IAO_0000115>
        <obo:IAO_0000412>http://langual.org</obo:IAO_0000412>
        <oboInOwl:hasDbXref>http://www.langual.org/langual_thesaurus.asp?termid=P0180</oboInOwl:hasDbXref>
        <rdfs:label xml:lang="en">reduced saturated fat food</rdfs:label>
    </owl:Class>
    


    <!-- http://purl.obolibrary.org/obo/FOODON_03510181 -->


    <owl:Class rdf:about="http://purl.obolibrary.org/obo/FOODON_03510181">
        <rdfs:subClassOf rdf:resource="http://purl.obolibrary.org/obo/FOODON_03510090"/>
        <obo:IAO_0000114 rdf:resource="http://purl.obolibrary.org/obo/IAO_0000428"/>
        <obo:IAO_0000115 xml:lang="en">Food having at least 25% less sugars per amount customarily consumed than the sugars content of a comparable food product.</obo:IAO_0000115>
        <obo:IAO_0000412>http://langual.org</obo:IAO_0000412>
        <oboInOwl:hasDbXref>http://www.langual.org/langual_thesaurus.asp?termid=P0181</oboInOwl:hasDbXref>
        <rdfs:label xml:lang="en">reduced sugars food</rdfs:label>
    </owl:Class>
    


    <!-- http://purl.obolibrary.org/obo/FOODON_03510182 -->


    <owl:Class rdf:about="http://purl.obolibrary.org/obo/FOODON_03510182">
        <rdfs:subClassOf rdf:resource="http://purl.obolibrary.org/obo/FOODON_03510159"/>
        <obo:IAO_0000114 rdf:resource="http://purl.obolibrary.org/obo/IAO_0000428"/>
        <obo:IAO_0000115 xml:lang="en">Wild or semiwild foods consumed only during periods of famine when no other food is available.</obo:IAO_0000115>
        <obo:IAO_0000412>http://langual.org</obo:IAO_0000412>
        <oboInOwl:hasDbXref>http://www.langual.org/langual_thesaurus.asp?termid=P0182</oboInOwl:hasDbXref>
        <oboInOwl:hasSynonym xml:lang="en">starvation food</oboInOwl:hasSynonym>
        <rdfs:label xml:lang="en">aliment de disette</rdfs:label>
    </owl:Class>
    


    <!-- http://purl.obolibrary.org/obo/FOODON_03510183 -->


    <owl:Class rdf:about="http://purl.obolibrary.org/obo/FOODON_03510183">
        <rdfs:subClassOf rdf:resource="http://purl.obolibrary.org/obo/FOODON_03510095"/>
        <obo:IAO_0000114 rdf:resource="http://purl.obolibrary.org/obo/IAO_0000428"/>
        <obo:IAO_0000115 xml:lang="en">A food is &apos;enriched&apos; when nutrients are added to it to replace those that are lost in processing.</obo:IAO_0000115>
        <obo:IAO_0000412>http://langual.org</obo:IAO_0000412>
        <oboInOwl:hasDbXref>http://www.langual.org/langual_thesaurus.asp?termid=P0183</oboInOwl:hasDbXref>
        <rdfs:comment xml:lang="en">LanguaL curation note: Used when nutrients are added to the food to replace those that are lost in processing</rdfs:comment>
        <rdfs:label xml:lang="en">enriched claim or use</rdfs:label>
    </owl:Class>
    


    <!-- http://purl.obolibrary.org/obo/FOODON_03510184 -->


    <owl:Class rdf:about="http://purl.obolibrary.org/obo/FOODON_03510184">
        <rdfs:subClassOf rdf:resource="http://purl.obolibrary.org/obo/FOODON_03510095"/>
        <obo:IAO_0000114 rdf:resource="http://purl.obolibrary.org/obo/IAO_0000428"/>
        <obo:IAO_0000115 xml:lang="en">A food is &apos;fortified&apos; when nutrients that were never present are added to it.</obo:IAO_0000115>
        <obo:IAO_0000412>http://langual.org</obo:IAO_0000412>
        <oboInOwl:hasDbXref>http://www.langual.org/langual_thesaurus.asp?termid=P0184</oboInOwl:hasDbXref>
        <rdfs:comment xml:lang="en">LanguaL curation note: Used  when nutrients that were never present are added to the food.</rdfs:comment>
        <rdfs:label xml:lang="en">fortified claim or use</rdfs:label>
    </owl:Class>
    


    <!-- http://purl.obolibrary.org/obo/FOODON_03510185 -->


    <owl:Class rdf:about="http://purl.obolibrary.org/obo/FOODON_03510185">
        <rdfs:subClassOf rdf:resource="http://purl.obolibrary.org/obo/FOODON_03510095"/>
        <obo:IAO_0000114 rdf:resource="http://purl.obolibrary.org/obo/IAO_0000428"/>
        <obo:IAO_0000412>http://langual.org</obo:IAO_0000412>
        <oboInOwl:hasDbXref>http://www.langual.org/langual_thesaurus.asp?termid=P0185</oboInOwl:hasDbXref>
        <rdfs:label xml:lang="en">iodized claim or use</rdfs:label>
    </owl:Class>
    


    <!-- http://purl.obolibrary.org/obo/FOODON_03510186 -->


    <owl:Class rdf:about="http://purl.obolibrary.org/obo/FOODON_03510186">
        <rdfs:subClassOf rdf:resource="http://purl.obolibrary.org/obo/FOODON_03510095"/>
        <obo:IAO_0000114 rdf:resource="http://purl.obolibrary.org/obo/IAO_0000428"/>
        <obo:IAO_0000412>http://langual.org</obo:IAO_0000412>
        <oboInOwl:hasDbXref>http://www.langual.org/langual_thesaurus.asp?termid=P0186</oboInOwl:hasDbXref>
        <rdfs:label xml:lang="en">unfortified claim or use</rdfs:label>
    </owl:Class>
    


    <!-- http://purl.obolibrary.org/obo/FOODON_03510187 -->


    <owl:Class rdf:about="http://purl.obolibrary.org/obo/FOODON_03510187">
        <rdfs:subClassOf rdf:resource="http://purl.obolibrary.org/obo/FOODON_03510126"/>
        <obo:IAO_0000114 rdf:resource="http://purl.obolibrary.org/obo/IAO_0000428"/>
        <obo:IAO_0000115 xml:lang="en">Characterized by adherence to the dietary practices required by Islamic law (Webster&apos;s).</obo:IAO_0000115>
        <obo:IAO_0000412>http://langual.org</obo:IAO_0000412>
        <oboInOwl:hasDbXref>http://www.langual.org/langual_thesaurus.asp?termid=P0187</oboInOwl:hasDbXref>
        <rdfs:label xml:lang="en">halal claim or use</rdfs:label>
    </owl:Class>
    


    <!-- http://purl.obolibrary.org/obo/FOODON_03510193 -->


    <owl:Class rdf:about="http://purl.obolibrary.org/obo/FOODON_03510193">
        <rdfs:subClassOf rdf:resource="http://purl.obolibrary.org/obo/FOODON_03510115"/>
        <obo:IAO_0000114 rdf:resource="http://purl.obolibrary.org/obo/IAO_0000428"/>
        <obo:IAO_0000412>http://langual.org</obo:IAO_0000412>
        <oboInOwl:hasDbXref>http://www.langual.org/langual_thesaurus.asp?termid=P0193</oboInOwl:hasDbXref>
        <rdfs:label xml:lang="en">low alcohol claim or use</rdfs:label>
    </owl:Class>
    


    <!-- http://purl.obolibrary.org/obo/FOODON_03510194 -->


    <owl:Class rdf:about="http://purl.obolibrary.org/obo/FOODON_03510194">
        <rdfs:subClassOf rdf:resource="http://purl.obolibrary.org/obo/FOODON_03510115"/>
        <obo:IAO_0000114 rdf:resource="http://purl.obolibrary.org/obo/IAO_0000428"/>
        <obo:IAO_0000412>http://langual.org</obo:IAO_0000412>
        <oboInOwl:hasDbXref>http://www.langual.org/langual_thesaurus.asp?termid=P0194</oboInOwl:hasDbXref>
        <rdfs:label xml:lang="en">probiotic claim or use</rdfs:label>
    </owl:Class>
    


    <!-- http://purl.obolibrary.org/obo/FOODON_03510195 -->


    <owl:Class rdf:about="http://purl.obolibrary.org/obo/FOODON_03510195">
        <rdfs:subClassOf rdf:resource="http://purl.obolibrary.org/obo/FOODON_03510017"/>
        <obo:IAO_0000114 rdf:resource="http://purl.obolibrary.org/obo/IAO_0000428"/>
        <obo:IAO_0000412>http://langual.org</obo:IAO_0000412>
        <oboInOwl:hasDbXref>http://www.langual.org/langual_thesaurus.asp?termid=P0195</oboInOwl:hasDbXref>
        <rdfs:label xml:lang="en">full fat claim or use</rdfs:label>
    </owl:Class>
    


    <!-- http://purl.obolibrary.org/obo/FOODON_03510196 -->


    <owl:Class rdf:about="http://purl.obolibrary.org/obo/FOODON_03510196">
        <rdfs:subClassOf rdf:resource="http://purl.obolibrary.org/obo/FOODON_03510017"/>
        <obo:IAO_0000114 rdf:resource="http://purl.obolibrary.org/obo/IAO_0000428"/>
        <obo:IAO_0000412>http://langual.org</obo:IAO_0000412>
        <oboInOwl:hasDbXref>http://www.langual.org/langual_thesaurus.asp?termid=P0196</oboInOwl:hasDbXref>
        <rdfs:label xml:lang="en">trans fat claim or use</rdfs:label>
    </owl:Class>
    


    <!-- http://purl.obolibrary.org/obo/FOODON_03510197 -->


    <owl:Class rdf:about="http://purl.obolibrary.org/obo/FOODON_03510197">
        <rdfs:subClassOf rdf:resource="http://purl.obolibrary.org/obo/FOODON_03510159"/>
        <obo:IAO_0000114 rdf:resource="http://purl.obolibrary.org/obo/IAO_0000428"/>
        <obo:IAO_0000115 xml:lang="en">Food Quality/Food Assurance Claim indicates, with reference to the product branding, labelling or packaging, whether the product is stamped with a quality mark, as approved by the governing authority, such as USDA for USA products [Source: GS1].</obo:IAO_0000115>
        <obo:IAO_0000412>http://langual.org</obo:IAO_0000412>
        <oboInOwl:hasDbXref>http://www.langual.org/langual_thesaurus.asp?termid=P0197</oboInOwl:hasDbXref>
        <rdfs:label xml:lang="en">food quality claim</rdfs:label>
    </owl:Class>
    


    <!-- http://purl.obolibrary.org/obo/FOODON_03510198 -->


    <owl:Class rdf:about="http://purl.obolibrary.org/obo/FOODON_03510198">
        <rdfs:subClassOf rdf:resource="http://purl.obolibrary.org/obo/FOODON_03510124"/>
        <obo:IAO_0000114 rdf:resource="http://purl.obolibrary.org/obo/IAO_0000428"/>
        <obo:IAO_0000115 xml:lang="en">It should be noted that such claims are illegal in some countries, e.g. Denmark, and that other countries, e.g. United Kingdom, are calling for an end to the use of terms such as &apos;diabetic&apos; or &apos;suitable for diabetics&apos; on food labels.
The European Commission is considering how foods intended specifically for people with diabetes can be controlled.</obo:IAO_0000115>
        <obo:IAO_0000412>http://langual.org</obo:IAO_0000412>
        <oboInOwl:hasDbXref>http://www.langual.org/langual_thesaurus.asp?termid=P0198</oboInOwl:hasDbXref>
        <rdfs:label xml:lang="en">diabetic or suitable for diabetics claim or use</rdfs:label>
    </owl:Class>
    


    <!-- http://purl.obolibrary.org/obo/FOODON_03510199 -->


    <owl:Class rdf:about="http://purl.obolibrary.org/obo/FOODON_03510199">
        <rdfs:subClassOf rdf:resource="http://purl.obolibrary.org/obo/FOODON_03510126"/>
        <obo:IAO_0000114 rdf:resource="http://purl.obolibrary.org/obo/IAO_0000428"/>
        <obo:IAO_0000412>http://langual.org</obo:IAO_0000412>
        <oboInOwl:hasDbXref>http://www.langual.org/langual_thesaurus.asp?termid=P0199</oboInOwl:hasDbXref>
        <rdfs:label xml:lang="en">vegan/vegetarian or suitability for vegan/vegetarian claim or use</rdfs:label>
    </owl:Class>
    


    <!-- http://purl.obolibrary.org/obo/FOODON_03510200 -->


    <owl:Class rdf:about="http://purl.obolibrary.org/obo/FOODON_03510200">
        <rdfs:subClassOf rdf:resource="http://purl.obolibrary.org/obo/FOODON_03510115"/>
        <obo:IAO_0000114 rdf:resource="http://purl.obolibrary.org/obo/IAO_0000428"/>
        <obo:IAO_0000412>http://langual.org</obo:IAO_0000412>
        <oboInOwl:hasDbXref>http://www.langual.org/langual_thesaurus.asp?termid=P0200</oboInOwl:hasDbXref>
        <rdfs:comment xml:lang="en">LanguaL curation note: Denotes a product that contains no pork meat.</rdfs:comment>
        <rdfs:label xml:lang="en">no pork added claim</rdfs:label>
    </owl:Class>
    


    <!-- http://purl.obolibrary.org/obo/FOODON_03510201 -->


    <owl:Class rdf:about="http://purl.obolibrary.org/obo/FOODON_03510201">
        <rdfs:subClassOf rdf:resource="http://purl.obolibrary.org/obo/FOODON_03510115"/>
        <obo:IAO_0000114 rdf:resource="http://purl.obolibrary.org/obo/IAO_0000428"/>
        <obo:IAO_0000412>http://langual.org</obo:IAO_0000412>
        <oboInOwl:hasDbXref>http://www.langual.org/langual_thesaurus.asp?termid=P0201</oboInOwl:hasDbXref>
        <rdfs:comment xml:lang="en">LanguaL curation note: Denotes a product that contains no beef or beef-products. Beef is considered to be a taboo foodproduct by some religions most notable Hinduism, Boedism and Jainism.</rdfs:comment>
        <rdfs:label xml:lang="en">no beef added claim</rdfs:label>
    </owl:Class>
    


    <!-- http://purl.obolibrary.org/obo/FOODON_03510202 -->


    <owl:Class rdf:about="http://purl.obolibrary.org/obo/FOODON_03510202">
        <rdfs:subClassOf rdf:resource="http://purl.obolibrary.org/obo/FOODON_03510065"/>
        <obo:IAO_0000114 rdf:resource="http://purl.obolibrary.org/obo/IAO_0000428"/>
        <obo:IAO_0000115 xml:lang="en">Food that is promoted as being either high or low in protein.</obo:IAO_0000115>
        <obo:IAO_0000412>http://langual.org</obo:IAO_0000412>
        <oboInOwl:hasDbXref>http://www.langual.org/langual_thesaurus.asp?termid=P0202</oboInOwl:hasDbXref>
        <rdfs:label xml:lang="en">protein special claim or use</rdfs:label>
    </owl:Class>
    


    <!-- http://purl.obolibrary.org/obo/FOODON_03510203 -->


    <owl:Class rdf:about="http://purl.obolibrary.org/obo/FOODON_03510203">
        <rdfs:subClassOf rdf:resource="http://purl.obolibrary.org/obo/FOODON_03510202"/>
        <obo:IAO_0000114 rdf:resource="http://purl.obolibrary.org/obo/IAO_0000428"/>
        <obo:IAO_0000115 xml:lang="en">A claim that a food is high in protein, and any claim likely to have the same meaning for the consumer, may only be made where at least 20 % of the energy value of the food is provided by protein [REGULATION (EC) No 1924/2006 Corrigendum 2007-01-18].</obo:IAO_0000115>
        <obo:IAO_0000412>http://langual.org</obo:IAO_0000412>
        <oboInOwl:hasDbXref>http://www.langual.org/langual_thesaurus.asp?termid=P0203</oboInOwl:hasDbXref>
        <rdfs:label xml:lang="en">high protein food</rdfs:label>
    </owl:Class>
    


    <!-- http://purl.obolibrary.org/obo/FOODON_03510204 -->


    <owl:Class rdf:about="http://purl.obolibrary.org/obo/FOODON_03510204">
        <rdfs:subClassOf rdf:resource="http://purl.obolibrary.org/obo/FOODON_03510210"/>
        <obo:IAO_0000114 rdf:resource="http://purl.obolibrary.org/obo/IAO_0000428"/>
        <obo:IAO_0000412>http://langual.org</obo:IAO_0000412>
        <oboInOwl:hasDbXref>http://www.langual.org/langual_thesaurus.asp?termid=P0204</oboInOwl:hasDbXref>
        <rdfs:comment xml:lang="en">LanguaL curation note: A claim that a food is a natural source of vitamins and/or minerals, and any claim likely to have the same meaning for the consumer, may only be made where the product contains at least 15% of the recommended daily allowance specified in the Annex of Council Directive 90/496/EEC per 100 g or 100 ml.</rdfs:comment>
        <rdfs:label xml:lang="en">natural source of vitamins and or minerals</rdfs:label>
    </owl:Class>
    


    <!-- http://purl.obolibrary.org/obo/FOODON_03510205 -->


    <owl:Class rdf:about="http://purl.obolibrary.org/obo/FOODON_03510205">
        <rdfs:subClassOf rdf:resource="http://purl.obolibrary.org/obo/FOODON_03510049"/>
        <obo:IAO_0000114 rdf:resource="http://purl.obolibrary.org/obo/IAO_0000428"/>
        <obo:IAO_0000115 xml:lang="en">A claim that a food is a source of fibre, and any claim likely to have the same meaning for the consumer, may only be made where the product contains at least 3 g of fibre per 100 g or at least 1,5 g of fibre per 100 kcal [REGULATION (EC) No 1924/2006 Corrigendum 2007-01-18].</obo:IAO_0000115>
        <obo:IAO_0000412>http://langual.org</obo:IAO_0000412>
        <oboInOwl:hasDbXref>http://www.langual.org/langual_thesaurus.asp?termid=P0205</oboInOwl:hasDbXref>
        <rdfs:label xml:lang="en">source of fibre</rdfs:label>
    </owl:Class>
    


    <!-- http://purl.obolibrary.org/obo/FOODON_03510206 -->


    <owl:Class rdf:about="http://purl.obolibrary.org/obo/FOODON_03510206">
        <rdfs:subClassOf rdf:resource="http://purl.obolibrary.org/obo/FOODON_03510202"/>
        <obo:IAO_0000114 rdf:resource="http://purl.obolibrary.org/obo/IAO_0000428"/>
        <obo:IAO_0000115 xml:lang="en">A claim that a food is a source of protein, and any claim likely to have the same meaning for the consumer, may only be made where at least 12 % of the energy value of the food is provided by protein. [REGULATION (EC) No 1924/2006 Corrigendum].</obo:IAO_0000115>
        <obo:IAO_0000412>http://langual.org</obo:IAO_0000412>
        <oboInOwl:hasDbXref>http://www.langual.org/langual_thesaurus.asp?termid=P0206</oboInOwl:hasDbXref>
        <rdfs:label xml:lang="en">source of protein</rdfs:label>
    </owl:Class>
    


    <!-- http://purl.obolibrary.org/obo/FOODON_03510207 -->


    <owl:Class rdf:about="http://purl.obolibrary.org/obo/FOODON_03510207">
        <rdfs:subClassOf rdf:resource="http://purl.obolibrary.org/obo/FOODON_03510095"/>
        <obo:IAO_0000114 rdf:resource="http://purl.obolibrary.org/obo/IAO_0000428"/>
        <obo:IAO_0000115 xml:lang="en">A claim that a food contains a nutrient or another substance, for which specific conditions are not laid down in this Regulation, or any claim likely to have the same meaning for the consumer, may only be made where the product complies with all the applicable provisions of this Regulation, and in particular Article 5. For vitamins and minerals the conditions of the claim &quot;source of&quot; shall apply. [REGULATION (EC) No 1924/2006 Corrigendum 2007-01-18].</obo:IAO_0000115>
        <obo:IAO_0000412>http://langual.org</obo:IAO_0000412>
        <oboInOwl:hasDbXref>http://www.langual.org/langual_thesaurus.asp?termid=P0207</oboInOwl:hasDbXref>
        <rdfs:comment xml:lang="en">LanguaL curation note: Used for claims like &quot;contains [name of the nutrient or other substance]&quot;.</rdfs:comment>
        <rdfs:label xml:lang="en">contains {name of the nutrient or other substance} nutrition claim</rdfs:label>
    </owl:Class>
    


    <!-- http://purl.obolibrary.org/obo/FOODON_03510208 -->


    <owl:Class rdf:about="http://purl.obolibrary.org/obo/FOODON_03510208">
        <rdfs:subClassOf rdf:resource="http://purl.obolibrary.org/obo/FOODON_03510095"/>
        <obo:IAO_0000114 rdf:resource="http://purl.obolibrary.org/obo/IAO_0000428"/>
        <obo:IAO_0000115 xml:lang="en">A claim stating that the content in one or more nutrients, other than vitamins and minerals, has been increased, and any claim likely to have the same meaning for the consumer, may only be made where the product meets the conditions for the claim &quot;source of&quot; and the increase in content is at least 30 % compared to a similar product. [Forordning (EF) nr. 1924/2006 Berigtigelse 2007-01-18].</obo:IAO_0000115>
        <obo:IAO_0000412>http://langual.org</obo:IAO_0000412>
        <oboInOwl:hasDbXref>http://www.langual.org/langual_thesaurus.asp?termid=P0208</oboInOwl:hasDbXref>
        <rdfs:label xml:lang="en">increased {name of nutrient} nutrition claim</rdfs:label>
    </owl:Class>
    


    <!-- http://purl.obolibrary.org/obo/FOODON_03510209 -->


    <owl:Class rdf:about="http://purl.obolibrary.org/obo/FOODON_03510209">
        <rdfs:subClassOf rdf:resource="http://purl.obolibrary.org/obo/FOODON_03510059"/>
        <obo:IAO_0000114 rdf:resource="http://purl.obolibrary.org/obo/IAO_0000428"/>
        <obo:IAO_0000115 xml:lang="en">Where a food naturally meets the condition(s) laid down in this Annex for the use of a nutritional claim, the term &quot;naturally/natural&quot; may be used as a prefix to the claim [REGULATION (EC) No 1924/2006 Corrigendum2007-01-18].</obo:IAO_0000115>
        <obo:IAO_0000412>http://langual.org</obo:IAO_0000412>
        <oboInOwl:hasDbXref>http://www.langual.org/langual_thesaurus.asp?termid=P0209</oboInOwl:hasDbXref>
        <rdfs:label xml:lang="en">&quot;naturally/natural&quot; label claim</rdfs:label>
    </owl:Class>
    


    <!-- http://purl.obolibrary.org/obo/FOODON_03510210 -->


    <owl:Class rdf:about="http://purl.obolibrary.org/obo/FOODON_03510210">
        <rdfs:subClassOf rdf:resource="http://purl.obolibrary.org/obo/FOODON_03510095"/>
        <obo:IAO_0000114 rdf:resource="http://purl.obolibrary.org/obo/IAO_0000428"/>
        <obo:IAO_0000115 xml:lang="en">A claim that a food is a source of vitamins and/or minerals, and any claim likely to have the same meaning for the consumer, may only be made where the product contains at least a significant amount as defined in the Annex to Directive 90/496/EEC or an amount provided for by derogations granted according to Article 6 of Regulation (EC) No 1925/2006 of the European Parliament and of the Council of 20 December 2006 on the addition of vitamins and minerals and of certain other substances to foods [REGULATION (EC) No 1924/2006 Corrigendum2007-01-18].</obo:IAO_0000115>
        <obo:IAO_0000412>http://langual.org</obo:IAO_0000412>
        <oboInOwl:hasDbXref>http://www.langual.org/langual_thesaurus.asp?termid=P0210</oboInOwl:hasDbXref>
        <rdfs:label xml:lang="en">source of {name of vitamin/s}  and/or {name of mineral/s} nutrition claim</rdfs:label>
    </owl:Class>
    


    <!-- http://purl.obolibrary.org/obo/FOODON_03510211 -->


    <owl:Class rdf:about="http://purl.obolibrary.org/obo/FOODON_03510211">
        <rdfs:subClassOf rdf:resource="http://purl.obolibrary.org/obo/FOODON_03510095"/>
        <obo:IAO_0000114 rdf:resource="http://purl.obolibrary.org/obo/IAO_0000428"/>
        <obo:IAO_0000115 xml:lang="en">A claim that a food is high in vitamins and/or minerals, and any claim likely to have the same meaning for the consumer, may only be made where the product contains at least twice the value of &quot;source of [NAME OF VITAMIN/S] and/or [NAME OF MINERAL/S]&quot; [REGULATION (EC) No 1924/2006 Corrigendum 2007-01-18].</obo:IAO_0000115>
        <obo:IAO_0000412>http://langual.org</obo:IAO_0000412>
        <oboInOwl:hasDbXref>http://www.langual.org/langual_thesaurus.asp?termid=P0211</oboInOwl:hasDbXref>
        <rdfs:label xml:lang="en">high {name of vitamin/s} and/or {name of mineral/s} nutrition claim</rdfs:label>
    </owl:Class>
    


    <!-- http://purl.obolibrary.org/obo/FOODON_03510212 -->


    <owl:Class rdf:about="http://purl.obolibrary.org/obo/FOODON_03510212">
        <rdfs:subClassOf rdf:resource="http://purl.obolibrary.org/obo/FOODON_03510095"/>
        <obo:IAO_0000114 rdf:resource="http://purl.obolibrary.org/obo/IAO_0000428"/>
        <obo:IAO_0000115 xml:lang="en">A claim stating that the content in one or more nutrients has been reduced, and any claim likely to have the same meaning for the consumer, may only be made where the reduction in content is at least 30 % compared to a similar product, except for micronutrients, where a 10 % difference in the reference values as set in Directive 90/496/EEC shall be acceptable, and for sodium, or the equivalent value for salt, where a 25 % difference shall be acceptable. [REGULATION (EC) No 1924/2006 Corrigendum 2007-01-18].</obo:IAO_0000115>
        <obo:IAO_0000412>http://langual.org</obo:IAO_0000412>
        <oboInOwl:hasDbXref>http://www.langual.org/langual_thesaurus.asp?termid=P0212</oboInOwl:hasDbXref>
        <rdfs:label xml:lang="en">reduced {name of nutrient} nutrition claim</rdfs:label>
    </owl:Class>
    


    <!-- http://purl.obolibrary.org/obo/FOODON_03510213 -->


    <owl:Class rdf:about="http://purl.obolibrary.org/obo/FOODON_03510213">
        <rdfs:subClassOf rdf:resource="http://purl.obolibrary.org/obo/FOODON_03510032"/>
        <obo:IAO_0000114 rdf:resource="http://purl.obolibrary.org/obo/IAO_0000428"/>
        <obo:IAO_0000412>http://langual.org</obo:IAO_0000412>
        <oboInOwl:hasDbXref>http://www.langual.org/langual_thesaurus.asp?termid=P0213</oboInOwl:hasDbXref>
        <rdfs:comment xml:lang="en">LanguaL curation note: This term is for CLASSIFICATION ONLY; DO NOT USE term in indexing. Use a more precise narrower term.</rdfs:comment>
        <rdfs:label xml:lang="en">food allergen labelling</rdfs:label>
    </owl:Class>
    


    <!-- http://purl.obolibrary.org/obo/FOODON_03510214 -->


    <owl:Class rdf:about="http://purl.obolibrary.org/obo/FOODON_03510214">
        <rdfs:subClassOf rdf:resource="http://purl.obolibrary.org/obo/FOODON_03510213"/>
        <obo:IAO_0000114 rdf:resource="http://purl.obolibrary.org/obo/IAO_0000428"/>
        <obo:IAO_0000115 xml:lang="en">Regulated by Directive 2003/89/EC of the European Parliament and of the Council of 10 November 2003 amending Directive 2000/13/EC as regards indication of the ingredients present in foodstuffs.</obo:IAO_0000115>
        <obo:IAO_0000412>http://langual.org</obo:IAO_0000412>
        <oboInOwl:hasDbXref>http://www.langual.org/langual_thesaurus.asp?termid=P0214</oboInOwl:hasDbXref>
        <rdfs:comment xml:lang="en">LanguaL curation note: Used for cereals containing gluten ( i.e. wheat, rye, barley, oats, spelt, kamut or their hybridised strains) and products thereof</rdfs:comment>
        <rdfs:label xml:lang="en">food allergen labelling about cereals containing gluten and products thereof</rdfs:label>
    </owl:Class>
    


    <!-- http://purl.obolibrary.org/obo/FOODON_03510215 -->


    <owl:Class rdf:about="http://purl.obolibrary.org/obo/FOODON_03510215">
        <rdfs:subClassOf rdf:resource="http://purl.obolibrary.org/obo/FOODON_03510213"/>
        <obo:IAO_0000114 rdf:resource="http://purl.obolibrary.org/obo/IAO_0000428"/>
        <obo:IAO_0000115 xml:lang="en">Regulated by Directive 2003/89/EC of the European Parliament and of the Council of 10 November 2003 amending Directive 2000/13/EC as regards indication of the ingredients present in foodstuffs.</obo:IAO_0000115>
        <obo:IAO_0000412>http://langual.org</obo:IAO_0000412>
        <oboInOwl:hasDbXref>http://www.langual.org/langual_thesaurus.asp?termid=P0215</oboInOwl:hasDbXref>
        <rdfs:label xml:lang="en">food allergen labelling about crustaceans and products thereof</rdfs:label>
    </owl:Class>
    


    <!-- http://purl.obolibrary.org/obo/FOODON_03510216 -->


    <owl:Class rdf:about="http://purl.obolibrary.org/obo/FOODON_03510216">
        <rdfs:subClassOf rdf:resource="http://purl.obolibrary.org/obo/FOODON_03510213"/>
        <obo:IAO_0000114 rdf:resource="http://purl.obolibrary.org/obo/IAO_0000428"/>
        <obo:IAO_0000115 xml:lang="en">Regulated by Directive 2003/89/EC of the European Parliament and of the Council of 10 November 2003 amending Directive 2000/13/EC as regards indication of the ingredients present in foodstuffs.</obo:IAO_0000115>
        <obo:IAO_0000412>http://langual.org</obo:IAO_0000412>
        <oboInOwl:hasDbXref>http://www.langual.org/langual_thesaurus.asp?termid=P0216</oboInOwl:hasDbXref>
        <rdfs:label xml:lang="en">food allergen labelling about eggs and products thereof</rdfs:label>
    </owl:Class>
    


    <!-- http://purl.obolibrary.org/obo/FOODON_03510217 -->


    <owl:Class rdf:about="http://purl.obolibrary.org/obo/FOODON_03510217">
        <rdfs:subClassOf rdf:resource="http://purl.obolibrary.org/obo/FOODON_03510213"/>
        <obo:IAO_0000114 rdf:resource="http://purl.obolibrary.org/obo/IAO_0000428"/>
        <obo:IAO_0000115 xml:lang="en">Regulated by Directive 2003/89/EC of the European Parliament and of the Council of 10 November 2003 amending Directive 2000/13/EC as regards indication of the ingredients present in foodstuffs.</obo:IAO_0000115>
        <obo:IAO_0000412>http://langual.org</obo:IAO_0000412>
        <oboInOwl:hasDbXref>http://www.langual.org/langual_thesaurus.asp?termid=P0217</oboInOwl:hasDbXref>
        <rdfs:label xml:lang="en">food allergen labelling about fish and products thereof</rdfs:label>
    </owl:Class>
    


    <!-- http://purl.obolibrary.org/obo/FOODON_03510218 -->


    <owl:Class rdf:about="http://purl.obolibrary.org/obo/FOODON_03510218">
        <rdfs:subClassOf rdf:resource="http://purl.obolibrary.org/obo/FOODON_03510213"/>
        <obo:IAO_0000114 rdf:resource="http://purl.obolibrary.org/obo/IAO_0000428"/>
        <obo:IAO_0000115 xml:lang="en">Regulated by Directive 2003/89/EC of the European Parliament and of the Council of 10 November 2003 amending Directive 2000/13/EC as regards indication of the ingredients present in foodstuffs.</obo:IAO_0000115>
        <obo:IAO_0000412>http://langual.org</obo:IAO_0000412>
        <oboInOwl:hasDbXref>http://www.langual.org/langual_thesaurus.asp?termid=P0218</oboInOwl:hasDbXref>
        <rdfs:label xml:lang="en">food allergen labelling about peanuts and products thereof</rdfs:label>
    </owl:Class>
    


    <!-- http://purl.obolibrary.org/obo/FOODON_03510219 -->


    <owl:Class rdf:about="http://purl.obolibrary.org/obo/FOODON_03510219">
        <rdfs:subClassOf rdf:resource="http://purl.obolibrary.org/obo/FOODON_03510213"/>
        <obo:IAO_0000114 rdf:resource="http://purl.obolibrary.org/obo/IAO_0000428"/>
        <obo:IAO_0000115 xml:lang="en">Regulated by Directive 2003/89/EC of the European Parliament and of the Council of 10 November 2003 amending Directive 2000/13/EC as regards indication of the ingredients present in foodstuffs.</obo:IAO_0000115>
        <obo:IAO_0000412>http://langual.org</obo:IAO_0000412>
        <oboInOwl:hasDbXref>http://www.langual.org/langual_thesaurus.asp?termid=P0219</oboInOwl:hasDbXref>
        <rdfs:label xml:lang="en">food allergen labelling about soybeans and products thereof</rdfs:label>
    </owl:Class>
    


    <!-- http://purl.obolibrary.org/obo/FOODON_03510220 -->


    <owl:Class rdf:about="http://purl.obolibrary.org/obo/FOODON_03510220">
        <rdfs:subClassOf rdf:resource="http://purl.obolibrary.org/obo/FOODON_03510213"/>
        <obo:IAO_0000114 rdf:resource="http://purl.obolibrary.org/obo/IAO_0000428"/>
        <obo:IAO_0000115 xml:lang="en">Regulated by Directive 2003/89/EC of the European Parliament and of the Council of 10 November 2003 amending Directive 2000/13/EC as regards indication of the ingredients present in foodstuffs.</obo:IAO_0000115>
        <obo:IAO_0000412>http://langual.org</obo:IAO_0000412>
        <oboInOwl:hasDbXref>http://www.langual.org/langual_thesaurus.asp?termid=P0220</oboInOwl:hasDbXref>
        <rdfs:label xml:lang="en">food allergen labelling about milk and products thereof, including lactose</rdfs:label>
    </owl:Class>
    


    <!-- http://purl.obolibrary.org/obo/FOODON_03510221 -->


    <owl:Class rdf:about="http://purl.obolibrary.org/obo/FOODON_03510221">
        <rdfs:subClassOf rdf:resource="http://purl.obolibrary.org/obo/FOODON_03510213"/>
        <obo:IAO_0000114 rdf:resource="http://purl.obolibrary.org/obo/IAO_0000428"/>
        <obo:IAO_0000115 xml:lang="en">Regulated by Directive 2003/89/EC of the European Parliament and of the Council of 10 November 2003 amending Directive 2000/13/EC as regards indication of the ingredients present in foodstuffs.</obo:IAO_0000115>
        <obo:IAO_0000412>http://langual.org</obo:IAO_0000412>
        <oboInOwl:hasDbXref>http://www.langual.org/langual_thesaurus.asp?termid=P0221</oboInOwl:hasDbXref>
        <rdfs:comment xml:lang="en">LanguaL curation note: Used for nuts i. e. Almond (Amygdalus communis L.), Hazelnut (Corylus avellana), Walnut (Juglans regia), Cashew (Anacardium occidentale), Pecan nut (Carya illinoiesis (Wangenh.) K. Koch), Brazil nut (Bertholletia excelsa), Pistachio nut (Pistacia vera), Macadamia nut and Queensland nut (Macadamia ternifolia) and products thereof.</rdfs:comment>
        <rdfs:label xml:lang="en">food allergen labelling about nuts and products thereof</rdfs:label>
    </owl:Class>
    


    <!-- http://purl.obolibrary.org/obo/FOODON_03510222 -->


    <owl:Class rdf:about="http://purl.obolibrary.org/obo/FOODON_03510222">
        <rdfs:subClassOf rdf:resource="http://purl.obolibrary.org/obo/FOODON_03510213"/>
        <obo:IAO_0000114 rdf:resource="http://purl.obolibrary.org/obo/IAO_0000428"/>
        <obo:IAO_0000115 xml:lang="en">Regulated by Directive 2003/89/EC of the European Parliament and of the Council of 10 November 2003 amending Directive 2000/13/EC as regards indication of the ingredients present in foodstuffs.</obo:IAO_0000115>
        <obo:IAO_0000412>http://langual.org</obo:IAO_0000412>
        <oboInOwl:hasDbXref>http://www.langual.org/langual_thesaurus.asp?termid=P0222</oboInOwl:hasDbXref>
        <rdfs:label xml:lang="en">food allergen labelling about celery and products thereof</rdfs:label>
    </owl:Class>
    


    <!-- http://purl.obolibrary.org/obo/FOODON_03510223 -->


    <owl:Class rdf:about="http://purl.obolibrary.org/obo/FOODON_03510223">
        <rdfs:subClassOf rdf:resource="http://purl.obolibrary.org/obo/FOODON_03510213"/>
        <obo:IAO_0000114 rdf:resource="http://purl.obolibrary.org/obo/IAO_0000428"/>
        <obo:IAO_0000115 xml:lang="en">Regulated by Directive 2003/89/EC of the European Parliament and of the Council of 10 November 2003 amending Directive 2000/13/EC as regards indication of the ingredients present in foodstuffs.</obo:IAO_0000115>
        <obo:IAO_0000412>http://langual.org</obo:IAO_0000412>
        <oboInOwl:hasDbXref>http://www.langual.org/langual_thesaurus.asp?termid=P0223</oboInOwl:hasDbXref>
        <rdfs:label xml:lang="en">food allergen labelling about mustard and products thereof</rdfs:label>
    </owl:Class>
    


    <!-- http://purl.obolibrary.org/obo/FOODON_03510224 -->


    <owl:Class rdf:about="http://purl.obolibrary.org/obo/FOODON_03510224">
        <rdfs:subClassOf rdf:resource="http://purl.obolibrary.org/obo/FOODON_03510213"/>
        <obo:IAO_0000114 rdf:resource="http://purl.obolibrary.org/obo/IAO_0000428"/>
        <obo:IAO_0000115 xml:lang="en">Regulated by Directive 2003/89/EC of the European Parliament and of the Council of 10 November 2003 amending Directive 2000/13/EC as regards indication of the ingredients present in foodstuffs.</obo:IAO_0000115>
        <obo:IAO_0000412>http://langual.org</obo:IAO_0000412>
        <oboInOwl:hasDbXref>http://www.langual.org/langual_thesaurus.asp?termid=P0224</oboInOwl:hasDbXref>
        <rdfs:label xml:lang="en">food allergen labelling about sesame seeds and products thereof</rdfs:label>
    </owl:Class>
    


    <!-- http://purl.obolibrary.org/obo/FOODON_03510225 -->


    <owl:Class rdf:about="http://purl.obolibrary.org/obo/FOODON_03510225">
        <rdfs:subClassOf rdf:resource="http://purl.obolibrary.org/obo/FOODON_03510213"/>
        <obo:IAO_0000114 rdf:resource="http://purl.obolibrary.org/obo/IAO_0000428"/>
        <obo:IAO_0000115 xml:lang="en">Sulphur dioxide and sulphites are included in the EU list of allergens
because they can cause adverse reactions in some people.

Regulated by Directive 2003/89/EC of the European Parliament and of the Council of 10 November 2003 amending Directive 2000/13/EC as regards indication of the ingredients present in foodstuffs.</obo:IAO_0000115>
        <obo:IAO_0000412>http://langual.org</obo:IAO_0000412>
        <oboInOwl:hasDbXref>http://www.langual.org/langual_thesaurus.asp?termid=P0225</oboInOwl:hasDbXref>
        <rdfs:comment xml:lang="en">LanguaL curation note: Used for sulphur dioxide and sulphites at concentrations of more than 10 mg/kg or 10 mg/litre expressed as SO2.</rdfs:comment>
        <rdfs:label xml:lang="en">food allergen labelling about sulphur dioxide and sulphites</rdfs:label>
    </owl:Class>
    


    <!-- http://purl.obolibrary.org/obo/FOODON_03510226 -->


    <owl:Class rdf:about="http://purl.obolibrary.org/obo/FOODON_03510226">
        <rdfs:subClassOf rdf:resource="http://purl.obolibrary.org/obo/FOODON_03510213"/>
        <obo:IAO_0000114 rdf:resource="http://purl.obolibrary.org/obo/IAO_0000428"/>
        <obo:IAO_0000115 xml:lang="en">Contained in GS1 Allergen Code List.</obo:IAO_0000115>
        <obo:IAO_0000412>http://langual.org</obo:IAO_0000412>
        <oboInOwl:hasDbXref>http://www.langual.org/langual_thesaurus.asp?termid=P0226</oboInOwl:hasDbXref>
        <rdfs:label xml:lang="en">food allergen labelling about cocoa and products thereof</rdfs:label>
    </owl:Class>
    


    <!-- http://purl.obolibrary.org/obo/FOODON_03510227 -->


    <owl:Class rdf:about="http://purl.obolibrary.org/obo/FOODON_03510227">
        <rdfs:subClassOf rdf:resource="http://purl.obolibrary.org/obo/FOODON_03510213"/>
        <obo:IAO_0000114 rdf:resource="http://purl.obolibrary.org/obo/IAO_0000428"/>
        <obo:IAO_0000115 xml:lang="en">Contained in GS1 Code List.</obo:IAO_0000115>
        <obo:IAO_0000412>http://langual.org</obo:IAO_0000412>
        <oboInOwl:hasDbXref>http://www.langual.org/langual_thesaurus.asp?termid=P0227</oboInOwl:hasDbXref>
        <rdfs:label xml:lang="en">food allergen labelling about coriander and products thereof</rdfs:label>
    </owl:Class>
    


    <!-- http://purl.obolibrary.org/obo/FOODON_03510228 -->


    <owl:Class rdf:about="http://purl.obolibrary.org/obo/FOODON_03510228">
        <rdfs:subClassOf rdf:resource="http://purl.obolibrary.org/obo/FOODON_03510213"/>
        <obo:IAO_0000114 rdf:resource="http://purl.obolibrary.org/obo/IAO_0000428"/>
        <obo:IAO_0000115 xml:lang="en">Contained in GS1 Code List.</obo:IAO_0000115>
        <obo:IAO_0000412>http://langual.org</obo:IAO_0000412>
        <oboInOwl:hasDbXref>http://www.langual.org/langual_thesaurus.asp?termid=P0228</oboInOwl:hasDbXref>
        <rdfs:label xml:lang="en">food allergen labelling about lupine and products thereof</rdfs:label>
    </owl:Class>
    


    <!-- http://purl.obolibrary.org/obo/FOODON_03510229 -->


    <owl:Class rdf:about="http://purl.obolibrary.org/obo/FOODON_03510229">
        <rdfs:subClassOf rdf:resource="http://purl.obolibrary.org/obo/FOODON_03510213"/>
        <obo:IAO_0000114 rdf:resource="http://purl.obolibrary.org/obo/IAO_0000428"/>
        <obo:IAO_0000115 xml:lang="en">Contained in GS1 Code List.</obo:IAO_0000115>
        <obo:IAO_0000412>http://langual.org</obo:IAO_0000412>
        <oboInOwl:hasDbXref>http://www.langual.org/langual_thesaurus.asp?termid=P0229</oboInOwl:hasDbXref>
        <rdfs:label xml:lang="en">food allergen labelling about corn and products thereof</rdfs:label>
    </owl:Class>
    


    <!-- http://purl.obolibrary.org/obo/FOODON_03510230 -->


    <owl:Class rdf:about="http://purl.obolibrary.org/obo/FOODON_03510230">
        <rdfs:subClassOf rdf:resource="http://purl.obolibrary.org/obo/FOODON_03510213"/>
        <obo:IAO_0000114 rdf:resource="http://purl.obolibrary.org/obo/IAO_0000428"/>
        <obo:IAO_0000115 xml:lang="en">Contained in GS1 Code List.</obo:IAO_0000115>
        <obo:IAO_0000412>http://langual.org</obo:IAO_0000412>
        <oboInOwl:hasDbXref>http://www.langual.org/langual_thesaurus.asp?termid=P0230</oboInOwl:hasDbXref>
        <rdfs:label xml:lang="en">food allergen labelling about pod fruits and products thereof</rdfs:label>
    </owl:Class>
    


    <!-- http://purl.obolibrary.org/obo/FOODON_03510231 -->


    <owl:Class rdf:about="http://purl.obolibrary.org/obo/FOODON_03510231">
        <rdfs:subClassOf rdf:resource="http://purl.obolibrary.org/obo/FOODON_03510213"/>
        <obo:IAO_0000114 rdf:resource="http://purl.obolibrary.org/obo/IAO_0000428"/>
        <obo:IAO_0000115 xml:lang="en">Contained in GS1 Code List.</obo:IAO_0000115>
        <obo:IAO_0000412>http://langual.org</obo:IAO_0000412>
        <oboInOwl:hasDbXref>http://www.langual.org/langual_thesaurus.asp?termid=P0231</oboInOwl:hasDbXref>
        <rdfs:label xml:lang="en">food allergen labelling about carrot and products thereof</rdfs:label>
    </owl:Class>
    


    <!-- http://purl.obolibrary.org/obo/FOODON_03510232 -->


    <owl:Class rdf:about="http://purl.obolibrary.org/obo/FOODON_03510232">
        <rdfs:subClassOf rdf:resource="http://purl.obolibrary.org/obo/FOODON_03510213"/>
        <obo:IAO_0000114 rdf:resource="http://purl.obolibrary.org/obo/IAO_0000428"/>
        <obo:IAO_0000115 xml:lang="en">Contained in GS1 Code List.</obo:IAO_0000115>
        <obo:IAO_0000412>http://langual.org</obo:IAO_0000412>
        <oboInOwl:hasDbXref>http://www.langual.org/langual_thesaurus.asp?termid=P0232</oboInOwl:hasDbXref>
        <rdfs:label xml:lang="en">food allergen labelling about molluscs and products thereof</rdfs:label>
    </owl:Class>
    


    <!-- http://purl.obolibrary.org/obo/FOODON_03510233 -->


    <owl:Class rdf:about="http://purl.obolibrary.org/obo/FOODON_03510233">
        <rdfs:subClassOf rdf:resource="http://purl.obolibrary.org/obo/FOODON_03510196"/>
        <obo:IAO_0000114 rdf:resource="http://purl.obolibrary.org/obo/IAO_0000428"/>
        <obo:IAO_0000412>http://langual.org</obo:IAO_0000412>
        <oboInOwl:hasDbXref>http://www.langual.org/langual_thesaurus.asp?termid=P0233</oboInOwl:hasDbXref>
        <rdfs:comment xml:lang="en">LanguaL curation note: Under the new FDA regulations, by Jan. 1, 2006, consumers will be able to find trans fat listed on food nutrition labels directly under the line for saturated fat. The new information is the first significant change on the Nutrition Facts panel since it was established in 1993. 
Source: http://www.fda.gov/oc/initiatives/transfat/.</rdfs:comment>
        <rdfs:label xml:lang="en">&quot;no trans fat&quot; claim or use</rdfs:label>
    </owl:Class>
    


    <!-- http://purl.obolibrary.org/obo/FOODON_03510234 -->


    <owl:Class rdf:about="http://purl.obolibrary.org/obo/FOODON_03510234">
        <rdfs:subClassOf rdf:resource="http://purl.obolibrary.org/obo/FOODON_03510126"/>
        <obo:IAO_0000114 rdf:resource="http://purl.obolibrary.org/obo/IAO_0000428"/>
        <obo:IAO_0000115 xml:lang="en">&apos;Traditional&quot; means proven usage on the Community market for a time period showing transmission between generations; this time period should be the one generally ascribed to one human generation, at least 25 years [COUNCIL REGULATION (EC) No 509/2006 of 20 March 2006 on agricultural products and foodstuffs as traditional specialities guaranteed].

A traditional food product is a product frequently consumed or associated to specific celebrations and/or seasons, normally transmitted from one generation to another, made with care in a specific way according to the gastronomic heritage, with little or no processing/manipulation, that is distinguished and known because of its sensory properties and associated to a certain local area, region or country. [http://www.truefood.eu/]

Traditional means conforming to established practice or specifications prior to the Second World War. Traditional food is a food of a specific feature or features, which distinguish it clearly from other similar products of the same category in terms of the use of traditional ingredients (raw materials or primary products), traditional composition or traditional type of production and/or processing method. [Traditional Foods in Europe, EuroFIR Synthesis report No 6, 2009]</obo:IAO_0000115>
        <obo:IAO_0000412>http://langual.org</obo:IAO_0000412>
        <oboInOwl:hasDbXref>http://www.langual.org/langual_thesaurus.asp?termid=P0234</oboInOwl:hasDbXref>
        <rdfs:label xml:lang="en">traditional food claim or use</rdfs:label>
    </owl:Class>
    


    <!-- http://purl.obolibrary.org/obo/FOODON_03510235 -->


    <owl:Class rdf:about="http://purl.obolibrary.org/obo/FOODON_03510235">
        <rdfs:subClassOf rdf:resource="http://purl.obolibrary.org/obo/FOODON_03510126"/>
        <obo:IAO_0000114 rdf:resource="http://purl.obolibrary.org/obo/IAO_0000428"/>
        <obo:IAO_0000115 xml:lang="en">Ethnic food is food from countries other than the home market contributing to a different food culture than the traditional cuisine of the host country. [Ethnic Groups and Foods in Europe, EuroFIR Synthesis report No 3, 2005]

&quot;Ethnic food&quot; has been used colloquially for a wide variety of foodstuffs, virtually any that can be identified in the public mind with a foreign source or an ethnic minority group. In the narrower ethnographic meaning, it pertains only to food prepared or consumed by members of an ethnic group as a manifestation of its ethnicity. In the end ethnic food is food that members of an ethnic group consider their own and that others attribute to them. [http://www.answers.com/topic/ethnic-cuisines]</obo:IAO_0000115>
        <obo:IAO_0000412>http://langual.org</obo:IAO_0000412>
        <oboInOwl:hasDbXref>http://www.langual.org/langual_thesaurus.asp?termid=P0235</oboInOwl:hasDbXref>
        <rdfs:label xml:lang="en">ethnic food claim or use</rdfs:label>
    </owl:Class>
    


    <!-- http://purl.obolibrary.org/obo/FOODON_03510236 -->


    <owl:Class rdf:about="http://purl.obolibrary.org/obo/FOODON_03510236">
        <rdfs:subClassOf rdf:resource="http://purl.obolibrary.org/obo/FOODON_03510234"/>
        <obo:IAO_0000114 rdf:resource="http://purl.obolibrary.org/obo/IAO_0000428"/>
        <obo:IAO_0000115 xml:lang="en">Raw material (species and/or varieties) or primary product either alone or as an ingredient that has been used in identifiable geographical areas and remains in use today (taking into account cases where use was abandoned for a time and then reinstated) and its characteristics are in accordance with current specifications of national and EU legislation. [Traditional Foods in Europe, EuroFIR Synthesis report No 6, 2009]</obo:IAO_0000115>
        <obo:IAO_0000412>http://langual.org</obo:IAO_0000412>
        <oboInOwl:hasDbXref>http://www.langual.org/langual_thesaurus.asp?termid=P0236</oboInOwl:hasDbXref>
        <rdfs:comment xml:lang="en">LanguaL curation note: Use when &quot;Traditional ingredients&quot; is claimed.</rdfs:comment>
        <rdfs:label xml:lang="en">traditional ingredient claim or use</rdfs:label>
    </owl:Class>
    


    <!-- http://purl.obolibrary.org/obo/FOODON_03510237 -->


    <owl:Class rdf:about="http://purl.obolibrary.org/obo/FOODON_03510237">
        <rdfs:subClassOf rdf:resource="http://purl.obolibrary.org/obo/FOODON_03510234"/>
        <obo:IAO_0000114 rdf:resource="http://purl.obolibrary.org/obo/IAO_0000428"/>
        <obo:IAO_0000115 xml:lang="en">The uniquely identifiable composition (in terms of ingredients) that was first established prior to the Second World War and passed down through generations by oral or other means (taking into account cases where composition was abandoned for a time and then reinstated) and when necessary is differentiated from the composition defined by the generally recognized characteristics of the wider food group to which the product belongs. [Traditional Foods in Europe, EuroFIR Synthesis report No 6, 2009]</obo:IAO_0000115>
        <obo:IAO_0000412>http://langual.org</obo:IAO_0000412>
        <oboInOwl:hasDbXref>http://www.langual.org/langual_thesaurus.asp?termid=P0237</oboInOwl:hasDbXref>
        <rdfs:comment xml:lang="en">LanguaL curation note: Use when &quot;Traditional composition&quot; is claimed.</rdfs:comment>
        <rdfs:label xml:lang="en">traditional composition claim or use</rdfs:label>
    </owl:Class>
    


    <!-- http://purl.obolibrary.org/obo/FOODON_03510238 -->


    <owl:Class rdf:about="http://purl.obolibrary.org/obo/FOODON_03510238">
        <rdfs:subClassOf rdf:resource="http://purl.obolibrary.org/obo/FOODON_03510234"/>
        <obo:IAO_0000114 rdf:resource="http://purl.obolibrary.org/obo/IAO_0000428"/>
        <obo:IAO_0000115 xml:lang="en">The production and/or processing of a food that has been transmitted from generation to generation through oral tradition or other means and has been applied prior to the Second World War and remains in use (taking into account cases where composition was abandoned for a time and then reinstated) despite its adjustment to binding rules from national or EU food hygiene regulations or the incorporation of technological progress, under the condition that production and/or processing remains in line with methods used originally and that the food&quot;s intrinsic features such as its physical, chemical, microbiological or organoleptic features are maintained. [Traditional Foods in Europe, EuroFIR Synthesis report No 6, 2009]</obo:IAO_0000115>
        <obo:IAO_0000412>http://langual.org</obo:IAO_0000412>
        <oboInOwl:hasDbXref>http://www.langual.org/langual_thesaurus.asp?termid=P0238</oboInOwl:hasDbXref>
        <rdfs:comment xml:lang="en">LanguaL curation note: Use when &quot;Traditional type of production and/or processing&quot; is claimed.</rdfs:comment>
        <rdfs:label xml:lang="en">traditional type of production and/or processing claim or use</rdfs:label>
    </owl:Class>
    


    <!-- http://purl.obolibrary.org/obo/FOODON_03510239 -->


    <owl:Class rdf:about="http://purl.obolibrary.org/obo/FOODON_03510239">
        <rdfs:subClassOf rdf:resource="http://purl.obolibrary.org/obo/FOODON_03510235"/>
        <obo:IAO_0000114 rdf:resource="http://purl.obolibrary.org/obo/IAO_0000428"/>
        <obo:IAO_0000115 xml:lang="en">Authentic ethnic food is food from countries other than the home market contributing to a different food culture than the traditional cuisine of the host country. Food may be adapted by combining local and imported ingredients. [Ethnic Groups and Foods in Europe, EuroFIR Synthesis report No 3, 2005]</obo:IAO_0000115>
        <obo:IAO_0000412>http://langual.org</obo:IAO_0000412>
        <oboInOwl:hasDbXref>http://www.langual.org/langual_thesaurus.asp?termid=P0239</oboInOwl:hasDbXref>
        <rdfs:label xml:lang="en">authentic ethnic food claim or use</rdfs:label>
    </owl:Class>
    


    <!-- http://purl.obolibrary.org/obo/FOODON_03510240 -->


    <owl:Class rdf:about="http://purl.obolibrary.org/obo/FOODON_03510240">
        <rdfs:subClassOf rdf:resource="http://purl.obolibrary.org/obo/FOODON_03510235"/>
        <obo:IAO_0000114 rdf:resource="http://purl.obolibrary.org/obo/IAO_0000428"/>
        <obo:IAO_0000115 xml:lang="en">Modified ethnic food: a commercially-available version of a food that has been modified to suit the taste and preference of the host country. [Ethnic Groups and Foods in Europe, EuroFIR Synthesis report No 3, 2005]</obo:IAO_0000115>
        <obo:IAO_0000412>http://langual.org</obo:IAO_0000412>
        <oboInOwl:hasDbXref>http://www.langual.org/langual_thesaurus.asp?termid=P0240</oboInOwl:hasDbXref>
        <rdfs:label xml:lang="en">modified ethnic food claim or use</rdfs:label>
    </owl:Class>
    


    <!-- http://purl.obolibrary.org/obo/FOODON_03510241 -->


    <owl:Class rdf:about="http://purl.obolibrary.org/obo/FOODON_03510241">
        <rdfs:subClassOf rdf:resource="http://purl.obolibrary.org/obo/FOODON_03510247"/>
        <obo:IAO_0000114 rdf:resource="http://purl.obolibrary.org/obo/IAO_0000428"/>
        <obo:IAO_0000115 xml:lang="en">COMMISSION REGULATION (EU) No 116/2010 of 9 February 2010 amending Regulation (EC) No 1924/2006 of the European Parliament and of the Council with regard to the list of nutrition claims.</obo:IAO_0000115>
        <obo:IAO_0000412>http://langual.org</obo:IAO_0000412>
        <oboInOwl:hasDbXref>http://www.langual.org/langual_thesaurus.asp?termid=P0241</oboInOwl:hasDbXref>
        <rdfs:label xml:lang="en">monounsaturated fat claim or use</rdfs:label>
    </owl:Class>
    


    <!-- http://purl.obolibrary.org/obo/FOODON_03510242 -->


    <owl:Class rdf:about="http://purl.obolibrary.org/obo/FOODON_03510242">
        <rdfs:subClassOf rdf:resource="http://purl.obolibrary.org/obo/FOODON_03510247"/>
        <obo:IAO_0000114 rdf:resource="http://purl.obolibrary.org/obo/IAO_0000428"/>
        <obo:IAO_0000115 xml:lang="en">COMMISSION REGULATION (EU) No 116/2010 of 9 February 2010 amending Regulation (EC) No 1924/2006 of the European Parliament and of the Council with regard to the list of nutrition claims</obo:IAO_0000115>
        <obo:IAO_0000412>http://langual.org</obo:IAO_0000412>
        <oboInOwl:hasDbXref>http://www.langual.org/langual_thesaurus.asp?termid=P0242</oboInOwl:hasDbXref>
        <rdfs:label xml:lang="en">polyunsaturated fat claim or use</rdfs:label>
    </owl:Class>
    


    <!-- http://purl.obolibrary.org/obo/FOODON_03510243 -->


    <owl:Class rdf:about="http://purl.obolibrary.org/obo/FOODON_03510243">
        <rdfs:subClassOf rdf:resource="http://purl.obolibrary.org/obo/FOODON_03510241"/>
        <obo:IAO_0000114 rdf:resource="http://purl.obolibrary.org/obo/IAO_0000428"/>
        <obo:IAO_0000115 xml:lang="en">A claim that a food is high in monounsaturated fat, and any claim likely to have the same meaning for the consumer, may only be made where at least 45 % of the fatty acids present in the product derive from monounsaturated fat under the condition that monounsaturated fat provides more than 20 % of energy of the product [COMMISSION REGULATION (EU) No 116/2010 of 9 February 2010 amending Regulation (EC) No 1924/2006 of the European Parliament and of the Council with regard to the list of nutrition claims].</obo:IAO_0000115>
        <obo:IAO_0000412>http://langual.org</obo:IAO_0000412>
        <oboInOwl:hasDbXref>http://www.langual.org/langual_thesaurus.asp?termid=P0243</oboInOwl:hasDbXref>
        <rdfs:label xml:lang="en">high monounsaturated fat</rdfs:label>
    </owl:Class>
    


    <!-- http://purl.obolibrary.org/obo/FOODON_03510244 -->


    <owl:Class rdf:about="http://purl.obolibrary.org/obo/FOODON_03510244">
        <rdfs:subClassOf rdf:resource="http://purl.obolibrary.org/obo/FOODON_03510242"/>
        <obo:IAO_0000114 rdf:resource="http://purl.obolibrary.org/obo/IAO_0000428"/>
        <obo:IAO_0000412>http://langual.org</obo:IAO_0000412>
        <oboInOwl:hasDbXref>http://www.langual.org/langual_thesaurus.asp?termid=P0244</oboInOwl:hasDbXref>
        <rdfs:label xml:lang="en">omega-3 fatty acids claim or use</rdfs:label>
    </owl:Class>
    


    <!-- http://purl.obolibrary.org/obo/FOODON_03510245 -->


    <owl:Class rdf:about="http://purl.obolibrary.org/obo/FOODON_03510245">
        <rdfs:subClassOf rdf:resource="http://purl.obolibrary.org/obo/FOODON_03510244"/>
        <obo:IAO_0000114 rdf:resource="http://purl.obolibrary.org/obo/IAO_0000428"/>
        <obo:IAO_0000115 xml:lang="en">A claim that a food is high in omega-3 fatty acids, and any claim likely to have the same meaning for the consumer, may only be made where the product contains at least 0,6 g alpha-linolenic acid per 100 g and per 100 kcal, or at least 80 mg of the sum of eicosapentaenoic acid and docosahexaenoic acid per 100 g and per 100 kcal [COMMISSION REGULATION (EU) No 116/2010 of 9 February 2010 amending Regulation (EC) No 1924/2006 of the European Parliament and of the Council with regard to the list of nutrition claims].</obo:IAO_0000115>
        <obo:IAO_0000412>http://langual.org</obo:IAO_0000412>
        <oboInOwl:hasDbXref>http://www.langual.org/langual_thesaurus.asp?termid=P0245</oboInOwl:hasDbXref>
        <rdfs:label xml:lang="en">high omega-3 fatty acids</rdfs:label>
    </owl:Class>
    


    <!-- http://purl.obolibrary.org/obo/FOODON_03510246 -->


    <owl:Class rdf:about="http://purl.obolibrary.org/obo/FOODON_03510246">
        <rdfs:subClassOf rdf:resource="http://purl.obolibrary.org/obo/FOODON_03510242"/>
        <obo:IAO_0000114 rdf:resource="http://purl.obolibrary.org/obo/IAO_0000428"/>
        <obo:IAO_0000115 xml:lang="en">A claim that a food is high in polyunsaturated fat, and any claim likely to have the same meaning for the consumer, may only be made where at least 45 % of the fatty acids present in the product derive from polyunsaturated fat under the condition that polyunsaturated fat provides more than 20 % of energy of the product [COMMISSION REGULATION (EU) No 116/2010 of 9 February 2010 amending Regulation (EC) No 1924/2006 of the European Parliament and of the Council with regard to the list of nutrition claims].</obo:IAO_0000115>
        <obo:IAO_0000412>http://langual.org</obo:IAO_0000412>
        <oboInOwl:hasDbXref>http://www.langual.org/langual_thesaurus.asp?termid=P0246</oboInOwl:hasDbXref>
        <rdfs:label xml:lang="en">high polyunsaturated fat</rdfs:label>
    </owl:Class>
    


    <!-- http://purl.obolibrary.org/obo/FOODON_03510247 -->


    <owl:Class rdf:about="http://purl.obolibrary.org/obo/FOODON_03510247">
        <rdfs:subClassOf rdf:resource="http://purl.obolibrary.org/obo/FOODON_03510017"/>
        <obo:IAO_0000114 rdf:resource="http://purl.obolibrary.org/obo/IAO_0000428"/>
        <obo:IAO_0000412>http://langual.org</obo:IAO_0000412>
        <oboInOwl:hasDbXref>http://www.langual.org/langual_thesaurus.asp?termid=P0247</oboInOwl:hasDbXref>
        <rdfs:label xml:lang="en">unsaturated fat claim or use</rdfs:label>
    </owl:Class>
    


    <!-- http://purl.obolibrary.org/obo/FOODON_03510248 -->


    <owl:Class rdf:about="http://purl.obolibrary.org/obo/FOODON_03510248">
        <rdfs:subClassOf rdf:resource="http://purl.obolibrary.org/obo/FOODON_03510247"/>
        <obo:IAO_0000114 rdf:resource="http://purl.obolibrary.org/obo/IAO_0000428"/>
        <obo:IAO_0000115 xml:lang="en">A claim that a food is high in unsaturated fat, and any claim likely to have the same meaning for the consumer may only be made where at least 70 % of the fatty acids present in the product derive from unsaturated fat under the condition that unsaturated fat provides more than 20 % of energy of the product [COMMISSION REGULATION (EU) No 116/2010 of 9 February 2010 amending Regulation (EC) No 1924/2006 of the European Parliament and of the Council with regard to the list of nutrition claims]..</obo:IAO_0000115>
        <obo:IAO_0000412>http://langual.org</obo:IAO_0000412>
        <oboInOwl:hasDbXref>http://www.langual.org/langual_thesaurus.asp?termid=P0248</oboInOwl:hasDbXref>
        <rdfs:label xml:lang="en">high unsaturated  fat</rdfs:label>
    </owl:Class>
    


    <!-- http://purl.obolibrary.org/obo/FOODON_03510249 -->


    <owl:Class rdf:about="http://purl.obolibrary.org/obo/FOODON_03510249">
        <rdfs:subClassOf rdf:resource="http://purl.obolibrary.org/obo/FOODON_03510244"/>
        <obo:IAO_0000114 rdf:resource="http://purl.obolibrary.org/obo/IAO_0000428"/>
        <obo:IAO_0000115 xml:lang="en">A claim that a food is a source of omega-3 fatty acids, and any claim likely to have the same meaning for the consumer, may only be made where the product contains at least 0,3 g alpha-linolenic acid per 100 g and per
100 kcal, or at least 40 mg of the sum of eicosapentaenoic acid and docosahexaenoic acid per 100 g and per 100 kcal [COMMISSION REGULATION (EU) No 116/2010 of 9 February 2010 amending Regulation (EC) No 1924/2006 of the European Parliament and of the Council with regard to the list of nutrition claims].</obo:IAO_0000115>
        <obo:IAO_0000412>http://langual.org</obo:IAO_0000412>
        <oboInOwl:hasDbXref>http://www.langual.org/langual_thesaurus.asp?termid=P0249</oboInOwl:hasDbXref>
        <rdfs:label xml:lang="en">source of omega-3 fatty acids</rdfs:label>
    </owl:Class>
    


    <!-- http://purl.obolibrary.org/obo/FOODON_03510257 -->


    <owl:Class rdf:about="http://purl.obolibrary.org/obo/FOODON_03510257">
        <rdfs:subClassOf rdf:resource="http://purl.obolibrary.org/obo/FOODON_03510124"/>
        <obo:IAO_0000114 rdf:resource="http://purl.obolibrary.org/obo/IAO_0000428"/>
        <obo:IAO_0000115 xml:lang="en">US FDA approved language lacking for the moment.</obo:IAO_0000115>
        <obo:IAO_0000412>http://langual.org</obo:IAO_0000412>
        <oboInOwl:hasDbXref>http://www.langual.org/langual_thesaurus.asp?termid=P0257</oboInOwl:hasDbXref>
        <rdfs:comment xml:lang="en">LanguaL curation note: Used in USA.</rdfs:comment>
        <rdfs:label xml:lang="en">calcium and osteoporosis related claim or use</rdfs:label>
    </owl:Class>
    


    <!-- http://purl.obolibrary.org/obo/FOODON_03510264 -->


    <owl:Class rdf:about="http://purl.obolibrary.org/obo/FOODON_03510264">
        <rdfs:subClassOf rdf:resource="http://purl.obolibrary.org/obo/FOODON_03510124"/>
        <obo:IAO_0000114 rdf:resource="http://purl.obolibrary.org/obo/IAO_0000428"/>
        <obo:IAO_0000115 xml:lang="en">In the United States, these claims, usually referred to as &quot;qualified health claims&quot;, are regulated by the Food and Drug Administration in the public interest, see 21 Code of Federal Regulations § 101.14 [http://www.accessdata.fda.gov/scripts/cdrh/cfdocs/cfcfr/CFRSearch.cfm?fr=101.14]</obo:IAO_0000115>
        <obo:IAO_0000412>http://langual.org</obo:IAO_0000412>
        <oboInOwl:hasDbXref>http://www.langual.org/langual_thesaurus.asp?termid=P0264</oboInOwl:hasDbXref>
        <rdfs:label xml:lang="en">qualified health claim</rdfs:label>
    </owl:Class>
    


    <!-- http://purl.obolibrary.org/obo/FOODON_03510265 -->


    <owl:Class rdf:about="http://purl.obolibrary.org/obo/FOODON_03510265">
        <rdfs:subClassOf rdf:resource="http://purl.obolibrary.org/obo/FOODON_03510124"/>
        <obo:IAO_0000114 rdf:resource="http://purl.obolibrary.org/obo/IAO_0000428"/>
        <obo:IAO_0000115 xml:lang="en">Structure/function claims describe the role of a nutrient or dietary ingredient intended to affect normal structure or function in humans, for example, &quot;calcium builds strong bones&quot;. In addition, they may characterize the means by which a nutrient or dietary ingredient acts to maintain such structure or function, for example, &quot;fiber maintains bowel regularity,&quot; or &quot;antioxidants maintain cell integrity,&quot; or they may describe general well-being from consumption of a nutrient or dietary ingredient. [http://www.fda.gov/Food/LabelingNutrition/LabelClaims/StructureFunctionClaims/default.htm]</obo:IAO_0000115>
        <obo:IAO_0000412>http://langual.org</obo:IAO_0000412>
        <oboInOwl:hasDbXref>http://www.langual.org/langual_thesaurus.asp?termid=P0265</oboInOwl:hasDbXref>
        <oboInOwl:hasSynonym xml:lang="en">article 13 health claims (european commission)</oboInOwl:hasSynonym>
        <oboInOwl:hasSynonym xml:lang="en">nutrient function claim (codex alimentarius)</oboInOwl:hasSynonym>
        <rdfs:label xml:lang="en">structure/function claim</rdfs:label>
    </owl:Class>
    


    <!-- http://purl.obolibrary.org/obo/FOODON_03510267 -->


    <owl:Class rdf:about="http://purl.obolibrary.org/obo/FOODON_03510267">
        <rdfs:subClassOf rdf:resource="http://purl.obolibrary.org/obo/FOODON_03510126"/>
        <obo:IAO_0000114 rdf:resource="http://purl.obolibrary.org/obo/IAO_0000428"/>
        <obo:IAO_0000412>http://langual.org</obo:IAO_0000412>
        <oboInOwl:hasDbXref>http://www.langual.org/langual_thesaurus.asp?termid=P0267</oboInOwl:hasDbXref>
        <rdfs:label xml:lang="en">native american food claim or use</rdfs:label>
    </owl:Class>
    


    <!-- http://purl.obolibrary.org/obo/FOODON_03510268 -->


    <owl:Class rdf:about="http://purl.obolibrary.org/obo/FOODON_03510268">
        <rdfs:subClassOf rdf:resource="http://purl.obolibrary.org/obo/FOODON_03510267"/>
        <obo:IAO_0000114 rdf:resource="http://purl.obolibrary.org/obo/IAO_0000428"/>
        <obo:IAO_0000412>http://langual.org</obo:IAO_0000412>
        <oboInOwl:hasDbXref>http://www.langual.org/langual_thesaurus.asp?termid=P0268</oboInOwl:hasDbXref>
        <rdfs:label xml:lang="en">alaskan native food claim or use</rdfs:label>
    </owl:Class>
    


    <!-- http://purl.obolibrary.org/obo/FOODON_03510269 -->


    <owl:Class rdf:about="http://purl.obolibrary.org/obo/FOODON_03510269">
        <rdfs:subClassOf rdf:resource="http://purl.obolibrary.org/obo/FOODON_03510267"/>
        <obo:IAO_0000114 rdf:resource="http://purl.obolibrary.org/obo/IAO_0000428"/>
        <obo:IAO_0000412>http://langual.org</obo:IAO_0000412>
        <oboInOwl:hasDbXref>http://www.langual.org/langual_thesaurus.asp?termid=P0269</oboInOwl:hasDbXref>
        <rdfs:label xml:lang="en">apache food claim or use</rdfs:label>
    </owl:Class>
    


    <!-- http://purl.obolibrary.org/obo/FOODON_03510270 -->


    <owl:Class rdf:about="http://purl.obolibrary.org/obo/FOODON_03510270">
        <rdfs:subClassOf rdf:resource="http://purl.obolibrary.org/obo/FOODON_03510267"/>
        <obo:IAO_0000114 rdf:resource="http://purl.obolibrary.org/obo/IAO_0000428"/>
        <obo:IAO_0000412>http://langual.org</obo:IAO_0000412>
        <oboInOwl:hasDbXref>http://www.langual.org/langual_thesaurus.asp?termid=P0270</oboInOwl:hasDbXref>
        <rdfs:label xml:lang="en">navajo food claim or use</rdfs:label>
    </owl:Class>
    


    <!-- http://purl.obolibrary.org/obo/FOODON_03510271 -->


    <owl:Class rdf:about="http://purl.obolibrary.org/obo/FOODON_03510271">
        <rdfs:subClassOf rdf:resource="http://purl.obolibrary.org/obo/FOODON_03510267"/>
        <obo:IAO_0000114 rdf:resource="http://purl.obolibrary.org/obo/IAO_0000428"/>
        <obo:IAO_0000412>http://langual.org</obo:IAO_0000412>
        <oboInOwl:hasDbXref>http://www.langual.org/langual_thesaurus.asp?termid=P0271</oboInOwl:hasDbXref>
        <rdfs:label xml:lang="en">shoshone bannock food claim or use</rdfs:label>
    </owl:Class>
    


    <!-- http://purl.obolibrary.org/obo/FOODON_03510272 -->


    <owl:Class rdf:about="http://purl.obolibrary.org/obo/FOODON_03510272">
        <rdfs:subClassOf rdf:resource="http://purl.obolibrary.org/obo/FOODON_03510267"/>
        <obo:IAO_0000114 rdf:resource="http://purl.obolibrary.org/obo/IAO_0000428"/>
        <obo:IAO_0000412>http://langual.org</obo:IAO_0000412>
        <oboInOwl:hasDbXref>http://www.langual.org/langual_thesaurus.asp?termid=P0272</oboInOwl:hasDbXref>
        <rdfs:label xml:lang="en">pacific food claim or use</rdfs:label>
    </owl:Class>
    


    <!-- http://purl.obolibrary.org/obo/FOODON_03510273 -->


    <owl:Class rdf:about="http://purl.obolibrary.org/obo/FOODON_03510273">
        <rdfs:subClassOf rdf:resource="http://purl.obolibrary.org/obo/FOODON_03510267"/>
        <obo:IAO_0000114 rdf:resource="http://purl.obolibrary.org/obo/IAO_0000428"/>
        <obo:IAO_0000412>http://langual.org</obo:IAO_0000412>
        <oboInOwl:hasDbXref>http://www.langual.org/langual_thesaurus.asp?termid=P0273</oboInOwl:hasDbXref>
        <rdfs:label xml:lang="en">northern plains food claim or use</rdfs:label>
    </owl:Class>
    


    <!-- http://purl.obolibrary.org/obo/FOODON_03510274 -->


    <owl:Class rdf:about="http://purl.obolibrary.org/obo/FOODON_03510274">
        <rdfs:subClassOf rdf:resource="http://purl.obolibrary.org/obo/FOODON_03510267"/>
        <obo:IAO_0000114 rdf:resource="http://purl.obolibrary.org/obo/IAO_0000428"/>
        <obo:IAO_0000412>http://langual.org</obo:IAO_0000412>
        <oboInOwl:hasDbXref>http://www.langual.org/langual_thesaurus.asp?termid=P0274</oboInOwl:hasDbXref>
        <rdfs:label xml:lang="en">southwest plains food claim or use</rdfs:label>
    </owl:Class>
    


    <!-- http://purl.obolibrary.org/obo/FOODON_03510275 -->


    <owl:Class rdf:about="http://purl.obolibrary.org/obo/FOODON_03510275">
        <rdfs:subClassOf rdf:resource="http://purl.obolibrary.org/obo/FOODON_03510267"/>
        <obo:IAO_0000114 rdf:resource="http://purl.obolibrary.org/obo/IAO_0000428"/>
        <obo:IAO_0000412>http://langual.org</obo:IAO_0000412>
        <oboInOwl:hasDbXref>http://www.langual.org/langual_thesaurus.asp?termid=P0275</oboInOwl:hasDbXref>
        <rdfs:label xml:lang="en">hopi food claim or use</rdfs:label>
    </owl:Class>
    


    <!-- http://purl.obolibrary.org/obo/FOODON_03510277 -->


    <owl:Class rdf:about="http://purl.obolibrary.org/obo/FOODON_03510277">
        <rdfs:subClassOf rdf:resource="http://purl.obolibrary.org/obo/FOODON_03510194"/>
        <obo:IAO_0000114 rdf:resource="http://purl.obolibrary.org/obo/IAO_0000428"/>
        <obo:IAO_0000412>http://langual.org</obo:IAO_0000412>
        <oboInOwl:hasDbXref>http://www.langual.org/langual_thesaurus.asp?termid=P0277</oboInOwl:hasDbXref>
        <oboInOwl:hasSynonym xml:lang="en">plant sterols or stanols claim or use</oboInOwl:hasSynonym>
        <rdfs:label xml:lang="en">phytosterol claim or use</rdfs:label>
    </owl:Class>
    


    <!-- http://purl.obolibrary.org/obo/FOODON_03530005 -->


    <owl:Class rdf:about="http://purl.obolibrary.org/obo/FOODON_03530005">
        <obo:IAO_0000114 rdf:resource="http://purl.obolibrary.org/obo/IAO_0000122"/>
        <obo:IAO_0000115 xml:lang="en">A data item consisting of a claim or record of a food product&apos;s origin or processing history or suitability for some purpose.</obo:IAO_0000115>
        <obo:IAO_0000117>Damion Dooley</obo:IAO_0000117>
        <obo:IAO_0000118 xml:lang="en">adjunct characteristics of food</obo:IAO_0000118>
        <obo:IAO_0000412>http://langual.org</obo:IAO_0000412>
        <oboInOwl:hasDbXref rdf:resource="http://www.langual.org/langual_thesaurus.asp?termid=Z0001"/>
        <oboInOwl:hasDbXref>http://www.langual.org/langual_thesaurus.asp?termid=Z0005</oboInOwl:hasDbXref>
        <rdfs:label xml:lang="en">food datum</rdfs:label>
    </owl:Class>
    


    <!-- http://purl.obolibrary.org/obo/FOODON_03530086 -->


    <owl:Class rdf:about="http://purl.obolibrary.org/obo/FOODON_03530086">
        <rdfs:subClassOf rdf:resource="http://purl.obolibrary.org/obo/FOODON_03530087"/>
        <obo:IAO_0000114 rdf:resource="http://purl.obolibrary.org/obo/IAO_0000428"/>
        <obo:IAO_0000115 xml:lang="en">The French certification granted to certain French geographical indications for wines, cheeses, butters, and other agricultural products, all under the auspices of the government bureau Institut National des Appellations d&apos;Origine (INAO). [Wikipedia]</obo:IAO_0000115>
        <obo:IAO_0000119 rdf:resource="https://en.wikipedia.org/wiki/Controlled_designation_of_origin"/>
        <obo:IAO_0000412>http://langual.org</obo:IAO_0000412>
        <oboInOwl:hasDbXref>http://www.langual.org/langual_thesaurus.asp?termid=Z0086</oboInOwl:hasDbXref>
        <oboInOwl:hasExactSynonym xml:lang="en">controlled designation of origin</oboInOwl:hasExactSynonym>
        <oboInOwl:hasSynonym xml:lang="en">controlled name</oboInOwl:hasSynonym>
        <oboInOwl:hasSynonym xml:lang="en">protected name</oboInOwl:hasSynonym>
        <rdfs:label xml:lang="en">Appellation d&apos;origine contrôlée</rdfs:label>
    </owl:Class>
    


    <!-- http://purl.obolibrary.org/obo/FOODON_03530087 -->


    <owl:Class rdf:about="http://purl.obolibrary.org/obo/FOODON_03530087">
        <rdfs:subClassOf rdf:resource="http://purl.obolibrary.org/obo/FOODON_03530005"/>
        <obo:IAO_0000114 rdf:resource="http://purl.obolibrary.org/obo/IAO_0000122"/>
        <obo:IAO_0000115 xml:lang="en">A datum indicating that use of a food product name is regulated within some legal framework.</obo:IAO_0000115>
        <oboInOwl:hasDbXref>http://www.langual.org/langual_thesaurus.asp?termid=Z0087</oboInOwl:hasDbXref>
        <rdfs:label xml:lang="en">food product appelation framework</rdfs:label>
    </owl:Class>
    


    <!-- http://purl.obolibrary.org/obo/FOODON_03530221 -->


    <owl:Class rdf:about="http://purl.obolibrary.org/obo/FOODON_03530221">
        <rdfs:subClassOf rdf:resource="http://purl.obolibrary.org/obo/FOODON_03530005"/>
        <obo:IAO_0000114 rdf:resource="http://purl.obolibrary.org/obo/IAO_0000428"/>
        <obo:IAO_0000115 xml:lang="en">US FDA 1995 Code:  HA00</obo:IAO_0000115>
        <obo:IAO_0000412>http://langual.org</obo:IAO_0000412>
        <oboInOwl:hasDbXref>http://www.langual.org/langual_thesaurus.asp?termid=Z0221</oboInOwl:hasDbXref>
        <rdfs:label xml:lang="en">haccp guide food safety term</rdfs:label>
    </owl:Class>
    


    <!-- http://purl.obolibrary.org/obo/FOODON_03530222 -->


    <owl:Class rdf:about="http://purl.obolibrary.org/obo/FOODON_03530222">
        <rdfs:subClassOf rdf:resource="http://purl.obolibrary.org/obo/FOODON_03530221"/>
        <obo:IAO_0000114 rdf:resource="http://purl.obolibrary.org/obo/IAO_0000428"/>
        <obo:IAO_0000412>http://langual.org</obo:IAO_0000412>
        <oboInOwl:hasDbXref>http://www.langual.org/langual_thesaurus.asp?termid=Z0222</oboInOwl:hasDbXref>
        <rdfs:comment xml:lang="en">LanguaL curation note: US FDA 1995 Code:  ANIN</rdfs:comment>
        <rdfs:label xml:lang="en">anisakis infestation</rdfs:label>
    </owl:Class>
    


    <!-- http://purl.obolibrary.org/obo/FOODON_03530223 -->


    <owl:Class rdf:about="http://purl.obolibrary.org/obo/FOODON_03530223">
        <rdfs:subClassOf rdf:resource="http://purl.obolibrary.org/obo/FOODON_03530221"/>
        <obo:IAO_0000114 rdf:resource="http://purl.obolibrary.org/obo/IAO_0000428"/>
        <obo:IAO_0000412>http://langual.org</obo:IAO_0000412>
        <oboInOwl:hasDbXref>http://www.langual.org/langual_thesaurus.asp?termid=Z0223</oboInOwl:hasDbXref>
        <rdfs:comment xml:lang="en">LanguaL curation note: US FDA 1995 Code:  ASFP</rdfs:comment>
        <rdfs:label xml:lang="en">amnesic shellfish poisoning</rdfs:label>
    </owl:Class>
    


    <!-- http://purl.obolibrary.org/obo/FOODON_03530224 -->


    <owl:Class rdf:about="http://purl.obolibrary.org/obo/FOODON_03530224">
        <rdfs:subClassOf rdf:resource="http://purl.obolibrary.org/obo/FOODON_03530221"/>
        <obo:IAO_0000114 rdf:resource="http://purl.obolibrary.org/obo/IAO_0000428"/>
        <obo:IAO_0000412>http://langual.org</obo:IAO_0000412>
        <oboInOwl:hasDbXref>http://www.langual.org/langual_thesaurus.asp?termid=Z0224</oboInOwl:hasDbXref>
        <rdfs:comment xml:lang="en">LanguaL curation note: US FDA 1995 Code:  CGTX</rdfs:comment>
        <rdfs:label xml:lang="en">ciguatoxic</rdfs:label>
    </owl:Class>
    


    <!-- http://purl.obolibrary.org/obo/FOODON_03530225 -->


    <owl:Class rdf:about="http://purl.obolibrary.org/obo/FOODON_03530225">
        <rdfs:subClassOf rdf:resource="http://purl.obolibrary.org/obo/FOODON_03530221"/>
        <obo:IAO_0000114 rdf:resource="http://purl.obolibrary.org/obo/IAO_0000428"/>
        <obo:IAO_0000412>http://langual.org</obo:IAO_0000412>
        <oboInOwl:hasDbXref>http://www.langual.org/langual_thesaurus.asp?termid=Z0225</oboInOwl:hasDbXref>
        <rdfs:comment xml:lang="en">LanguaL curation note: US FDA 1995 Code:  CHFP</rdfs:comment>
        <rdfs:label xml:lang="en">chimaeroid poisoning</rdfs:label>
    </owl:Class>
    


    <!-- http://purl.obolibrary.org/obo/FOODON_03530226 -->


    <owl:Class rdf:about="http://purl.obolibrary.org/obo/FOODON_03530226">
        <rdfs:subClassOf rdf:resource="http://purl.obolibrary.org/obo/FOODON_03530221"/>
        <obo:IAO_0000114 rdf:resource="http://purl.obolibrary.org/obo/IAO_0000428"/>
        <obo:IAO_0000412>http://langual.org</obo:IAO_0000412>
        <oboInOwl:hasDbXref>http://www.langual.org/langual_thesaurus.asp?termid=Z0226</oboInOwl:hasDbXref>
        <rdfs:comment xml:lang="en">LanguaL curation note: US FDA 1995 Code:  CPFP</rdfs:comment>
        <rdfs:label xml:lang="en">clupeotoxic poisoning</rdfs:label>
    </owl:Class>
    


    <!-- http://purl.obolibrary.org/obo/FOODON_03530227 -->


    <owl:Class rdf:about="http://purl.obolibrary.org/obo/FOODON_03530227">
        <rdfs:subClassOf rdf:resource="http://purl.obolibrary.org/obo/FOODON_03530221"/>
        <obo:IAO_0000114 rdf:resource="http://purl.obolibrary.org/obo/IAO_0000428"/>
        <obo:IAO_0000412>http://langual.org</obo:IAO_0000412>
        <oboInOwl:hasDbXref>http://www.langual.org/langual_thesaurus.asp?termid=Z0227</oboInOwl:hasDbXref>
        <rdfs:comment xml:lang="en">LanguaL curation note: US FDA 1995 Code:  DBIN</rdfs:comment>
        <rdfs:label xml:lang="en">diphyllobothrium infestation</rdfs:label>
    </owl:Class>
    


    <!-- http://purl.obolibrary.org/obo/FOODON_03530228 -->


    <owl:Class rdf:about="http://purl.obolibrary.org/obo/FOODON_03530228">
        <rdfs:subClassOf rdf:resource="http://purl.obolibrary.org/obo/FOODON_03530221"/>
        <obo:IAO_0000114 rdf:resource="http://purl.obolibrary.org/obo/IAO_0000428"/>
        <obo:IAO_0000412>http://langual.org</obo:IAO_0000412>
        <oboInOwl:hasDbXref>http://www.langual.org/langual_thesaurus.asp?termid=Z0228</oboInOwl:hasDbXref>
        <rdfs:comment xml:lang="en">LanguaL curation note: US FDA 1995 Code:  DSFP</rdfs:comment>
        <rdfs:label xml:lang="en">diarrhetic shellfish poisoning</rdfs:label>
    </owl:Class>
    


    <!-- http://purl.obolibrary.org/obo/FOODON_03530229 -->


    <owl:Class rdf:about="http://purl.obolibrary.org/obo/FOODON_03530229">
        <rdfs:subClassOf rdf:resource="http://purl.obolibrary.org/obo/FOODON_03530221"/>
        <obo:IAO_0000114 rdf:resource="http://purl.obolibrary.org/obo/IAO_0000428"/>
        <obo:IAO_0000412>http://langual.org</obo:IAO_0000412>
        <oboInOwl:hasDbXref>http://www.langual.org/langual_thesaurus.asp?termid=Z0229</oboInOwl:hasDbXref>
        <rdfs:comment xml:lang="en">LanguaL curation note: US FDA 1995 Code:  HA01</rdfs:comment>
        <rdfs:label xml:lang="en">hazard 1</rdfs:label>
    </owl:Class>
    


    <!-- http://purl.obolibrary.org/obo/FOODON_03530230 -->


    <owl:Class rdf:about="http://purl.obolibrary.org/obo/FOODON_03530230">
        <rdfs:subClassOf rdf:resource="http://purl.obolibrary.org/obo/FOODON_03530221"/>
        <obo:IAO_0000114 rdf:resource="http://purl.obolibrary.org/obo/IAO_0000428"/>
        <obo:IAO_0000412>http://langual.org</obo:IAO_0000412>
        <oboInOwl:hasDbXref>http://www.langual.org/langual_thesaurus.asp?termid=Z0230</oboInOwl:hasDbXref>
        <rdfs:comment xml:lang="en">LanguaL curation note: US FDA 1995 Code:  HA02</rdfs:comment>
        <rdfs:label xml:lang="en">hazard 2</rdfs:label>
    </owl:Class>
    


    <!-- http://purl.obolibrary.org/obo/FOODON_03530231 -->


    <owl:Class rdf:about="http://purl.obolibrary.org/obo/FOODON_03530231">
        <rdfs:subClassOf rdf:resource="http://purl.obolibrary.org/obo/FOODON_03530221"/>
        <obo:IAO_0000114 rdf:resource="http://purl.obolibrary.org/obo/IAO_0000428"/>
        <obo:IAO_0000412>http://langual.org</obo:IAO_0000412>
        <oboInOwl:hasDbXref>http://www.langual.org/langual_thesaurus.asp?termid=Z0231</oboInOwl:hasDbXref>
        <rdfs:comment xml:lang="en">LanguaL curation note: US FDA 1995 Code:  HA03</rdfs:comment>
        <rdfs:label xml:lang="en">hazard 3</rdfs:label>
    </owl:Class>
    


    <!-- http://purl.obolibrary.org/obo/FOODON_03530232 -->


    <owl:Class rdf:about="http://purl.obolibrary.org/obo/FOODON_03530232">
        <rdfs:subClassOf rdf:resource="http://purl.obolibrary.org/obo/FOODON_03530221"/>
        <obo:IAO_0000114 rdf:resource="http://purl.obolibrary.org/obo/IAO_0000428"/>
        <obo:IAO_0000412>http://langual.org</obo:IAO_0000412>
        <oboInOwl:hasDbXref>http://www.langual.org/langual_thesaurus.asp?termid=Z0232</oboInOwl:hasDbXref>
        <rdfs:comment xml:lang="en">LanguaL curation note: US FDA 1995 Code:  HA04</rdfs:comment>
        <rdfs:label xml:lang="en">hazard 4</rdfs:label>
    </owl:Class>
    


    <!-- http://purl.obolibrary.org/obo/FOODON_03530233 -->


    <owl:Class rdf:about="http://purl.obolibrary.org/obo/FOODON_03530233">
        <rdfs:subClassOf rdf:resource="http://purl.obolibrary.org/obo/FOODON_03530221"/>
        <obo:IAO_0000114 rdf:resource="http://purl.obolibrary.org/obo/IAO_0000428"/>
        <obo:IAO_0000412>http://langual.org</obo:IAO_0000412>
        <oboInOwl:hasDbXref>http://www.langual.org/langual_thesaurus.asp?termid=Z0233</oboInOwl:hasDbXref>
        <rdfs:comment xml:lang="en">LanguaL curation note: US FDA 1995 Code:  HA05</rdfs:comment>
        <rdfs:label xml:lang="en">hazard 5</rdfs:label>
    </owl:Class>
    


    <!-- http://purl.obolibrary.org/obo/FOODON_03530234 -->


    <owl:Class rdf:about="http://purl.obolibrary.org/obo/FOODON_03530234">
        <rdfs:subClassOf rdf:resource="http://purl.obolibrary.org/obo/FOODON_03530221"/>
        <obo:IAO_0000114 rdf:resource="http://purl.obolibrary.org/obo/IAO_0000428"/>
        <obo:IAO_0000412>http://langual.org</obo:IAO_0000412>
        <oboInOwl:hasDbXref>http://www.langual.org/langual_thesaurus.asp?termid=Z0234</oboInOwl:hasDbXref>
        <rdfs:comment xml:lang="en">LanguaL curation note: US FDA 1995 Code:  HA06</rdfs:comment>
        <rdfs:label xml:lang="en">hazard 6</rdfs:label>
    </owl:Class>
    


    <!-- http://purl.obolibrary.org/obo/FOODON_03530235 -->


    <owl:Class rdf:about="http://purl.obolibrary.org/obo/FOODON_03530235">
        <rdfs:subClassOf rdf:resource="http://purl.obolibrary.org/obo/FOODON_03530221"/>
        <obo:IAO_0000114 rdf:resource="http://purl.obolibrary.org/obo/IAO_0000428"/>
        <obo:IAO_0000412>http://langual.org</obo:IAO_0000412>
        <oboInOwl:hasDbXref>http://www.langual.org/langual_thesaurus.asp?termid=Z0235</oboInOwl:hasDbXref>
        <rdfs:comment xml:lang="en">LanguaL curation note: US FDA 1995 Code:  HA07</rdfs:comment>
        <rdfs:label xml:lang="en">hazard 7</rdfs:label>
    </owl:Class>
    


    <!-- http://purl.obolibrary.org/obo/FOODON_03530236 -->


    <owl:Class rdf:about="http://purl.obolibrary.org/obo/FOODON_03530236">
        <rdfs:subClassOf rdf:resource="http://purl.obolibrary.org/obo/FOODON_03530221"/>
        <obo:IAO_0000114 rdf:resource="http://purl.obolibrary.org/obo/IAO_0000428"/>
        <obo:IAO_0000412>http://langual.org</obo:IAO_0000412>
        <oboInOwl:hasDbXref>http://www.langual.org/langual_thesaurus.asp?termid=Z0236</oboInOwl:hasDbXref>
        <rdfs:comment xml:lang="en">LanguaL curation note: US FDA 1995 Code:  HA08</rdfs:comment>
        <rdfs:label xml:lang="en">hazard 8</rdfs:label>
    </owl:Class>
    


    <!-- http://purl.obolibrary.org/obo/FOODON_03530237 -->


    <owl:Class rdf:about="http://purl.obolibrary.org/obo/FOODON_03530237">
        <rdfs:subClassOf rdf:resource="http://purl.obolibrary.org/obo/FOODON_03530221"/>
        <obo:IAO_0000114 rdf:resource="http://purl.obolibrary.org/obo/IAO_0000428"/>
        <obo:IAO_0000412>http://langual.org</obo:IAO_0000412>
        <oboInOwl:hasDbXref>http://www.langual.org/langual_thesaurus.asp?termid=Z0237</oboInOwl:hasDbXref>
        <rdfs:comment xml:lang="en">LanguaL curation note: US FDA 1995 Code:  HA09</rdfs:comment>
        <rdfs:label xml:lang="en">hazard 9</rdfs:label>
    </owl:Class>
    


    <!-- http://purl.obolibrary.org/obo/FOODON_03530238 -->


    <owl:Class rdf:about="http://purl.obolibrary.org/obo/FOODON_03530238">
        <rdfs:subClassOf rdf:resource="http://purl.obolibrary.org/obo/FOODON_03530221"/>
        <obo:IAO_0000114 rdf:resource="http://purl.obolibrary.org/obo/IAO_0000428"/>
        <obo:IAO_0000412>http://langual.org</obo:IAO_0000412>
        <oboInOwl:hasDbXref>http://www.langual.org/langual_thesaurus.asp?termid=Z0238</oboInOwl:hasDbXref>
        <rdfs:comment xml:lang="en">LanguaL curation note: US FDA 1995 Code:  HA10</rdfs:comment>
        <rdfs:label xml:lang="en">hazard 10</rdfs:label>
    </owl:Class>
    


    <!-- http://purl.obolibrary.org/obo/FOODON_03530239 -->


    <owl:Class rdf:about="http://purl.obolibrary.org/obo/FOODON_03530239">
        <rdfs:subClassOf rdf:resource="http://purl.obolibrary.org/obo/FOODON_03530221"/>
        <obo:IAO_0000114 rdf:resource="http://purl.obolibrary.org/obo/IAO_0000428"/>
        <obo:IAO_0000412>http://langual.org</obo:IAO_0000412>
        <oboInOwl:hasDbXref>http://www.langual.org/langual_thesaurus.asp?termid=Z0239</oboInOwl:hasDbXref>
        <rdfs:comment xml:lang="en">LanguaL curation note: US FDA 1995 Code:  IAFP</rdfs:comment>
        <rdfs:label xml:lang="en">ichthyoallyeinotoxic poisoning</rdfs:label>
    </owl:Class>
    


    <!-- http://purl.obolibrary.org/obo/FOODON_03530240 -->


    <owl:Class rdf:about="http://purl.obolibrary.org/obo/FOODON_03530240">
        <rdfs:subClassOf rdf:resource="http://purl.obolibrary.org/obo/FOODON_03530221"/>
        <obo:IAO_0000114 rdf:resource="http://purl.obolibrary.org/obo/IAO_0000428"/>
        <obo:IAO_0000412>http://langual.org</obo:IAO_0000412>
        <oboInOwl:hasDbXref>http://www.langual.org/langual_thesaurus.asp?termid=Z0240</oboInOwl:hasDbXref>
        <rdfs:comment xml:lang="en">LanguaL curation note: US FDA 1995 Code:  ICFP</rdfs:comment>
        <rdfs:label xml:lang="en">ichthyocrinotoxic poisoning</rdfs:label>
    </owl:Class>
    


    <!-- http://purl.obolibrary.org/obo/FOODON_03530241 -->


    <owl:Class rdf:about="http://purl.obolibrary.org/obo/FOODON_03530241">
        <rdfs:subClassOf rdf:resource="http://purl.obolibrary.org/obo/FOODON_03530221"/>
        <obo:IAO_0000114 rdf:resource="http://purl.obolibrary.org/obo/IAO_0000428"/>
        <obo:IAO_0000412>http://langual.org</obo:IAO_0000412>
        <oboInOwl:hasDbXref>http://www.langual.org/langual_thesaurus.asp?termid=Z0241</oboInOwl:hasDbXref>
        <rdfs:comment xml:lang="en">LanguaL curation note: US FDA 1995 Code:  IHFP</rdfs:comment>
        <rdfs:label xml:lang="en">ichthyohepatotoxic poisoning</rdfs:label>
    </owl:Class>
    


    <!-- http://purl.obolibrary.org/obo/FOODON_03530242 -->


    <owl:Class rdf:about="http://purl.obolibrary.org/obo/FOODON_03530242">
        <rdfs:subClassOf rdf:resource="http://purl.obolibrary.org/obo/FOODON_03530221"/>
        <obo:IAO_0000114 rdf:resource="http://purl.obolibrary.org/obo/IAO_0000428"/>
        <obo:IAO_0000412>http://langual.org</obo:IAO_0000412>
        <oboInOwl:hasDbXref>http://www.langual.org/langual_thesaurus.asp?termid=Z0242</oboInOwl:hasDbXref>
        <rdfs:comment xml:lang="en">LanguaL curation note: US FDA 1995 Code:  IOFP</rdfs:comment>
        <rdfs:label xml:lang="en">ichthyootoxic poisoning</rdfs:label>
    </owl:Class>
    


    <!-- http://purl.obolibrary.org/obo/FOODON_03530243 -->


    <owl:Class rdf:about="http://purl.obolibrary.org/obo/FOODON_03530243">
        <rdfs:subClassOf rdf:resource="http://purl.obolibrary.org/obo/FOODON_03530221"/>
        <obo:IAO_0000114 rdf:resource="http://purl.obolibrary.org/obo/IAO_0000428"/>
        <obo:IAO_0000412>http://langual.org</obo:IAO_0000412>
        <oboInOwl:hasDbXref>http://www.langual.org/langual_thesaurus.asp?termid=Z0243</oboInOwl:hasDbXref>
        <rdfs:comment xml:lang="en">LanguaL curation note: US FDA 1995 Code:  LEPO</rdfs:comment>
        <rdfs:label xml:lang="en">lead poisoning</rdfs:label>
    </owl:Class>
    


    <!-- http://purl.obolibrary.org/obo/FOODON_03530244 -->


    <owl:Class rdf:about="http://purl.obolibrary.org/obo/FOODON_03530244">
        <rdfs:subClassOf rdf:resource="http://purl.obolibrary.org/obo/FOODON_03530221"/>
        <obo:IAO_0000114 rdf:resource="http://purl.obolibrary.org/obo/IAO_0000428"/>
        <obo:IAO_0000412>http://langual.org</obo:IAO_0000412>
        <oboInOwl:hasDbXref>http://www.langual.org/langual_thesaurus.asp?termid=Z0244</oboInOwl:hasDbXref>
        <rdfs:comment xml:lang="en">LanguaL curation note: US FDA 1995 Code:  NATP</rdfs:comment>
        <rdfs:label xml:lang="en">sodium tripolyphosphate</rdfs:label>
    </owl:Class>
    


    <!-- http://purl.obolibrary.org/obo/FOODON_03530245 -->


    <owl:Class rdf:about="http://purl.obolibrary.org/obo/FOODON_03530245">
        <rdfs:subClassOf rdf:resource="http://purl.obolibrary.org/obo/FOODON_03530221"/>
        <obo:IAO_0000114 rdf:resource="http://purl.obolibrary.org/obo/IAO_0000428"/>
        <obo:IAO_0000412>http://langual.org</obo:IAO_0000412>
        <oboInOwl:hasDbXref>http://www.langual.org/langual_thesaurus.asp?termid=Z0245</oboInOwl:hasDbXref>
        <rdfs:comment xml:lang="en">LanguaL curation note: US FDA 1995 Code:  NMIN</rdfs:comment>
        <rdfs:label xml:lang="en">nematode infestation</rdfs:label>
    </owl:Class>
    


    <!-- http://purl.obolibrary.org/obo/FOODON_03530246 -->


    <owl:Class rdf:about="http://purl.obolibrary.org/obo/FOODON_03530246">
        <rdfs:subClassOf rdf:resource="http://purl.obolibrary.org/obo/FOODON_03530221"/>
        <obo:IAO_0000114 rdf:resource="http://purl.obolibrary.org/obo/IAO_0000428"/>
        <obo:IAO_0000412>http://langual.org</obo:IAO_0000412>
        <oboInOwl:hasDbXref>http://www.langual.org/langual_thesaurus.asp?termid=Z0246</oboInOwl:hasDbXref>
        <rdfs:comment xml:lang="en">LanguaL curation note: US FDA 1995 Code:  NSFP</rdfs:comment>
        <rdfs:label xml:lang="en">neurotoxic shellfish poisoning</rdfs:label>
    </owl:Class>
    


    <!-- http://purl.obolibrary.org/obo/FOODON_03530247 -->


    <owl:Class rdf:about="http://purl.obolibrary.org/obo/FOODON_03530247">
        <rdfs:subClassOf rdf:resource="http://purl.obolibrary.org/obo/FOODON_03530221"/>
        <obo:IAO_0000114 rdf:resource="http://purl.obolibrary.org/obo/IAO_0000428"/>
        <obo:IAO_0000412>http://langual.org</obo:IAO_0000412>
        <oboInOwl:hasDbXref>http://www.langual.org/langual_thesaurus.asp?termid=Z0247</oboInOwl:hasDbXref>
        <rdfs:comment xml:lang="en">LanguaL curation note: US FDA 1995 Code:  PSFP</rdfs:comment>
        <rdfs:label xml:lang="en">paralytic shellfish poisoning</rdfs:label>
    </owl:Class>
    


    <!-- http://purl.obolibrary.org/obo/FOODON_03530248 -->


    <owl:Class rdf:about="http://purl.obolibrary.org/obo/FOODON_03530248">
        <rdfs:subClassOf rdf:resource="http://purl.obolibrary.org/obo/FOODON_03530221"/>
        <obo:IAO_0000114 rdf:resource="http://purl.obolibrary.org/obo/IAO_0000428"/>
        <obo:IAO_0000412>http://langual.org</obo:IAO_0000412>
        <oboInOwl:hasDbXref>http://www.langual.org/langual_thesaurus.asp?termid=Z0248</oboInOwl:hasDbXref>
        <rdfs:comment xml:lang="en">LanguaL curation note: US FDA 1995 Code:  SCOM</rdfs:comment>
        <rdfs:label xml:lang="en">scombrotoxic</rdfs:label>
    </owl:Class>
    


    <!-- http://purl.obolibrary.org/obo/FOODON_03530249 -->


    <owl:Class rdf:about="http://purl.obolibrary.org/obo/FOODON_03530249">
        <rdfs:subClassOf rdf:resource="http://purl.obolibrary.org/obo/FOODON_03530221"/>
        <obo:IAO_0000114 rdf:resource="http://purl.obolibrary.org/obo/IAO_0000428"/>
        <obo:IAO_0000412>http://langual.org</obo:IAO_0000412>
        <oboInOwl:hasDbXref>http://www.langual.org/langual_thesaurus.asp?termid=Z0249</oboInOwl:hasDbXref>
        <rdfs:comment xml:lang="en">LanguaL curation note: US FDA 1995 Code:  TDFP</rdfs:comment>
        <rdfs:label xml:lang="en">tetrodotoxic poisoning</rdfs:label>
    </owl:Class>
    


    <!-- http://purl.obolibrary.org/obo/FOODON_03530250 -->


    <owl:Class rdf:about="http://purl.obolibrary.org/obo/FOODON_03530250">
        <rdfs:subClassOf rdf:resource="http://purl.obolibrary.org/obo/FOODON_03530221"/>
        <obo:IAO_0000114 rdf:resource="http://purl.obolibrary.org/obo/IAO_0000428"/>
        <obo:IAO_0000412>http://langual.org</obo:IAO_0000412>
        <oboInOwl:hasDbXref>http://www.langual.org/langual_thesaurus.asp?termid=Z0250</oboInOwl:hasDbXref>
        <rdfs:comment xml:lang="en">LanguaL curation note: US FDA 1995 Code:  PCBP</rdfs:comment>
        <rdfs:label xml:lang="en">chlorinated biphenyl</rdfs:label>
    </owl:Class>
    


    <!-- http://purl.obolibrary.org/obo/FOODON_03530254 -->


    <owl:Class rdf:about="http://purl.obolibrary.org/obo/FOODON_03530254">
        <rdfs:subClassOf rdf:resource="http://purl.obolibrary.org/obo/FOODON_03530087"/>
        <obo:IAO_0000114 rdf:resource="http://purl.obolibrary.org/obo/IAO_0000428"/>
        <obo:IAO_0000115 xml:lang="en">A legal framework defined in European Union law to protect the names of regional foods.</obo:IAO_0000115>
        <obo:IAO_0000119 rdf:resource="https://en.wikipedia.org/wiki/Geographical_indications_and_traditional_specialities_in_the_European_Union"/>
        <obo:IAO_0000412>http://langual.org</obo:IAO_0000412>
        <oboInOwl:hasDbXref>http://www.langual.org/langual_thesaurus.asp?termid=Z0254</oboInOwl:hasDbXref>
        <oboInOwl:hasExactSynonym xml:lang="en">PGS</oboInOwl:hasExactSynonym>
        <rdfs:comment xml:lang="en">Protected Designation of Origin (PDO), Protected Geographical Indication (PGI) and Traditional Speciality Guaranteed (TSG) are geographical indications, or more precisely regimes, within the framework. The law (enforced within the EU and being gradually expanded internationally via bilateral agreements of the EU with non-EU countries) ensures that only products genuinely originating in that region are allowed in commerce as such. The legislation came into force in 1992. The purpose of the law is to protect the reputation of the regional foods and eliminate the unfair competition and misleading of consumers by non-genuine products, which may be of inferior quality or of different flavour. [https://en.wikipedia.org/wiki/Geographical_indications_and_traditional_specialities_in_the_European_Union#Protected_geographical_indication_(PGI)]</rdfs:comment>
        <rdfs:label xml:lang="en">Protected Geographical Status</rdfs:label>
        <rdfs:seeAlso rdf:resource="http://ec.europa.eu/agriculture/quality/index_en.htm"/>
    </owl:Class>
    


    <!-- http://purl.obolibrary.org/obo/FOODON_03530255 -->


    <owl:Class rdf:about="http://purl.obolibrary.org/obo/FOODON_03530255">
        <rdfs:subClassOf rdf:resource="http://purl.obolibrary.org/obo/FOODON_03530254"/>
        <obo:IAO_0000114 rdf:resource="http://purl.obolibrary.org/obo/IAO_0000428"/>
        <obo:IAO_0000115 xml:lang="en">A Protected Geographical Status which covers agricultural products and foodstuffs which are produced, processed and prepared in a given geographical area using recognised know-how.</obo:IAO_0000115>
        <obo:IAO_0000119 rdf:resource="http://ec.europa.eu/agriculture/quality/schemes/index_en.htm"/>
        <obo:IAO_0000412>http://langual.org</obo:IAO_0000412>
        <oboInOwl:hasDbXref>http://www.langual.org/langual_thesaurus.asp?termid=Z0255</oboInOwl:hasDbXref>
        <oboInOwl:hasExactSynonym xml:lang="en">PDO</oboInOwl:hasExactSynonym>
        <rdfs:label xml:lang="en">Protected Designation of Origin</rdfs:label>
    </owl:Class>
    


    <!-- http://purl.obolibrary.org/obo/FOODON_03530256 -->


    <owl:Class rdf:about="http://purl.obolibrary.org/obo/FOODON_03530256">
        <rdfs:subClassOf rdf:resource="http://purl.obolibrary.org/obo/FOODON_03530254"/>
        <obo:IAO_0000114 rdf:resource="http://purl.obolibrary.org/obo/IAO_0000122"/>
        <obo:IAO_0000115 xml:lang="en">A Protected Geographical Status which covers agricultural products and foodstuffs closely linked to the geographical area.</obo:IAO_0000115>
        <obo:IAO_0000119 rdf:resource="http://ec.europa.eu/agriculture/quality/schemes/index_en.htm"/>
        <obo:IAO_0000412>http://langual.org</obo:IAO_0000412>
        <oboInOwl:hasDbXref>http://www.langual.org/langual_thesaurus.asp?termid=Z0256</oboInOwl:hasDbXref>
        <oboInOwl:hasExactSynonym xml:lang="en">PGI</oboInOwl:hasExactSynonym>
        <rdfs:comment xml:lang="en">&quot;At least one of the stages of production, processing or preparation takes place in the area.&quot; [http://ec.europa.eu/agriculture/quality/schemes/index_en.htm].</rdfs:comment>
        <rdfs:label xml:lang="en">Protected Geographical Indication</rdfs:label>
    </owl:Class>
    


    <!-- http://purl.obolibrary.org/obo/FOODON_03530257 -->


    <owl:Class rdf:about="http://purl.obolibrary.org/obo/FOODON_03530257">
        <rdfs:subClassOf rdf:resource="http://purl.obolibrary.org/obo/FOODON_03530254"/>
        <obo:IAO_0000114 rdf:resource="http://purl.obolibrary.org/obo/IAO_0000122"/>
        <obo:IAO_0000115 xml:lang="en">A Protected Geographical Status which highlights traditional character, either in the composition or means of production.</obo:IAO_0000115>
        <obo:IAO_0000119 rdf:resource="http://ec.europa.eu/agriculture/quality/schemes/index_en.htm"/>
        <obo:IAO_0000412>http://langual.org</obo:IAO_0000412>
        <oboInOwl:hasDbXref>http://www.langual.org/langual_thesaurus.asp?termid=Z0257</oboInOwl:hasDbXref>
        <oboInOwl:hasExactSynonym xml:lang="en">TSG</oboInOwl:hasExactSynonym>
        <rdfs:label xml:lang="en">Traditional Speciality Guaranteed</rdfs:label>
    </owl:Class>
    


    <!-- http://purl.obolibrary.org/obo/FOODON_03530258 -->


    <owl:Class rdf:about="http://purl.obolibrary.org/obo/FOODON_03530258">
        <rdfs:subClassOf rdf:resource="http://purl.obolibrary.org/obo/FOODON_03530087"/>
        <rdfs:label xml:lang="en">Denominazione di origine controllata</rdfs:label>
    </owl:Class>
</rdf:RDF>



<!-- Generated by the OWL API (version 5.1.18) https://github.com/owlcs/owlapi/ -->


